<?xml version="1.0" encoding="UTF-8"?>
<rdf:RDF xmlns:skos="http://www.w3.org/2004/02/skos/core#"
	xmlns:dc="http://purl.org/dc/elements/1.1/"
	xmlns:rdf="http://www.w3.org/1999/02/22-rdf-syntax-ns#"
	xmlns:rdfs="http://www.w3.org/2000/01/rdf-schema#">
	<skos:ConceptScheme rdf:about="urn:cgi:classifierScheme:CGI:SimpleLithology:2008">
		<skos:prefLabel xml:lang="en">Simple Lithology</skos:prefLabel>
		<skos:changeNote>
			<rdf:Description>
				<rdf:value>
					Converted manually from xls document https://www.seegrid.csiro.au/subversion/GeoSciML/tags/Vocabulary_200811/SimpleLithology200811.xls 
					in order to demonstrate SKOS encoding
					
					rdfs:isDefinedBy used to link to source ref
					
					skos:related used to link to Genetic Category
				</rdf:value>
				<dc:date>2009-05-07</dc:date>
				<dc:creator>Simon Cox</dc:creator>
			</rdf:Description>
		</skos:changeNote>
		<skos:editorialNote>Links to ParticleType, grainSize, ChemicalCategory, PetrographicCategory, FabricType, Shape, Sorting, ConsolidationDegree, not yet present  added</skos:editorialNote>
		<skos:hasTopConcept
			rdf:resource="urn:cgi:classifier:CGI:SimpleLithology:2008:compound_material"/>
		<skos:hasTopConcept rdf:resource="urn:cgi:classifier:CGI:SimpleLithology:2008:breccia"/>
		<skos:hasTopConcept
			rdf:resource="urn:cgi:classifier:CGI:SimpleLithology:2008:composite_genesis_material"/>
		<skos:hasTopConcept
			rdf:resource="urn:cgi:classifier:CGI:SimpleLithology:2008:anthropogenic_unconsolidated_material"/>
		<skos:hasTopConcept rdf:resource="urn:cgi:classifier:CGI:SimpleLithology:2008:rock"/>
		<skos:hasTopConcept
			rdf:resource="urn:cgi:classifier:CGI:SimpleLithology:2008:igneous_material"/>
		<skos:hasTopConcept
			rdf:resource="urn:cgi:classifier:CGI:SimpleLithology:2008:anthropogenic_material"/>
		<rdfs:isDefinedBy>
			ASTM, 2002, Annual Book of ASTM Standards, Petroleum Products, Lubricants, and Fossil Fuels: American Society of Testing Materials, 522 p.
			CGI Simple Lithology vocabulary, in review 2008, Draft vocabularies for GeoSciML Web services. Available at https://www.seegrid.csiro.au/twiki/bin/view/CGIModel/ConceptDefinitionsTG
			Dunham, R. J., 1962, Classification of carbonate rocks according to depositional texture. In: Ham, W. E. (ed.), Classification of carbonate rocks: American Association of Petroleum Geologists Memoir, p. 108-121.
			Taylor, Graham, and Eggleton, R.A., 2001, Regolith Geology and Geomorphology: Nature and Process: New York, John Wiley and Sons, 375 p.
			Fettes, Douglas, and Desmons, Jacqueline, eds.,  2007 Metamorphic Rocks: A Classification and Glossary of Terms , Cambridge University Press, Cambridge, UK,. ISBN 13.9780521868105.
			Flint, R.F., Sanders, J.E., and Rodgers, J., 1960. Diamictite, a substitute term for symmictite: Geological Society of America Bulletin, vol. 71, p. 1809.
			Folk, R. L., 1954, The distinction between grain size and mineral composition in sedimentary-rock nomenclature: Journal of Geology, v. 62, p. 344-359
			Folk, R. L., 1968, Petrology of sedimentary rocks: Austin, Texas, Hemphill’s Bookstore, 170 p
			Folk, R.L., 1980, Petrology of sedimentary rocks:  Austin, Texas, Hemphill’s Bookstore, 170 p.
			Gillespie, M. R., and Styles, M. T., 1999, BGS Rock Classification Scheme, Volume 1, Classification of igneous rocks: British Geological Survey Research Report, (2nd edition), RR 99–06.
			Hallsworth, C. R., and Knox, R. W. O’B., 1999, Classification of sediments and sedimentary rocks: v. 3 of the BGS rock classification scheme: British Geological Survey Research Report Number RR 99-03, 44 p.
			Jackson, J. A., 1997, Glossary of geology, 4th ed.: Alexandria, Virginia, American Geological Institute, 769 p.
			LeMaitre, R. W. (ed.), Streckiesen, A., Zanettin, B., LeBas, M.J., Bonin, B., Bateman, P., Bellieni, G., Dudek, A., Efremova, S., Keller, J., Lameyre, J., Sabine, P. A., Schmid, R., Sorensen, H., and Woolley, A. R., 2002, Igneous Rocks, A classification and Glossary of terms: Cambridge, U.K., Cambridge University Press, 236 p.
			Marshak, S., and Mitra, G., 1988. Basic Methods of Structural Geology: Englewood Cliffs (Prentice-Hall).
			McMillan, A.A., and Powell, J.H., 1999, BGS Rock Classification Scheme Volume 4--Classification of artificial (man-made) ground and natural superficial deposits applications to geological maps and datasets in the UK: Keyworth, UK, British Geological Survey Research Report, RR 99–04.
			North American Geologic Map Data Model Steering Committee Science Language Technical Team (SLTT), 2004, Report on Progress to Develop a North American Science-Language Standard for Digital Geologic-Map Databases, in D.R. Soller, ed., Digital Mapping Techniques '04— Workshop Proceedings: U.S. Geological Survey Open-File Report 2004–1451, accessed at http://pubs.usgs.gov/of/2004/1451/nadm/ (includes all science language documents).
			North American Geologic Map Data Model Steering Committee (NADMC1), 2004, NADM Conceptual Model 1.0, A Conceptual Model For Geologic Map Information: Geological Survey Of Canada, Open File 4737, 1 CD-Rom, U.S. Geological Survey Open-File Report 2004-1334, 58 p., accessed at Http://Pubs.Usgs.Gov/Of/2004/1334.
			North American Geologic-map Data Model Science Language Technical Team (NADM SLTTs), 2004a, Sedimentary materials: science language for their classification, description, and interpretation in digital geologic-map databases, Version 1.0 (12/18/2004): U.S. Geological Survey Open-File Report 2004–1451 appendix C, 595 p., accessed at http://pubs.usgs.gov/of/2004/1451/nadm/.
			North American Geologic-map Data Model Science Language Technical Team (NADM SLTTm), 2004b, Classification of metamorphic and other composite-genesis rocks, including hydrothermally altered, impact-metamorphic, mylonitic, and cataclastic rocks, Version 1.0 (12/18/2004): U.S. Geological Survey Open-File Report 2004–1451 appendix B, 56 p., accessed at http://pubs.usgs.gov/of/2004/1451/nadm/.
			Neuendorf, K.K.E., Mehl Jr., J.P., and Jackson, J.A., Eds., 2005, Glossary of Geology, Fifth Edition: Alexandria, VA, American Geological Institute, 779 p.
			Pettijohn, F.J., Potter, P.E., and Siever, R., 1987, Sand and sandstone, Second Edition: New York, Springer-Verlag, 553 p., ISBN 0387963502, 9780387963501.
			Schmid, R., 1981. Descriptive nomenclature and classification of pyroclastic deposits and fragments: Recommendations of the International Union of Geological Sciences Subcommission on the Systematics of Igneous Rocks: Geology, Vol. 9, p. 41-43.
			Schopf, J.M., 1956, A definition of coal: Economic Geology, v. 51, p. 521-527.
			Soller, D. R., and Berg, T. M., 2003, The National Geologic Map Database: Overview and Progress, in Soller, David R., ed., Digital Mapping Techniques ‘03—Workshop Proceedings, U. S. Geological Survey Open-File Report 03-471, p. 57-78, accessed at http://pubs.usgs.gov/of/2003/of03-471/soller1/index.html .
			Stöffler, D., and Grieve, R.A.F., 2001, IUGS classification and nomenclature of impact metamorphic rocks:  Towards a final proposal [indexed as:  Towards a unified nomenclature of metamorphism:  IUGS classification and nomenclature of impact metamorphic rocks. A proposal on behalf of the IUGS Subcommission on the Systematics of Metamorphic Rocks, Web version of 14.01.2001]:  3 p., available online at http://www.bgs.ac.uk/SCMR
			Streckeisen, A., 1976, To each plutonic rock its proper name: Earth Science Reviews, Vol. 12, 1–33.
		</rdfs:isDefinedBy>
	</skos:ConceptScheme>
	<skos:Concept rdf:about="urn:cgi:classifier:CGI:SimpleLithology:2008:acidic_igneous_material">
		<skos:inScheme rdf:resource="urn:cgi:classifierScheme:CGI:SimpleLithology:2008"/>
		<skos:definition>Igneous material with more than 63 percent SiO2.</skos:definition>
		<skos:prefLabel xml:lang="fr">matériel igné acide</skos:prefLabel>
		<skos:prefLabel xml:lang="it">materiale igneo acido</skos:prefLabel>
		<skos:prefLabel xml:lang="en">Acidic igneous material</skos:prefLabel>
		<skos:inScheme rdf:resource="urn:cgi:classifierScheme:CGI:SimpleLithology:2008"/>
		<skos:broader rdf:resource="urn:cgi:classifier:CGI:SimpleLithology:2008:igneous_material"/>
		<rdfs:isDefinedBy>after LeMaitre et al. 2002</rdfs:isDefinedBy>
		<skos:related rdf:resource="urn:cgi:classifier:CGI:GeneticCategory:2008:igneous_genesis"/>
	</skos:Concept>
	<skos:Concept rdf:about="urn:cgi:classifier:CGI:SimpleLithology:2008:acidic_igneous_rock">
		<skos:inScheme rdf:resource="urn:cgi:classifierScheme:CGI:SimpleLithology:2008"/>
		<skos:definition>Igneous rock with more than 63 percent SiO2.</skos:definition>
		<skos:prefLabel xml:lang="fr">roche ignée acide</skos:prefLabel>
		<skos:prefLabel xml:lang="it">roccia ignea acida</skos:prefLabel>
		<skos:prefLabel xml:lang="en">acidic igneous rock</skos:prefLabel>
		<skos:inScheme rdf:resource="urn:cgi:classifierScheme:CGI:SimpleLithology:2008"/>
		<skos:broader rdf:resource="urn:cgi:classifier:CGI:SimpleLithology:2008:igneous_rock"/>
		<rdfs:isDefinedBy>after LeMaitre et al. 2002</rdfs:isDefinedBy>
		<skos:related rdf:resource="urn:cgi:classifier:CGI:GeneticCategory:2008:igneous_genesis"/>
	</skos:Concept>
	<skos:Concept rdf:about="urn:cgi:classifier:CGI:SimpleLithology:2008:amphibolite">
		<skos:inScheme rdf:resource="urn:cgi:classifierScheme:CGI:SimpleLithology:2008"/>
		<skos:definition>Metamorphic rock mainly consisting of green, brown or black amphibole and plagioclase (including albite), which combined form 75 percent or more of the rock, and both of which are present as major constituents. The amphibole constitutes 50 percent or more of the total mafic constituents and is present in an amount of 30 percent or more; other common minerals include quartz, clinopyroxene, garnet, epidote-group minerals, biotite, titanite and scapolite.</skos:definition>
		<skos:editorialNote>I guess we're stuck with the 'green, brown, or black amphibole', but does  'dark-colored amphibole' capture the concept better.</skos:editorialNote>
		<skos:prefLabel xml:lang="fr">amphibolites</skos:prefLabel>
		<skos:prefLabel xml:lang="it">anfibolite</skos:prefLabel>
		<skos:prefLabel xml:lang="en">amphibolite</skos:prefLabel>
		<skos:inScheme rdf:resource="urn:cgi:classifierScheme:CGI:SimpleLithology:2008"/>
		<skos:broader rdf:resource="urn:cgi:classifier:CGI:SimpleLithology:2008:metamorphic_rock"/>
		<rdfs:isDefinedBy>Coutinho et al. 2007, IUGS SCMR chapter 8 (http://www.bgs.ac.uk/SCMR/)</rdfs:isDefinedBy>
		<skos:related rdf:resource="urn:cgi:classifier:CGI:GeneticCategory:2008:metamorphic_genesis"
		/>
	</skos:Concept>
	<skos:Concept rdf:about="urn:cgi:classifier:CGI:SimpleLithology:2008:andesitic_rock">
		<skos:inScheme rdf:resource="urn:cgi:classifierScheme:CGI:SimpleLithology:2008"/>
		<skos:definition>Fine grained crystalline rock, usually porphyritic, consisting of plagioclase (frequently zoned from labradorite to oligoclase), pyroxene, hornblende and/or biotite; color index M less than 35. Includes rocks defined modally in QAPF fields 9 and 10 or chemically in TAS field O2 as andesite. Fine grained equivalent of dioritic rock.</skos:definition>
		<skos:prefLabel xml:lang="fr">andésites</skos:prefLabel>
		<skos:prefLabel xml:lang="it">andesite</skos:prefLabel>
		<skos:prefLabel xml:lang="en">andesitic rock</skos:prefLabel>
		<skos:inScheme rdf:resource="urn:cgi:classifierScheme:CGI:SimpleLithology:2008"/>
		<skos:broader
			rdf:resource="urn:cgi:classifier:CGI:SimpleLithology:2008:fine_grained_igneous_rock"/>
		<rdfs:isDefinedBy>after LeMaitre et al. 2002</rdfs:isDefinedBy>
		<skos:related
			rdf:resource="urn:cgi:classifier:CGI:GeneticCategory:2008:igneous_extrusive_genesis"/>
	</skos:Concept>
	<skos:Concept rdf:about="urn:cgi:classifier:CGI:SimpleLithology:2008:anorthositic_rock">
		<skos:inScheme rdf:resource="urn:cgi:classifierScheme:CGI:SimpleLithology:2008"/>
		<skos:definition>General term for a leucocratic phaneritic crystalline rock consisting essentially of plagioclase, often with small amounts of pyroxene; colour index M less than 10. Includes rocks defined modally in QAPF field 10 as anorthosite. </skos:definition>
		<skos:prefLabel xml:lang="fr">anorthosite</skos:prefLabel>
		<skos:prefLabel xml:lang="it">anortosite</skos:prefLabel>
		<skos:prefLabel xml:lang="en">anorthositic rock</skos:prefLabel>
		<skos:inScheme rdf:resource="urn:cgi:classifierScheme:CGI:SimpleLithology:2008"/>
		<skos:broader
			rdf:resource="urn:cgi:classifier:CGI:SimpleLithology:2008:phaneritic_igneous_rock"/>
		<rdfs:isDefinedBy>after LeMaitre et al. 2002</rdfs:isDefinedBy>
		<skos:related
			rdf:resource="urn:cgi:classifier:CGI:GeneticCategory:2008:igneous_intrusive_genesis"/>
		<skos:editorialNote> **** Incomplete from here on down ****</skos:editorialNote>

	</skos:Concept>
	<skos:Concept rdf:about="urn:cgi:classifier:CGI:SimpleLithology:2008:anthropogenic_material">
		<skos:inScheme rdf:resource="urn:cgi:classifierScheme:CGI:SimpleLithology:2008"/>
		<skos:definition>Material known to have artificial (human-related) origin; insufficient information to classify in more detail. (CGI concepts task group)</skos:definition>
		<skos:prefLabel xml:lang="fr">matériel anthropique</skos:prefLabel>
		<skos:prefLabel xml:lang="it">materiale antropico</skos:prefLabel>
		<skos:prefLabel xml:lang="en">anthropogenic material</skos:prefLabel>
		<skos:inScheme rdf:resource="urn:cgi:classifierScheme:CGI:SimpleLithology:2008"/>
		<skos:broader rdf:resource="urn:cgi:classifier:CGI:SimpleLithology:2008:compound_material"/>
	</skos:Concept>
	<skos:Concept
		rdf:about="urn:cgi:classifier:CGI:SimpleLithology:2008:anthropogenic_unconsolidated_material">
		<skos:inScheme rdf:resource="urn:cgi:classifierScheme:CGI:SimpleLithology:2008"/>
		<skos:definition>Unconsolidated material known to have artificial (human-related) origin. (NGMDB 2008)</skos:definition>
		<skos:prefLabel xml:lang="fr">marériel anthropique non consolidé</skos:prefLabel>
		<skos:prefLabel xml:lang="it">materiale antropico non consolidato</skos:prefLabel>
		<skos:prefLabel xml:lang="en">anthropogenic unconsolidated material</skos:prefLabel>
		<skos:inScheme rdf:resource="urn:cgi:classifierScheme:CGI:SimpleLithology:2008"/>
		<skos:broader
			rdf:resource="urn:cgi:classifier:CGI:SimpleLithology:2008:unconsolidated_material"/>
	</skos:Concept>
	<skos:Concept rdf:about="urn:cgi:classifier:CGI:SimpleLithology:2008:aphanite">
		<skos:inScheme rdf:resource="urn:cgi:classifierScheme:CGI:SimpleLithology:2008"/>
		<skos:definition>Rock that is too fine grained to categorize in more detail. (NGMDB 2008)</skos:definition>
		<skos:prefLabel xml:lang="fr">roche aphanitique</skos:prefLabel>
		<skos:prefLabel xml:lang="it">roccia afanitica</skos:prefLabel>
		<skos:prefLabel xml:lang="en">aphanite</skos:prefLabel>
		<skos:inScheme rdf:resource="urn:cgi:classifierScheme:CGI:SimpleLithology:2008"/>
		<skos:broader rdf:resource="urn:cgi:classifier:CGI:SimpleLithology:2008:rock"/>
	</skos:Concept>
	<skos:Concept rdf:about="urn:cgi:classifier:CGI:SimpleLithology:2008:aplite">
		<skos:inScheme rdf:resource="urn:cgi:classifierScheme:CGI:SimpleLithology:2008"/>
		<skos:definition>Light coloured crystalline rock, characterized by a fine grained allotriomorphic-granular (aplitic, saccharoidal or xenomorphic) texture; typically granitic composition, consisting of quartz, K-feldspar and sodic plagioclase. (Neuendorf et al. 2005)</skos:definition>
		<skos:prefLabel xml:lang="fr">aplite</skos:prefLabel>
		<skos:prefLabel xml:lang="it">aplite</skos:prefLabel>
		<skos:prefLabel xml:lang="en">aplite</skos:prefLabel>
		<skos:inScheme rdf:resource="urn:cgi:classifierScheme:CGI:SimpleLithology:2008"/>
		<skos:broader
			rdf:resource="urn:cgi:classifier:CGI:SimpleLithology:2008:phaneritic_igneous_rock"/>
	</skos:Concept>
	<skos:Concept rdf:about="urn:cgi:classifier:CGI:SimpleLithology:2008:ash_and_lapilli">
		<skos:inScheme rdf:resource="urn:cgi:classifierScheme:CGI:SimpleLithology:2008"/>
		<skos:definition>Tephra in which less than 25 percent of fragments are greater than 64 mm in longest dimension (Schmid 1981; LeMaitre et al. 2002)</skos:definition>
		<skos:prefLabel xml:lang="fr">cendre et lapilli</skos:prefLabel>
		<skos:prefLabel xml:lang="it">cenere e lapilli</skos:prefLabel>
		<skos:prefLabel xml:lang="en">Ash and lapilli</skos:prefLabel>
		<skos:inScheme rdf:resource="urn:cgi:classifierScheme:CGI:SimpleLithology:2008"/>
		<skos:broader rdf:resource="urn:cgi:classifier:CGI:SimpleLithology:2008:tephra"/>
	</skos:Concept>
	<skos:Concept
		rdf:about="urn:cgi:classifier:CGI:SimpleLithology:2008:ash_breccia_bomb_or_block_tephra">
		<skos:inScheme rdf:resource="urn:cgi:classifierScheme:CGI:SimpleLithology:2008"/>
		<skos:definition>Tephra in which more than 25 percent of particles are greater than 64 mm in largest dimension. Includes ash breccia, bomb tephra and block tephra of Gillespie and Styles (1999) (Schmid 1981; LeMaitre et al. 2002)</skos:definition>
		<skos:prefLabel xml:lang="fr"
			>brèche cendreuse , bombe, ou bloques de téphra</skos:prefLabel>
		<skos:prefLabel xml:lang="it"
			>tephra a brecce cineritiche, a bombe vulcaniche, a
						blocchi</skos:prefLabel>
		<skos:prefLabel xml:lang="en">Ash breccia, bomb, or block tephra</skos:prefLabel>
		<skos:inScheme rdf:resource="urn:cgi:classifierScheme:CGI:SimpleLithology:2008"/>
		<skos:broader rdf:resource="urn:cgi:classifier:CGI:SimpleLithology:2008:tephra"/>
	</skos:Concept>
	<skos:Concept
		rdf:about="urn:cgi:classifier:CGI:SimpleLithology:2008:ash_tuff_lapillistone_and_lapilli_tuff">
		<skos:inScheme rdf:resource="urn:cgi:classifierScheme:CGI:SimpleLithology:2008"/>
		<skos:definition>Pyroclastic rock in which less than 25 percent of rock by volume are more than 64 mm in longest diameter. Includes tuff, lapilli tuff, and lapillistone. (Schmid 1981; LeMaitre et al. 2002)</skos:definition>
		<skos:prefLabel xml:lang="fr">cendre tuffacé, lapilli, et tuf lapillitique</skos:prefLabel>
		<skos:prefLabel xml:lang="it">tufo cineritico, tufo a lapilli</skos:prefLabel>
		<skos:prefLabel xml:lang="en">Ash tuff, lapillistone, and lapilli tuff</skos:prefLabel>
		<skos:inScheme rdf:resource="urn:cgi:classifierScheme:CGI:SimpleLithology:2008"/>
		<skos:broader rdf:resource="urn:cgi:classifier:CGI:SimpleLithology:2008:pyroclastic_rock"/>
	</skos:Concept>
	<skos:Concept rdf:about="urn:cgi:classifier:CGI:SimpleLithology:2008:basaltic_rock">
		<skos:inScheme rdf:resource="urn:cgi:classifierScheme:CGI:SimpleLithology:2008"/>
		<skos:definition>Fine-grained or porphyritic igneous rock with less than 20 percent quartz, and less than 10 percent feldspathoid minerals, in which the ratio of plagioclase to alkali feldspar is greater than 66 percent, and the color index is greater than 35. Typically composed of calcic plagioclase and clinopyroxene; phenocrysts typically include one or more of calcic plagioclase, clinopyroxene, orthopyroxene, and olivine. Includes rocks defined modally in QAPF fields 9 and 10 or chemically in TAS field B as basalt. (after LeMaitre et al. 2002)</skos:definition>
		<skos:prefLabel xml:lang="fr">basaltes</skos:prefLabel>
		<skos:prefLabel xml:lang="it">basalto</skos:prefLabel>
		<skos:prefLabel xml:lang="en">basaltic rock</skos:prefLabel>
		<skos:inScheme rdf:resource="urn:cgi:classifierScheme:CGI:SimpleLithology:2008"/>
		<skos:broader
			rdf:resource="urn:cgi:classifier:CGI:SimpleLithology:2008:fine_grained_igneous_rock"/>
	</skos:Concept>
	<skos:Concept rdf:about="urn:cgi:classifier:CGI:SimpleLithology:2008:basic_igneous_material">
		<skos:inScheme rdf:resource="urn:cgi:classifierScheme:CGI:SimpleLithology:2008"/>
		<skos:definition>Igneous material with between 45 and 52 percent SiO2. (after LeMaitre et al. 2002)</skos:definition>
		<skos:prefLabel xml:lang="fr">matériel igné basique</skos:prefLabel>
		<skos:prefLabel xml:lang="it">materiale igneo basico</skos:prefLabel>
		<skos:prefLabel xml:lang="en">basic igneous material</skos:prefLabel>
		<skos:inScheme rdf:resource="urn:cgi:classifierScheme:CGI:SimpleLithology:2008"/>
		<skos:broader rdf:resource="urn:cgi:classifier:CGI:SimpleLithology:2008:igneous_material"/>
	</skos:Concept>
	<skos:Concept rdf:about="urn:cgi:classifier:CGI:SimpleLithology:2008:basic_igneous_rock">
		<skos:inScheme rdf:resource="urn:cgi:classifierScheme:CGI:SimpleLithology:2008"/>
		<skos:definition>Igneous rock with between 45 and 52 percent SiO2. (after LeMaitre et al. 2002)</skos:definition>
		<skos:prefLabel xml:lang="fr">roche ignée basique</skos:prefLabel>
		<skos:prefLabel xml:lang="it">roccia ignea basica</skos:prefLabel>
		<skos:prefLabel xml:lang="en">basic igneous rock</skos:prefLabel>
		<skos:inScheme rdf:resource="urn:cgi:classifierScheme:CGI:SimpleLithology:2008"/>
		<skos:broader rdf:resource="urn:cgi:classifier:CGI:SimpleLithology:2008:igneous_rock"/>
	</skos:Concept>
	<skos:Concept rdf:about="urn:cgi:classifier:CGI:SimpleLithology:2008:bauxite">
		<skos:inScheme rdf:resource="urn:cgi:classifierScheme:CGI:SimpleLithology:2008"/>
		<skos:definition>Highly aluminous material containing abundant aluminium hydroxides (gibbsite, less commonly boehmite, diaspore) and aluminium-substituted iron oxides or hydroxides and generally minor or negligible kaolin minerals; may contain up to 20 percent quartz. Commonly has a pisolitic or nodular texture, and may be cemented. (Eggleton, 2001)</skos:definition>
		<skos:prefLabel xml:lang="fr">bauxite</skos:prefLabel>
		<skos:prefLabel xml:lang="it">bauxite</skos:prefLabel>
		<skos:prefLabel xml:lang="en">bauxite</skos:prefLabel>
		<skos:inScheme rdf:resource="urn:cgi:classifierScheme:CGI:SimpleLithology:2008"/>
		<skos:broader rdf:resource="urn:cgi:classifier:CGI:SimpleLithology:2008:compound_material"/>
	</skos:Concept>
	<skos:Concept rdf:about="urn:cgi:classifier:CGI:SimpleLithology:2008:biogenic_sediment">
		<skos:inScheme rdf:resource="urn:cgi:classifierScheme:CGI:SimpleLithology:2008"/>
		<skos:definition>Sediment composed of greater than 50 percent material of biogenic origin. (NGMDB 2008)</skos:definition>
		<skos:prefLabel xml:lang="fr">sédiment biogénique</skos:prefLabel>
		<skos:prefLabel xml:lang="it">sedimento biogenico</skos:prefLabel>
		<skos:prefLabel xml:lang="en">biogenic sediment</skos:prefLabel>
		<skos:inScheme rdf:resource="urn:cgi:classifierScheme:CGI:SimpleLithology:2008"/>
		<skos:broader rdf:resource="urn:cgi:classifier:CGI:SimpleLithology:2008:sediment"/>
	</skos:Concept>
	<skos:Concept
		rdf:about="urn:cgi:classifier:CGI:SimpleLithology:2008:biogenic_silica_sedimentary_rock">
		<skos:inScheme rdf:resource="urn:cgi:classifierScheme:CGI:SimpleLithology:2008"/>
		<skos:definition>Sedimentary rock that consists of at least 50 percent silicate mineral material, deposited directly by biological processes at the depositional surface, or in particles formed by biological processes within the basin of deposition. (based on NADM SLTT sedimentary; Hallsworth and Knox 1999)</skos:definition>
		<skos:prefLabel xml:lang="fr">roche sédimentaire siliceuse biogénique</skos:prefLabel>
		<skos:prefLabel xml:lang="it">roccia sedimentaria biogenica silicea</skos:prefLabel>
		<skos:prefLabel xml:lang="en">biogenic silica sedimentary rock</skos:prefLabel>
		<skos:inScheme rdf:resource="urn:cgi:classifierScheme:CGI:SimpleLithology:2008"/>
		<skos:broader
			rdf:resource="urn:cgi:classifier:CGI:SimpleLithology:2008:non_clastic_siliceous_sedimentary_rock"
		/>
	</skos:Concept>
	<skos:Concept rdf:about="urn:cgi:classifier:CGI:SimpleLithology:2008:boundstone">
		<skos:inScheme rdf:resource="urn:cgi:classifierScheme:CGI:SimpleLithology:2008"/>
		<skos:definition>Sedimentary carbonate rock with preserved biogenic texture, whose original components were bound and encrusted together during deposition by the action of plants and animals during deposition, and remained substantially in the position of growth. (Hallsworth and Knox 1999; SLTTs 2004)</skos:definition>
		<skos:prefLabel xml:lang="fr">boundstone</skos:prefLabel>
		<skos:prefLabel xml:lang="it">boundstone</skos:prefLabel>
		<skos:prefLabel xml:lang="en">boundstone</skos:prefLabel>
		<skos:inScheme rdf:resource="urn:cgi:classifierScheme:CGI:SimpleLithology:2008"/>
		<skos:broader
			rdf:resource="urn:cgi:classifier:CGI:SimpleLithology:2008:carbonate_sedimentary_rock"/>
	</skos:Concept>
	<skos:Concept rdf:about="urn:cgi:classifier:CGI:SimpleLithology:2008:breccia">
		<skos:inScheme rdf:resource="urn:cgi:classifierScheme:CGI:SimpleLithology:2008"/>
		<skos:definition>Coarse-grained material composed of angular broken rock fragments; the fragments typically have sharp edges and unworn corners. The fragments may be held together by a mineral cement, or in a fine-grained matrix. Clasts may be of any composition or origin. (Neuendorf et al. 2005)</skos:definition>
		<skos:prefLabel xml:lang="fr">brèches</skos:prefLabel>
		<skos:prefLabel xml:lang="it">breccia</skos:prefLabel>
		<skos:prefLabel xml:lang="en">breccia</skos:prefLabel>
		<skos:inScheme rdf:resource="urn:cgi:classifierScheme:CGI:SimpleLithology:2008"/>
		<skos:broader rdf:resource="urn:cgi:classifier:CGI:SimpleLithology:2008:compound_material"/>
	</skos:Concept>
	<skos:Concept rdf:about="urn:cgi:classifier:CGI:SimpleLithology:2008:breccia_gouge_series">
		<skos:inScheme rdf:resource="urn:cgi:classifierScheme:CGI:SimpleLithology:2008"/>
		<skos:definition>Fault material with features such as void spaces (filled or unfilled), or unconsolidated matrix material between fragments, indicating loss of cohesion during deformation. Includes fault-related breccia and gouge. (NGMDB 2008)</skos:definition>
		<skos:prefLabel xml:lang="fr">brèche de faille</skos:prefLabel>
		<skos:prefLabel xml:lang="it">breccia di faglia</skos:prefLabel>
		<skos:prefLabel xml:lang="en">breccia-gouge series</skos:prefLabel>
		<skos:inScheme rdf:resource="urn:cgi:classifierScheme:CGI:SimpleLithology:2008"/>
		<skos:broader
			rdf:resource="urn:cgi:classifier:CGI:SimpleLithology:2008:fault_related_material"/>
	</skos:Concept>
	<skos:Concept
		rdf:about="urn:cgi:classifier:CGI:SimpleLithology:2008:calcareous_carbonate_sediment">
		<skos:inScheme rdf:resource="urn:cgi:classifierScheme:CGI:SimpleLithology:2008"/>
		<skos:definition>Carbonate sediment with a calcite (plus aragonite) to dolomite ratio greater than 1 to 1. Includes lime-sediments. (after Hallsworth and Knox 1999)</skos:definition>
		<skos:prefLabel xml:lang="fr">sédiment carbonaté calcaire</skos:prefLabel>
		<skos:prefLabel xml:lang="it">sedimento calcareo carbonatico</skos:prefLabel>
		<skos:prefLabel xml:lang="en">calcareous carbonate sediment</skos:prefLabel>
		<skos:inScheme rdf:resource="urn:cgi:classifierScheme:CGI:SimpleLithology:2008"/>
		<skos:broader rdf:resource="urn:cgi:classifier:CGI:SimpleLithology:2008:carbonate_sediment"
		/>
	</skos:Concept>
	<skos:Concept
		rdf:about="urn:cgi:classifier:CGI:SimpleLithology:2008:calcareous_carbonate_sedimentary_material">
		<skos:inScheme rdf:resource="urn:cgi:classifierScheme:CGI:SimpleLithology:2008"/>
		<skos:definition>Carbonate sedimentary material of unspecified consolidation state with a calcite (plus aragonite) to dolomite ratio greater than 1 to 1. Includes lime-sediments, limestone and dolomitic limestone. (after Hallsworth and Knox 1999)</skos:definition>
		<skos:prefLabel xml:lang="fr">matériel sédimentaire carbonaté calcaire</skos:prefLabel>
		<skos:prefLabel xml:lang="it">materiale sedimentario calcareo carbonatico</skos:prefLabel>
		<skos:prefLabel xml:lang="en">calcareous carbonate sedimentary material</skos:prefLabel>
		<skos:inScheme rdf:resource="urn:cgi:classifierScheme:CGI:SimpleLithology:2008"/>
		<skos:broader
			rdf:resource="urn:cgi:classifier:CGI:SimpleLithology:2008:carbonate_sedimentary_material"
		/>
	</skos:Concept>
	<skos:Concept
		rdf:about="urn:cgi:classifier:CGI:SimpleLithology:2008:calcareous_carbonate_sedimentary_rock">
		<skos:inScheme rdf:resource="urn:cgi:classifierScheme:CGI:SimpleLithology:2008"/>
		<skos:definition>Carbonate sedimentary rock with a calcite (plus aragonite) to dolomite ratio greater than 1 to 1. Includes limestone and dolomitic limestone. (NADM SLTT sedimentary; Hallsworth and Knox 1999)</skos:definition>
		<skos:prefLabel xml:lang="fr">calcaires</skos:prefLabel>
		<skos:prefLabel xml:lang="it">calcare</skos:prefLabel>
		<skos:prefLabel xml:lang="en">calcareous carbonate sedimentary rock</skos:prefLabel>
		<skos:inScheme rdf:resource="urn:cgi:classifierScheme:CGI:SimpleLithology:2008"/>
		<skos:broader
			rdf:resource="urn:cgi:classifier:CGI:SimpleLithology:2008:carbonate_sedimentary_rock"/>
	</skos:Concept>
	<skos:Concept rdf:about="urn:cgi:classifier:CGI:SimpleLithology:2008:carbonate_gravel">
		<skos:inScheme rdf:resource="urn:cgi:classifierScheme:CGI:SimpleLithology:2008"/>
		<skos:definition>Carbonate sediment composed of more than 25 percent gravel-sized clasts (maximum diameter more than 2 mm). (Hallsworth and Knox 1999)</skos:definition>
		<skos:prefLabel xml:lang="fr">gravier carbonaté</skos:prefLabel>
		<skos:prefLabel xml:lang="it">ghiaia calcarea</skos:prefLabel>
		<skos:prefLabel xml:lang="en">carbonate gravel</skos:prefLabel>
		<skos:inScheme rdf:resource="urn:cgi:classifierScheme:CGI:SimpleLithology:2008"/>
		<skos:broader rdf:resource="urn:cgi:classifier:CGI:SimpleLithology:2008:carbonate_sediment"
		/>
	</skos:Concept>
	<skos:Concept rdf:about="urn:cgi:classifier:CGI:SimpleLithology:2008:carbonate_mud">
		<skos:inScheme rdf:resource="urn:cgi:classifierScheme:CGI:SimpleLithology:2008"/>
		<skos:definition>Carbonate sediment composed of more than 75 percent mud-sized clasts (maximum diameter less than 32 microns). (Hallsworth and Knox 1999)</skos:definition>
		<skos:prefLabel xml:lang="fr">boue carbonatée</skos:prefLabel>
		<skos:prefLabel xml:lang="it">fango calcareo</skos:prefLabel>
		<skos:prefLabel xml:lang="en">carbonate mud</skos:prefLabel>
		<skos:inScheme rdf:resource="urn:cgi:classifierScheme:CGI:SimpleLithology:2008"/>
		<skos:broader rdf:resource="urn:cgi:classifier:CGI:SimpleLithology:2008:carbonate_sediment"
		/>
	</skos:Concept>
	<skos:Concept rdf:about="urn:cgi:classifier:CGI:SimpleLithology:2008:carbonate_mudstone">
		<skos:inScheme rdf:resource="urn:cgi:classifierScheme:CGI:SimpleLithology:2008"/>
		<skos:definition>Carbonate sedimentary rock with matrix-supported fabric, composed of more than 75 percent mud-sized grains (maximum diameter less than 32 microns). The original depositional texture is preserved. (Hallsworth and Knox 1999; NADM SLTT sedimentary)</skos:definition>
		<skos:prefLabel xml:lang="fr">mudstone carbonatée</skos:prefLabel>
		<skos:prefLabel xml:lang="it">mudstone carbonatico</skos:prefLabel>
		<skos:prefLabel xml:lang="en">carbonate mudstone</skos:prefLabel>
		<skos:inScheme rdf:resource="urn:cgi:classifierScheme:CGI:SimpleLithology:2008"/>
		<skos:broader
			rdf:resource="urn:cgi:classifier:CGI:SimpleLithology:2008:carbonate_sedimentary_rock"/>
	</skos:Concept>
	<skos:Concept rdf:about="urn:cgi:classifier:CGI:SimpleLithology:2008:carbonate_sand">
		<skos:inScheme rdf:resource="urn:cgi:classifierScheme:CGI:SimpleLithology:2008"/>
		<skos:definition>Carbonate sediment composed of more than 75 percent sand-sized clasts (maximum diameter between 32 microns and 2 mm). (Hallsworth and Knox 1999)</skos:definition>
		<skos:prefLabel xml:lang="fr">sable carbonaté</skos:prefLabel>
		<skos:prefLabel xml:lang="it">sabbia calcarea</skos:prefLabel>
		<skos:prefLabel xml:lang="en">carbonate sand</skos:prefLabel>
		<skos:inScheme rdf:resource="urn:cgi:classifierScheme:CGI:SimpleLithology:2008"/>
		<skos:broader rdf:resource="urn:cgi:classifier:CGI:SimpleLithology:2008:carbonate_sediment"
		/>
	</skos:Concept>
	<skos:Concept rdf:about="urn:cgi:classifier:CGI:SimpleLithology:2008:carbonate_sediment">
		<skos:inScheme rdf:resource="urn:cgi:classifierScheme:CGI:SimpleLithology:2008"/>
		<skos:definition>Sediment in which at least 50 percent of the primary and/or recrystallized constituents are composed of one (or more) of the carbonate minerals calcite, aragonite and dolomite, in particles of intrabasinal origin. (after NADM SLTT sedimentary rocks)</skos:definition>
		<skos:prefLabel xml:lang="fr">sédiment carbonaté</skos:prefLabel>
		<skos:prefLabel xml:lang="it">sedimento carbonatico</skos:prefLabel>
		<skos:prefLabel xml:lang="en">carbonate sediment</skos:prefLabel>
		<skos:inScheme rdf:resource="urn:cgi:classifierScheme:CGI:SimpleLithology:2008"/>
		<skos:broader rdf:resource="urn:cgi:classifier:CGI:SimpleLithology:2008:sediment"/>
	</skos:Concept>
	<skos:Concept
		rdf:about="urn:cgi:classifier:CGI:SimpleLithology:2008:carbonate_sedimentary_material">
		<skos:inScheme rdf:resource="urn:cgi:classifierScheme:CGI:SimpleLithology:2008"/>
		<skos:definition>Sedimentary material in which at least 50 percent of the primary and/or recrystallized constituents are composed of one (or more) of the carbonate minerals calcite, aragonite and dolomite, in particles of intrabasinal origin. (after NADM SLTT sedimentary rocks)</skos:definition>
		<skos:prefLabel xml:lang="fr">matériel sédimentaire carbonaté </skos:prefLabel>
		<skos:prefLabel xml:lang="it">materiale sedimentario carbonatico</skos:prefLabel>
		<skos:prefLabel xml:lang="en">carbonate sedimentary material</skos:prefLabel>
		<skos:inScheme rdf:resource="urn:cgi:classifierScheme:CGI:SimpleLithology:2008"/>
		<skos:broader
			rdf:resource="urn:cgi:classifier:CGI:SimpleLithology:2008:sedimentary_material"/>
	</skos:Concept>
	<skos:Concept rdf:about="urn:cgi:classifier:CGI:SimpleLithology:2008:carbonate_sedimentary_rock">
		<skos:inScheme rdf:resource="urn:cgi:classifierScheme:CGI:SimpleLithology:2008"/>
		<skos:definition>Sedimentary rock in which at least 50 percent of the primary and/or recrystallized constituents are composed of one (or more) of the carbonate minerals calcite, aragonite and dolomite, in particles of intrabasinal origin. (after NADM SLTT sedimentary rocks)</skos:definition>
		<skos:prefLabel xml:lang="fr">roche sédimentaire carbonaté </skos:prefLabel>
		<skos:prefLabel xml:lang="it">roccia sedimentaria carbonatica</skos:prefLabel>
		<skos:prefLabel xml:lang="en">carbonate sedimentary rock</skos:prefLabel>
		<skos:inScheme rdf:resource="urn:cgi:classifierScheme:CGI:SimpleLithology:2008"/>
		<skos:broader rdf:resource="urn:cgi:classifier:CGI:SimpleLithology:2008:sedimentary_rock"/>
	</skos:Concept>
	<skos:Concept rdf:about="urn:cgi:classifier:CGI:SimpleLithology:2008:carbonate_wackestone">
		<skos:inScheme rdf:resource="urn:cgi:classifierScheme:CGI:SimpleLithology:2008"/>
		<skos:definition>Carbonate sedimentary rock with discernible mud supported depositional texture and containing greater than 10 percent grains. ()</skos:definition>
		<skos:prefLabel xml:lang="fr">calcaire wackestone</skos:prefLabel>
		<skos:prefLabel xml:lang="it">wackestone carbonatico</skos:prefLabel>
		<skos:prefLabel xml:lang="en">carbonate wackestone</skos:prefLabel>
		<skos:inScheme rdf:resource="urn:cgi:classifierScheme:CGI:SimpleLithology:2008"/>
		<skos:broader rdf:resource="urn:cgi:classifier:CGI:SimpleLithology:2008:sedimentary_rock"/>
	</skos:Concept>
	<skos:Concept rdf:about="urn:cgi:classifier:CGI:SimpleLithology:2008:carbonatite">
		<skos:inScheme rdf:resource="urn:cgi:classifierScheme:CGI:SimpleLithology:2008"/>
		<skos:definition>Igneous rock composed of more than 50 percent modal carbonate minerals. (LeMaitre et al. 2002)</skos:definition>
		<skos:prefLabel xml:lang="fr">carbonatite</skos:prefLabel>
		<skos:prefLabel xml:lang="it">carbonatite</skos:prefLabel>
		<skos:prefLabel xml:lang="en">carbonatite</skos:prefLabel>
		<skos:inScheme rdf:resource="urn:cgi:classifierScheme:CGI:SimpleLithology:2008"/>
		<skos:broader
			rdf:resource="urn:cgi:classifier:CGI:SimpleLithology:2008:exotic_composition_igneous_rock"
		/>
	</skos:Concept>
	<skos:Concept rdf:about="urn:cgi:classifier:CGI:SimpleLithology:2008:cataclasite_series">
		<skos:inScheme rdf:resource="urn:cgi:classifierScheme:CGI:SimpleLithology:2008"/>
		<skos:definition>Fault-related rock that maintained primary cohesion during deformation, with matrix comprising 50 to 90 percent of rock mass; matrix is fine-grained material caused by tectonic grainsize reduction. Includes cataclasite, protocataclasite and ultracataclasite. (Sibson, 1977; Scholz, 1990; Snoke and Tullis, 1998; Barker, 1998 Appendix II; NADM SLTTm, 2004)</skos:definition>
		<skos:prefLabel xml:lang="fr">cataclasites</skos:prefLabel>
		<skos:prefLabel xml:lang="it">cataclasite</skos:prefLabel>
		<skos:prefLabel xml:lang="en">cataclasite series</skos:prefLabel>
		<skos:inScheme rdf:resource="urn:cgi:classifierScheme:CGI:SimpleLithology:2008"/>
		<skos:broader
			rdf:resource="urn:cgi:classifier:CGI:SimpleLithology:2008:fault_related_material"/>
	</skos:Concept>
	<skos:Concept rdf:about="urn:cgi:classifier:CGI:SimpleLithology:2008:chemical_sediment">
		<skos:inScheme rdf:resource="urn:cgi:classifierScheme:CGI:SimpleLithology:2008"/>
		<skos:definition>Sediment that consists of at least 50 percent material produced by chemical (organic or inorganic) processes within the basin of deposition. Includes organic-rich, non-clastic siliceous, carbonate, evaporite, iron-rich, and phosphatic sediment classes. (NGMDB 2008)</skos:definition>
		<skos:prefLabel xml:lang="fr">sédiment chimique</skos:prefLabel>
		<skos:prefLabel xml:lang="it">sedimento chimico</skos:prefLabel>
		<skos:prefLabel xml:lang="en">chemical sediment</skos:prefLabel>
		<skos:inScheme rdf:resource="urn:cgi:classifierScheme:CGI:SimpleLithology:2008"/>
		<skos:broader rdf:resource="urn:cgi:classifier:CGI:SimpleLithology:2008:sediment"/>
	</skos:Concept>
	<skos:Concept rdf:about="urn:cgi:classifier:CGI:SimpleLithology:2008:clastic_sediment">
		<skos:inScheme rdf:resource="urn:cgi:classifierScheme:CGI:SimpleLithology:2008"/>
		<skos:definition>Sediment in which at least 50 percent of the constituent particles were derived from erosion, weathering, or mass-wasting of pre-existing earth materials, and transported to the place of deposition by mechanical agents such as water, wind, ice and gravity. (SLTTs, 2004; Neuendorf et al., 2005)</skos:definition>
		<skos:prefLabel xml:lang="fr">sédiment clastique</skos:prefLabel>
		<skos:prefLabel xml:lang="it">sedimento clastico</skos:prefLabel>
		<skos:prefLabel xml:lang="en">clastic sediment</skos:prefLabel>
		<skos:inScheme rdf:resource="urn:cgi:classifierScheme:CGI:SimpleLithology:2008"/>
		<skos:broader rdf:resource="urn:cgi:classifier:CGI:SimpleLithology:2008:sediment"/>
	</skos:Concept>
	<skos:Concept
		rdf:about="urn:cgi:classifier:CGI:SimpleLithology:2008:clastic_sedimentary_material">
		<skos:inScheme rdf:resource="urn:cgi:classifierScheme:CGI:SimpleLithology:2008"/>
		<skos:definition>Sedimentary material of unspecified consolidation state in which at least 50 percent of the constituent particles were derived from erosion, weathering, or mass-wasting of pre-existing earth materials, and transported to the place of deposition by mechanical agents such as water, wind, ice and gravity. (SLTTs, 2004; Neuendorf et al., 2005)</skos:definition>
		<skos:prefLabel xml:lang="fr">matériel sédimentaire clastique</skos:prefLabel>
		<skos:prefLabel xml:lang="it">materiale sedimentario clastico</skos:prefLabel>
		<skos:prefLabel xml:lang="en">clastic sedimentary material</skos:prefLabel>
		<skos:inScheme rdf:resource="urn:cgi:classifierScheme:CGI:SimpleLithology:2008"/>
		<skos:broader
			rdf:resource="urn:cgi:classifier:CGI:SimpleLithology:2008:sedimentary_material"/>
	</skos:Concept>
	<skos:Concept rdf:about="urn:cgi:classifier:CGI:SimpleLithology:2008:clastic_sedimentary_rock">
		<skos:inScheme rdf:resource="urn:cgi:classifierScheme:CGI:SimpleLithology:2008"/>
		<skos:definition>Sedimentary rock in which at least 50 percent of the constituent particles were derived from erosion, weathering, or mass-wasting of pre-existing earth materials, and transported to the place of deposition by mechanical agents such as water, wind, ice and gravity. (SLTTs, 2004; Neuendorf et al., 2005)</skos:definition>
		<skos:prefLabel xml:lang="fr">roche sédimentaire clastique</skos:prefLabel>
		<skos:prefLabel xml:lang="it">roccia detritica</skos:prefLabel>
		<skos:prefLabel xml:lang="en">clastic sedimentary rock</skos:prefLabel>
		<skos:inScheme rdf:resource="urn:cgi:classifierScheme:CGI:SimpleLithology:2008"/>
		<skos:broader rdf:resource="urn:cgi:classifier:CGI:SimpleLithology:2008:sedimentary_rock"/>
	</skos:Concept>
	<skos:Concept rdf:about="urn:cgi:classifier:CGI:SimpleLithology:2008:coal">
		<skos:inScheme rdf:resource="urn:cgi:classifierScheme:CGI:SimpleLithology:2008"/>
		<skos:definition>Hard, black, organic rich sedimentary rock that yields greater than 8,300 Btu on a moist, mineral-matter-free basis, or contains greater than 69 percent fixed carbon on a dry, mineral-matter-free basis; formed from the compaction or induration of variously altered plant remains similar to those of peaty deposits. (ASTM 2002; Schopf 1956)</skos:definition>
		<skos:prefLabel xml:lang="fr">charbons</skos:prefLabel>
		<skos:prefLabel xml:lang="it">carbone</skos:prefLabel>
		<skos:prefLabel xml:lang="en">coal</skos:prefLabel>
		<skos:inScheme rdf:resource="urn:cgi:classifierScheme:CGI:SimpleLithology:2008"/>
		<skos:broader
			rdf:resource="urn:cgi:classifier:CGI:SimpleLithology:2008:organic_rich_sedimentary_rock"
		/>
	</skos:Concept>
	<skos:Concept rdf:about="urn:cgi:classifier:CGI:SimpleLithology:2008:composite_genesis_material">
		<skos:inScheme rdf:resource="urn:cgi:classifierScheme:CGI:SimpleLithology:2008"/>
		<skos:definition>Material of unspecified consolidation state formed by geological modification of pre-existing materials outside the realm of igneous and sedimentary processes. Includes rocks formed by impact metamorphism, standard dynamothermal metamorphism, brittle deformation, weathering, metasomatism and hydrothermal alteration (diagenesis is a sedimentary process in this context). (NADM SLTT metamorphic)</skos:definition>
		<skos:prefLabel xml:lang="fr">matériel modifié et/ou transformé</skos:prefLabel>
		<skos:prefLabel xml:lang="it">materiale modificato o trasformato</skos:prefLabel>
		<skos:prefLabel xml:lang="en">composite (transformed) genesis material</skos:prefLabel>
		<skos:inScheme rdf:resource="urn:cgi:classifierScheme:CGI:SimpleLithology:2008"/>
		<skos:broader rdf:resource="urn:cgi:classifier:CGI:SimpleLithology:2008:compound_material"/>
	</skos:Concept>
	<skos:Concept rdf:about="urn:cgi:classifier:CGI:SimpleLithology:2008:composite_genesis_rock">
		<skos:inScheme rdf:resource="urn:cgi:classifierScheme:CGI:SimpleLithology:2008"/>
		<skos:definition>Rock formed by geological modification of pre-existing rocks outside the realm of igneous and sedimentary processes. Includes rocks formed by impact metamorphism, standard dynamothermal metamorphism, brittle deformation, weathering, metasomatism and hydrothermal alteration (diagenesis is a sedimentary process in this context). (NGMDB 2008)</skos:definition>
		<skos:prefLabel xml:lang="fr">roche modifiée et/ou transformée</skos:prefLabel>
		<skos:prefLabel xml:lang="it">roccia modificata o trasformata</skos:prefLabel>
		<skos:prefLabel xml:lang="en">composite (transformed) genesis rock</skos:prefLabel>
		<skos:inScheme rdf:resource="urn:cgi:classifierScheme:CGI:SimpleLithology:2008"/>
		<skos:broader rdf:resource="urn:cgi:classifier:CGI:SimpleLithology:2008:rock"/>
	</skos:Concept>
	<skos:Concept rdf:about="urn:cgi:classifier:CGI:SimpleLithology:2008:conglomerate">
		<skos:inScheme rdf:resource="urn:cgi:classifierScheme:CGI:SimpleLithology:2008"/>
		<skos:definition>Coarse grained sedimentary rock composed of at least 30 percent rounded to subangular fragments larger than 2 mm in diameter; typically contains finer grained material in interstices between larger fragments. (Neuendorf et al. 2005; NADM SLTT sedimentary)</skos:definition>
		<skos:prefLabel xml:lang="fr">conglomérats</skos:prefLabel>
		<skos:prefLabel xml:lang="it">conglomerato</skos:prefLabel>
		<skos:prefLabel xml:lang="en">conglomerate</skos:prefLabel>
		<skos:inScheme rdf:resource="urn:cgi:classifierScheme:CGI:SimpleLithology:2008"/>
		<skos:broader
			rdf:resource="urn:cgi:classifier:CGI:SimpleLithology:2008:clastic_sedimentary_rock"/>
	</skos:Concept>
	<skos:Concept rdf:about="urn:cgi:classifier:CGI:SimpleLithology:2008:crystalline_carbonate">
		<skos:inScheme rdf:resource="urn:cgi:classifierScheme:CGI:SimpleLithology:2008"/>
		<skos:definition>Carbonate rock of indeterminate mineralogy in which diagenetic processes have obliterated any original depositional texture. (NADM SLTTs 2004)</skos:definition>
		<skos:prefLabel xml:lang="fr">calcaire cristallin</skos:prefLabel>
		<skos:prefLabel xml:lang="it">calcare cristallino</skos:prefLabel>
		<skos:prefLabel xml:lang="en">crystalline carbonate</skos:prefLabel>
		<skos:inScheme rdf:resource="urn:cgi:classifierScheme:CGI:SimpleLithology:2008"/>
		<skos:broader
			rdf:resource="urn:cgi:classifier:CGI:SimpleLithology:2008:carbonate_sedimentary_rock"/>
	</skos:Concept>
	<skos:Concept rdf:about="urn:cgi:classifier:CGI:SimpleLithology:2008:dacitic_rock">
		<skos:inScheme rdf:resource="urn:cgi:classifierScheme:CGI:SimpleLithology:2008"/>
		<skos:definition>Fine grained or porphyritic crystalline rock composed of quartz and sodic plagioclase with minor amounts of biotite and/or hornblende and/or pyroxene; volcanic equivalent of granodiorite and tonalite. Includes rocks defined modally in QAPF fields 4 and 5 or chemically in TAS Field O3. (LeMaitre et al. 2002)</skos:definition>
		<skos:prefLabel xml:lang="fr">dacites</skos:prefLabel>
		<skos:prefLabel xml:lang="it">dacite</skos:prefLabel>
		<skos:prefLabel xml:lang="en">dacitic rock</skos:prefLabel>
		<skos:inScheme rdf:resource="urn:cgi:classifierScheme:CGI:SimpleLithology:2008"/>
		<skos:broader
			rdf:resource="urn:cgi:classifier:CGI:SimpleLithology:2008:fine_grained_igneous_rock"/>
	</skos:Concept>
	<skos:Concept rdf:about="urn:cgi:classifier:CGI:SimpleLithology:2008:diamictite">
		<skos:inScheme rdf:resource="urn:cgi:classifierScheme:CGI:SimpleLithology:2008"/>
		<skos:definition>Unsorted or poorly sorted, clastic sedimentary rock with a wide range of particle sizes such that it cannot be assigned to any other class. (Fairbridge and Bourgeois 1978)</skos:definition>
		<skos:prefLabel xml:lang="fr">tillite</skos:prefLabel>
		<skos:prefLabel xml:lang="it">diamictite</skos:prefLabel>
		<skos:prefLabel xml:lang="en">diamictite</skos:prefLabel>
		<skos:inScheme rdf:resource="urn:cgi:classifierScheme:CGI:SimpleLithology:2008"/>
		<skos:broader
			rdf:resource="urn:cgi:classifier:CGI:SimpleLithology:2008:clastic_sedimentary_rock"/>
	</skos:Concept>
	<skos:Concept rdf:about="urn:cgi:classifier:CGI:SimpleLithology:2008:diamicton">
		<skos:inScheme rdf:resource="urn:cgi:classifierScheme:CGI:SimpleLithology:2008"/>
		<skos:definition>Unsorted or poorly sorted, clastic sediment with a wide range of particle sizes such that it cannot be assigned to any other class. (Fairbridge and Bourgeois 1978)</skos:definition>
		<skos:prefLabel xml:lang="fr">diamictite</skos:prefLabel>
		<skos:prefLabel xml:lang="it">diamicton</skos:prefLabel>
		<skos:prefLabel xml:lang="en">diamicton</skos:prefLabel>
		<skos:inScheme rdf:resource="urn:cgi:classifierScheme:CGI:SimpleLithology:2008"/>
		<skos:broader rdf:resource="urn:cgi:classifier:CGI:SimpleLithology:2008:clastic_sediment"/>
	</skos:Concept>
	<skos:Concept rdf:about="urn:cgi:classifier:CGI:SimpleLithology:2008:diorite">
		<skos:inScheme rdf:resource="urn:cgi:classifierScheme:CGI:SimpleLithology:2008"/>
		<skos:definition>Phaneritic crystalline rock consisting of intermediate plagioclase, commonly with hornblende and often with biotite or augite; colour index M less than 90, sodic plagioclase (An0-An50). Includes rocks defined modally in QAPF field 10 as diorite. (LeMaitre et al. 2002)</skos:definition>
		<skos:prefLabel xml:lang="fr">diorites</skos:prefLabel>
		<skos:prefLabel xml:lang="it">diorite</skos:prefLabel>
		<skos:prefLabel xml:lang="en">diorite</skos:prefLabel>
		<skos:inScheme rdf:resource="urn:cgi:classifierScheme:CGI:SimpleLithology:2008"/>
		<skos:broader
			rdf:resource="urn:cgi:classifier:CGI:SimpleLithology:2008:phaneritic_igneous_rock"/>
	</skos:Concept>
	<skos:Concept rdf:about="urn:cgi:classifier:CGI:SimpleLithology:2008:dioritic_rock">
		<skos:inScheme rdf:resource="urn:cgi:classifierScheme:CGI:SimpleLithology:2008"/>
		<skos:definition>Phaneritic crystalline rock with M less than 90, consisting of intermediate plagioclase, commonly with hornblende and often with biotite or augite. Includes rocks defined modally in QAPF fields 9 and 10 as diorite, monzodiorite. (LeMaitre et al. 2002)</skos:definition>
		<skos:prefLabel xml:lang="fr">diorites</skos:prefLabel>
		<skos:prefLabel xml:lang="it">roccia dioritica</skos:prefLabel>
		<skos:prefLabel xml:lang="en">dioritic rock</skos:prefLabel>
		<skos:inScheme rdf:resource="urn:cgi:classifierScheme:CGI:SimpleLithology:2008"/>
		<skos:broader
			rdf:resource="urn:cgi:classifier:CGI:SimpleLithology:2008:phaneritic_igneous_rock"/>
	</skos:Concept>
	<skos:Concept rdf:about="urn:cgi:classifier:CGI:SimpleLithology:2008:doleritic_rock">
		<skos:inScheme rdf:resource="urn:cgi:classifierScheme:CGI:SimpleLithology:2008"/>
		<skos:definition>Dark colored gabbroic (basaltic) or dioritic (andesitic) rock intermediate in grain size between basalt and gabbro and composed of plagioclase, pyroxene and opaque minerals; often with ophitic texture. Typically occurs as hypabyssal intrusions. Includes dolerite, microdiorite, diabase and microgabbro. (Neuendorf et al 2005; LeMaitre et al 2002; Gillespie and Styles, 1999)</skos:definition>
		<skos:prefLabel xml:lang="fr">dolérites</skos:prefLabel>
		<skos:prefLabel xml:lang="it">dolerite</skos:prefLabel>
		<skos:prefLabel xml:lang="en">doleritic rock</skos:prefLabel>
		<skos:inScheme rdf:resource="urn:cgi:classifierScheme:CGI:SimpleLithology:2008"/>
		<skos:broader
			rdf:resource="urn:cgi:classifier:CGI:SimpleLithology:2008:phaneritic_igneous_rock"/>
	</skos:Concept>
	<skos:Concept
		rdf:about="urn:cgi:classifier:CGI:SimpleLithology:2008:dolomitic_or_magnesian_sedimentary_material">
		<skos:inScheme rdf:resource="urn:cgi:classifierScheme:CGI:SimpleLithology:2008"/>
		<skos:definition>Carbonate sedimentary material of unspecified consolidation degree with a ratio of magnesium carbonate to calcite (plus aragonite) greater than 1 to 1. Includes dolomite sediment, dolostone, lime dolostone and magnesite-stone. (after NADM SLTTs 2004, Hallsworth and Knox 1999)</skos:definition>
		<skos:prefLabel xml:lang="fr"
			>matériel sédimentaire dolomitique ou magnésien</skos:prefLabel>
		<skos:prefLabel xml:lang="it"
			>materiale sedimentario dolomitico o magnesiaco</skos:prefLabel>
		<skos:prefLabel xml:lang="en">dolomitic or magnesian sedimentary material</skos:prefLabel>
		<skos:inScheme rdf:resource="urn:cgi:classifierScheme:CGI:SimpleLithology:2008"/>
		<skos:broader
			rdf:resource="urn:cgi:classifier:CGI:SimpleLithology:2008:carbonate_sedimentary_material"
		/>
	</skos:Concept>
	<skos:Concept
		rdf:about="urn:cgi:classifier:CGI:SimpleLithology:2008:dolomitic_or_magnesian_sedimentary_rock">
		<skos:inScheme rdf:resource="urn:cgi:classifierScheme:CGI:SimpleLithology:2008"/>
		<skos:definition>Carbonate sedimentary rock with a ratio of magnesium carbonate to calcite (plus aragonite) greater than 1 to 1. Includes dolostone, lime dolostone and magnesite-stone. (after NADM SLTTs 2004, Hallsworth and Knox 1999)</skos:definition>
		<skos:prefLabel xml:lang="fr">dolomies</skos:prefLabel>
		<skos:prefLabel xml:lang="it">dolomia</skos:prefLabel>
		<skos:prefLabel xml:lang="en">dolomitic or magnesian sedimentary rock</skos:prefLabel>
		<skos:inScheme rdf:resource="urn:cgi:classifierScheme:CGI:SimpleLithology:2008"/>
		<skos:broader
			rdf:resource="urn:cgi:classifier:CGI:SimpleLithology:2008:carbonate_sedimentary_rock"/>
	</skos:Concept>
	<skos:Concept rdf:about="urn:cgi:classifier:CGI:SimpleLithology:2008:dolomitic_sediment">
		<skos:inScheme rdf:resource="urn:cgi:classifierScheme:CGI:SimpleLithology:2008"/>
		<skos:definition>Carbonate sediment with a ratio of magnesium carbonate to calcite (plus aragonite) greater than 1 to 1. (after NADM SLTTs 2004, Hallsworth and Knox 1999)</skos:definition>
		<skos:prefLabel xml:lang="fr">sédiment dolomitique</skos:prefLabel>
		<skos:prefLabel xml:lang="it">sedimento dolomitico</skos:prefLabel>
		<skos:prefLabel xml:lang="en">dolomitic sediment</skos:prefLabel>
		<skos:inScheme rdf:resource="urn:cgi:classifierScheme:CGI:SimpleLithology:2008"/>
		<skos:broader rdf:resource="urn:cgi:classifier:CGI:SimpleLithology:2008:carbonate_sediment"
		/>
	</skos:Concept>
	<skos:Concept rdf:about="urn:cgi:classifier:CGI:SimpleLithology:2008:duricrust">
		<skos:inScheme rdf:resource="urn:cgi:classifierScheme:CGI:SimpleLithology:2008"/>
		<skos:definition>Rock forming a hard crust or layer at or near the Earth's surface at the time of formation, e.g. in the upper horizons of a soil, characterized by structures indicative of pedogenic origin. (CGI concepts task group)</skos:definition>
		<skos:prefLabel xml:lang="fr">calcrète</skos:prefLabel>
		<skos:prefLabel xml:lang="it">duricrust (o orizzonte indurito)</skos:prefLabel>
		<skos:prefLabel xml:lang="en">duricrust</skos:prefLabel>
		<skos:inScheme rdf:resource="urn:cgi:classifierScheme:CGI:SimpleLithology:2008"/>
		<skos:broader rdf:resource="urn:cgi:classifier:CGI:SimpleLithology:2008:rock"/>
	</skos:Concept>
	<skos:Concept rdf:about="urn:cgi:classifier:CGI:SimpleLithology:2008:eclogite">
		<skos:inScheme rdf:resource="urn:cgi:classifierScheme:CGI:SimpleLithology:2008"/>
		<skos:definition>Metamorphic rock composed of 75 percent or more (by volume) omphacite and garnet, both of which are present as major constituents, the amount of neither of them being higher than 75 percent (by volume); the presence of plagioclase precludes classification as an eclogite. (IUGS SCMR 2007 (http://www.bgs.ac.uk/SCMR/))</skos:definition>
		<skos:prefLabel xml:lang="fr">éclogites</skos:prefLabel>
		<skos:prefLabel xml:lang="it">eclogite</skos:prefLabel>
		<skos:prefLabel xml:lang="en">eclogite</skos:prefLabel>
		<skos:inScheme rdf:resource="urn:cgi:classifierScheme:CGI:SimpleLithology:2008"/>
		<skos:broader rdf:resource="urn:cgi:classifier:CGI:SimpleLithology:2008:metamorphic_rock"/>
	</skos:Concept>
	<skos:Concept rdf:about="urn:cgi:classifier:CGI:SimpleLithology:2008:evaporite">
		<skos:inScheme rdf:resource="urn:cgi:classifierScheme:CGI:SimpleLithology:2008"/>
		<skos:definition>Nonclastic sedimentary rock composed of at least 50 percent non-carbonate salts, including chloride, sulfate or borate minerals; formed through precipitation of mineral salts from a saline solution (non-carbonate salt rock). (Jackson 1997; NADM SLTT sedimentary)</skos:definition>
		<skos:prefLabel xml:lang="fr">évaporites</skos:prefLabel>
		<skos:prefLabel xml:lang="it">evaporite</skos:prefLabel>
		<skos:prefLabel xml:lang="en">evaporite</skos:prefLabel>
		<skos:inScheme rdf:resource="urn:cgi:classifierScheme:CGI:SimpleLithology:2008"/>
		<skos:broader rdf:resource="urn:cgi:classifier:CGI:SimpleLithology:2008:sedimentary_rock"/>
	</skos:Concept>
	<skos:Concept
		rdf:about="urn:cgi:classifier:CGI:SimpleLithology:2008:exotic_alkalic_igneous_rock">
		<skos:inScheme rdf:resource="urn:cgi:classifierScheme:CGI:SimpleLithology:2008"/>
		<skos:definition>Igneous rock containing greater than 10 percent melilite or kalsilite. Typically undersaturated, ultrapotassic (kalsilitic rocks) or calcium-rich (melilitic rocks) mafic or ultramafic rocks. (NGMDB 2008)</skos:definition>
		<skos:prefLabel xml:lang="fr">roche ignée exotique alcaline</skos:prefLabel>
		<skos:prefLabel xml:lang="it">roccia ignea esotica alcalina</skos:prefLabel>
		<skos:prefLabel xml:lang="en">exotic alkalic igneous rock</skos:prefLabel>
		<skos:inScheme rdf:resource="urn:cgi:classifierScheme:CGI:SimpleLithology:2008"/>
		<skos:broader
			rdf:resource="urn:cgi:classifier:CGI:SimpleLithology:2008:exotic_composition_igneous_rock"
		/>
	</skos:Concept>
	<skos:Concept rdf:about="urn:cgi:classifier:CGI:SimpleLithology:2008:exotic_alkaline_rock">
		<skos:inScheme rdf:resource="urn:cgi:classifierScheme:CGI:SimpleLithology:2008"/>
		<skos:definition>Kimberlite, lamproite, or lamprophyre. Generally are potassic, mafic or ultramafic rocks. Olivine (commonly serpentinized in kimberlite), and phlogopite are significant constituents. (NGMDB 2008)</skos:definition>
		<skos:prefLabel xml:lang="fr">roche exotique alcaline </skos:prefLabel>
		<skos:prefLabel xml:lang="it">roccia esotica alcalina</skos:prefLabel>
		<skos:prefLabel xml:lang="en">exotic alkaline rock</skos:prefLabel>
		<skos:inScheme rdf:resource="urn:cgi:classifierScheme:CGI:SimpleLithology:2008"/>
		<skos:broader
			rdf:resource="urn:cgi:classifier:CGI:SimpleLithology:2008:exotic_composition_igneous_rock"
		/>
	</skos:Concept>
	<skos:Concept
		rdf:about="urn:cgi:classifier:CGI:SimpleLithology:2008:exotic_composition_igneous_rock">
		<skos:inScheme rdf:resource="urn:cgi:classifierScheme:CGI:SimpleLithology:2008"/>
		<skos:definition>Rock with 'exotic' mineralogical, textural or field setting characteristics; typically dark colored, with abundant phenocrysts. Criteria include: presence of greater than 10 percent melilite or leucite; presence of kalsilite; greater than 50 percent carbonate minerals. (Gillespie and Styles 1999; LeMaitre et al. 2002)</skos:definition>
		<skos:prefLabel xml:lang="fr">roche ignée de composition exotique</skos:prefLabel>
		<skos:prefLabel xml:lang="it">roccia ignea a composizione esotica</skos:prefLabel>
		<skos:prefLabel xml:lang="en">exotic composition igneous rock</skos:prefLabel>
		<skos:inScheme rdf:resource="urn:cgi:classifierScheme:CGI:SimpleLithology:2008"/>
		<skos:broader rdf:resource="urn:cgi:classifier:CGI:SimpleLithology:2008:igneous_rock"/>
	</skos:Concept>
	<skos:Concept rdf:about="urn:cgi:classifier:CGI:SimpleLithology:2008:fault_related_material">
		<skos:inScheme rdf:resource="urn:cgi:classifierScheme:CGI:SimpleLithology:2008"/>
		<skos:definition>Material formed as a result brittle faulting, composed of greater than 10 percent matrix; matrix is fine-grained material caused by tectonic grainsize reduction. Includes cohesive (cataclasite series) and non-cohesive (breccia-gouge series) material. (CGI concepts task group)</skos:definition>
		<skos:prefLabel xml:lang="fr">brèches de faille</skos:prefLabel>
		<skos:prefLabel xml:lang="it">breccia di faglia</skos:prefLabel>
		<skos:prefLabel xml:lang="en">fault-related material</skos:prefLabel>
		<skos:inScheme rdf:resource="urn:cgi:classifierScheme:CGI:SimpleLithology:2008"/>
		<skos:broader
			rdf:resource="urn:cgi:classifier:CGI:SimpleLithology:2008:composite_genesis_material"/>
	</skos:Concept>
	<skos:Concept rdf:about="urn:cgi:classifier:CGI:SimpleLithology:2008:fine_grained_igneous_rock">
		<skos:inScheme rdf:resource="urn:cgi:classifierScheme:CGI:SimpleLithology:2008"/>
		<skos:definition>Aphanitic or porphyritic igneous rock composed of greater than 10 percent groundmass, in which most of the crystals cannot be distinguished with the unaided eye; grainsize is typically less than 1mm. Igneous rocks with 'exotic' composition are excluded from this concept. (Gillespie and Styles 1999; LeMaitre et al. 2002)</skos:definition>
		<skos:prefLabel xml:lang="fr">roche ignée à grain fin</skos:prefLabel>
		<skos:prefLabel xml:lang="it">roccia ignea a grana fine</skos:prefLabel>
		<skos:prefLabel xml:lang="en">fine grained igneous rock</skos:prefLabel>
		<skos:inScheme rdf:resource="urn:cgi:classifierScheme:CGI:SimpleLithology:2008"/>
		<skos:broader rdf:resource="urn:cgi:classifier:CGI:SimpleLithology:2008:igneous_rock"/>
	</skos:Concept>
	<skos:Concept rdf:about="urn:cgi:classifier:CGI:SimpleLithology:2008:foid_dioritic_rock">
		<skos:inScheme rdf:resource="urn:cgi:classifierScheme:CGI:SimpleLithology:2008"/>
		<skos:definition>Phaneritic crystalline rock in which M is less than 90, composed of feldspathoids as 10-60 percent of the felsic minerals, sodic plagioclase (An0-An50) and large amounts of mafic minerals. Includes rocks defined modally in QAPF field 14. (LeMaitre et al. 2002)</skos:definition>
		<skos:prefLabel xml:lang="fr">diorites foïdique</skos:prefLabel>
		<skos:prefLabel xml:lang="it">diorite foiditica</skos:prefLabel>
		<skos:prefLabel xml:lang="en">foid dioritic rock</skos:prefLabel>
		<skos:inScheme rdf:resource="urn:cgi:classifierScheme:CGI:SimpleLithology:2008"/>
		<skos:broader
			rdf:resource="urn:cgi:classifier:CGI:SimpleLithology:2008:phaneritic_igneous_rock"/>
	</skos:Concept>
	<skos:Concept rdf:about="urn:cgi:classifier:CGI:SimpleLithology:2008:foid_gabbroic_rock">
		<skos:inScheme rdf:resource="urn:cgi:classifierScheme:CGI:SimpleLithology:2008"/>
		<skos:definition>Phaneritic crystalline rock in which M is less than 90, composed of feldspathoids as 10-60 percent of the felsic minerals, calcic plagioclase (An50-An100) and large amounts of mafic minerals. Includes rocks defined modally in QAPF field 14. (LeMaitre et al. 2002)</skos:definition>
		<skos:prefLabel xml:lang="fr">gabbros foïdique</skos:prefLabel>
		<skos:prefLabel xml:lang="it">gabbro foiditico</skos:prefLabel>
		<skos:prefLabel xml:lang="en">foid gabbroic rock</skos:prefLabel>
		<skos:inScheme rdf:resource="urn:cgi:classifierScheme:CGI:SimpleLithology:2008"/>
		<skos:broader
			rdf:resource="urn:cgi:classifier:CGI:SimpleLithology:2008:phaneritic_igneous_rock"/>
	</skos:Concept>
	<skos:Concept rdf:about="urn:cgi:classifier:CGI:SimpleLithology:2008:foid_syenitic_rock">
		<skos:inScheme rdf:resource="urn:cgi:classifierScheme:CGI:SimpleLithology:2008"/>
		<skos:definition>Leucocratic, phaneritic crystalline rock composed of feldspathoids as 10-60 percent of the felsic minerals, alkali feldspar and mafic minerals. Includes rocks defined modally in QAPF field 11. (LeMaitre et al. 2002)</skos:definition>
		<skos:prefLabel xml:lang="fr">syénites foïdique</skos:prefLabel>
		<skos:prefLabel xml:lang="it">sienite foiditica</skos:prefLabel>
		<skos:prefLabel xml:lang="en">foid syenitic rock</skos:prefLabel>
		<skos:inScheme rdf:resource="urn:cgi:classifierScheme:CGI:SimpleLithology:2008"/>
		<skos:broader
			rdf:resource="urn:cgi:classifier:CGI:SimpleLithology:2008:phaneritic_igneous_rock"/>
	</skos:Concept>
	<skos:Concept rdf:about="urn:cgi:classifier:CGI:SimpleLithology:2008:foiditic_rock">
		<skos:inScheme rdf:resource="urn:cgi:classifierScheme:CGI:SimpleLithology:2008"/>
		<skos:definition>Fine grained crystalline rock containing more than 60 percent feldspathoids in total light-coloured constituents. Includes rocks defined modally in QAPF field 15 or chemically in TAS field F. (LeMaitre et al. 2002)</skos:definition>
		<skos:prefLabel xml:lang="fr">roche foïdique</skos:prefLabel>
		<skos:prefLabel xml:lang="it">roccia foiditica</skos:prefLabel>
		<skos:prefLabel xml:lang="en">foiditic rock</skos:prefLabel>
		<skos:inScheme rdf:resource="urn:cgi:classifierScheme:CGI:SimpleLithology:2008"/>
		<skos:broader
			rdf:resource="urn:cgi:classifier:CGI:SimpleLithology:2008:phaneritic_igneous_rock"/>
	</skos:Concept>
	<skos:Concept rdf:about="urn:cgi:classifier:CGI:SimpleLithology:2008:foidolite">
		<skos:inScheme rdf:resource="urn:cgi:classifierScheme:CGI:SimpleLithology:2008"/>
		<skos:definition>Phaneritic crystalline rock containing more than 60 percent feldspathoids in total light-coloured constituents. Includes rocks defined modally in QAPF field 15 (LeMaitre et al. 2002)</skos:definition>
		<skos:prefLabel xml:lang="fr">foïdolite</skos:prefLabel>
		<skos:prefLabel xml:lang="it">foidolite</skos:prefLabel>
		<skos:prefLabel xml:lang="en">foidolite</skos:prefLabel>
		<skos:inScheme rdf:resource="urn:cgi:classifierScheme:CGI:SimpleLithology:2008"/>
		<skos:broader
			rdf:resource="urn:cgi:classifier:CGI:SimpleLithology:2008:phaneritic_igneous_rock"/>
	</skos:Concept>
	<skos:Concept rdf:about="urn:cgi:classifier:CGI:SimpleLithology:2008:foliated_metamorphic_rock">
		<skos:inScheme rdf:resource="urn:cgi:classifierScheme:CGI:SimpleLithology:2008"/>
		<skos:definition>Metamorphic rock in which 10 percent or more of the contained mineral grains are elements in a planar or linear fabric. Cataclastic or glassy character precludes classification with this concept. (based on NADM SLTT metamorphic)</skos:definition>
		<skos:prefLabel xml:lang="fr">roche métamorphique foliée</skos:prefLabel>
		<skos:prefLabel xml:lang="it">roccia metamorfica foliata</skos:prefLabel>
		<skos:prefLabel xml:lang="en">foliated metamorphic rock</skos:prefLabel>
		<skos:inScheme rdf:resource="urn:cgi:classifierScheme:CGI:SimpleLithology:2008"/>
		<skos:broader rdf:resource="urn:cgi:classifier:CGI:SimpleLithology:2008:metamorphic_rock"/>
	</skos:Concept>
	<skos:Concept
		rdf:about="urn:cgi:classifier:CGI:SimpleLithology:2008:fragmental_igneous_material">
		<skos:inScheme rdf:resource="urn:cgi:classifierScheme:CGI:SimpleLithology:2008"/>
		<skos:definition>Igneous material of unspecified consolidation state in which greater than 75 percent of the rock consists of fragments produced as a result of igneous rock-forming process. (CGI concepts task group)</skos:definition>
		<skos:prefLabel xml:lang="fr">matériel igné fragmenté</skos:prefLabel>
		<skos:prefLabel xml:lang="it">materiale igneo frammentato</skos:prefLabel>
		<skos:prefLabel xml:lang="en">fragmental igneous material</skos:prefLabel>
		<skos:inScheme rdf:resource="urn:cgi:classifierScheme:CGI:SimpleLithology:2008"/>
		<skos:broader rdf:resource="urn:cgi:classifier:CGI:SimpleLithology:2008:igneous_material"/>
	</skos:Concept>
	<skos:Concept rdf:about="urn:cgi:classifier:CGI:SimpleLithology:2008:fragmental_igneous_rock">
		<skos:inScheme rdf:resource="urn:cgi:classifierScheme:CGI:SimpleLithology:2008"/>
		<skos:definition>Igneous rock in which greater than 75 percent of the rock consists of fragments produced as a result of igneous rock-forming process. Includes pyroclastic rocks, autobreccia associated with lava flows and intrusive breccias. Excludes deposits reworked by epiclastic processes. (NGMDB 2008)</skos:definition>
		<skos:prefLabel xml:lang="fr">roche ignée fragmentée</skos:prefLabel>
		<skos:prefLabel xml:lang="it">roccia ignea brecciata</skos:prefLabel>
		<skos:prefLabel xml:lang="en">fragmental igneous rock</skos:prefLabel>
		<skos:inScheme rdf:resource="urn:cgi:classifierScheme:CGI:SimpleLithology:2008"/>
		<skos:broader rdf:resource="urn:cgi:classifier:CGI:SimpleLithology:2008:igneous_rock"/>
	</skos:Concept>
	<skos:Concept rdf:about="urn:cgi:classifier:CGI:SimpleLithology:2008:framestone">
		<skos:inScheme rdf:resource="urn:cgi:classifierScheme:CGI:SimpleLithology:2008"/>
		<skos:definition>Carbonate reef rock consisting of a rigid framework of colonies, shells or skeletons, with internal cavities filled with fine sediment; usually created through the activities of colonial organisms. (Hallsworth and Knox 1999; SLTTs, 2004, Table 15-3-1)</skos:definition>
		<skos:prefLabel xml:lang="fr">framestone</skos:prefLabel>
		<skos:prefLabel xml:lang="it">framestone</skos:prefLabel>
		<skos:prefLabel xml:lang="en">framestone</skos:prefLabel>
		<skos:inScheme rdf:resource="urn:cgi:classifierScheme:CGI:SimpleLithology:2008"/>
		<skos:broader
			rdf:resource="urn:cgi:classifier:CGI:SimpleLithology:2008:carbonate_sedimentary_rock"/>
	</skos:Concept>
	<skos:Concept rdf:about="urn:cgi:classifier:CGI:SimpleLithology:2008:gabbro">
		<skos:inScheme rdf:resource="urn:cgi:classifierScheme:CGI:SimpleLithology:2008"/>
		<skos:definition>Phaneritic crystalline rock composed essentially of calcic plagioclase (An50 to An100), pyroxene and iron oxides. Includes rocks defined modally in QAPF Field 10 as gabbro. (LeMaitre et al. 2002)</skos:definition>
		<skos:prefLabel xml:lang="fr">gabbros</skos:prefLabel>
		<skos:prefLabel xml:lang="it">gabbro</skos:prefLabel>
		<skos:prefLabel xml:lang="en">gabbro</skos:prefLabel>
		<skos:inScheme rdf:resource="urn:cgi:classifierScheme:CGI:SimpleLithology:2008"/>
		<skos:broader rdf:resource="urn:cgi:classifier:CGI:SimpleLithology:2008:gabbroic_rock"/>
	</skos:Concept>
	<skos:Concept rdf:about="urn:cgi:classifier:CGI:SimpleLithology:2008:gabbroic_rock">
		<skos:inScheme rdf:resource="urn:cgi:classifierScheme:CGI:SimpleLithology:2008"/>
		<skos:definition>Phaneritic crystalline rock composed of 65 percent or more of calcic plagioclase and up to 20 percent quartz or up to 10 percent feldspathoid. Includes rocks defined modally in QAPF fields 9 and 10 as gabbro or monzogabbro and foid-bearing varieties. (LeMaitre et al. 2002)</skos:definition>
		<skos:prefLabel xml:lang="fr">roche gabbroïque</skos:prefLabel>
		<skos:prefLabel xml:lang="it">roccia gabbrica</skos:prefLabel>
		<skos:prefLabel xml:lang="en">gabbroic rock</skos:prefLabel>
		<skos:inScheme rdf:resource="urn:cgi:classifierScheme:CGI:SimpleLithology:2008"/>
		<skos:broader
			rdf:resource="urn:cgi:classifier:CGI:SimpleLithology:2008:phaneritic_igneous_rock"/>
	</skos:Concept>
	<skos:Concept rdf:about="urn:cgi:classifier:CGI:SimpleLithology:2008:glassy_igneous_rock">
		<skos:inScheme rdf:resource="urn:cgi:classifierScheme:CGI:SimpleLithology:2008"/>
		<skos:definition>Igneous rock that consists of greater than 90 percent glass. (NGMDB Glassy extrusive rock)</skos:definition>
		<skos:prefLabel xml:lang="fr">roche ignée vitreuse</skos:prefLabel>
		<skos:prefLabel xml:lang="it">roccia ignea vetrosa</skos:prefLabel>
		<skos:prefLabel xml:lang="en">glassy igneous rock</skos:prefLabel>
		<skos:inScheme rdf:resource="urn:cgi:classifierScheme:CGI:SimpleLithology:2008"/>
		<skos:broader rdf:resource="urn:cgi:classifier:CGI:SimpleLithology:2008:igneous_rock"/>
	</skos:Concept>
	<skos:Concept rdf:about="urn:cgi:classifier:CGI:SimpleLithology:2008:gneiss">
		<skos:inScheme rdf:resource="urn:cgi:classifierScheme:CGI:SimpleLithology:2008"/>
		<skos:definition>Foliated metamorphic rock with bands or lenticles rich in granular minerals alternating with bands or lenticles rich in minerals with a flaky or elongate prismatic habit. Mylonitic foliation or well developed, continuous schistosity (greater than 50 percent of the rock consists of grains participate in a planar or linear fabric) precludes classification with this concept. (Neuendorf et al. 2005)</skos:definition>
		<skos:prefLabel xml:lang="fr">orthogneiss</skos:prefLabel>
		<skos:prefLabel xml:lang="it">gneiss</skos:prefLabel>
		<skos:prefLabel xml:lang="en">gneiss</skos:prefLabel>
		<skos:inScheme rdf:resource="urn:cgi:classifierScheme:CGI:SimpleLithology:2008"/>
		<skos:broader
			rdf:resource="urn:cgi:classifier:CGI:SimpleLithology:2008:foliated_metamorphic_rock"/>
	</skos:Concept>
	<skos:Concept rdf:about="urn:cgi:classifier:CGI:SimpleLithology:2008:grainstone">
		<skos:inScheme rdf:resource="urn:cgi:classifierScheme:CGI:SimpleLithology:2008"/>
		<skos:definition>Carbonate sedimentary rock with recognizable depositional fabric that is grain-supported; contains little or no mud matrix. (Dunham 1962)</skos:definition>
		<skos:prefLabel xml:lang="fr">grainstone</skos:prefLabel>
		<skos:prefLabel xml:lang="it">grainstone</skos:prefLabel>
		<skos:prefLabel xml:lang="en">grainstone</skos:prefLabel>
		<skos:inScheme rdf:resource="urn:cgi:classifierScheme:CGI:SimpleLithology:2008"/>
		<skos:broader
			rdf:resource="urn:cgi:classifier:CGI:SimpleLithology:2008:carbonate_sedimentary_rock"/>
	</skos:Concept>
	<skos:Concept rdf:about="urn:cgi:classifier:CGI:SimpleLithology:2008:granite">
		<skos:inScheme rdf:resource="urn:cgi:classifierScheme:CGI:SimpleLithology:2008"/>
		<skos:definition>Phaneritic crystalline rock consisting of quartz, alkali feldspar and plagioclase (typically sodic) in variable amounts, usually with biotite and/or hornblende. Includes rocks defined modally in QAPF Field 3. (LeMaitre et al. 2002)</skos:definition>
		<skos:prefLabel xml:lang="fr">granite</skos:prefLabel>
		<skos:prefLabel xml:lang="it">granito</skos:prefLabel>
		<skos:prefLabel xml:lang="en">granite</skos:prefLabel>
		<skos:inScheme rdf:resource="urn:cgi:classifierScheme:CGI:SimpleLithology:2008"/>
		<skos:broader rdf:resource="urn:cgi:classifier:CGI:SimpleLithology:2008:granitic_rock"/>
	</skos:Concept>
	<skos:Concept rdf:about="urn:cgi:classifier:CGI:SimpleLithology:2008:granitic_rock">
		<skos:inScheme rdf:resource="urn:cgi:classifierScheme:CGI:SimpleLithology:2008"/>
		<skos:definition>Phaneritic crystalline igneous rock consisting of quartz, alkali feldspar and/or plagioclase. Includes rocks defined modally in QAPF fields 2, 3, 4 and 5 as alkali granite, granite, granodiorite or tonalite. (LeMaitre et al. 2002)</skos:definition>
		<skos:prefLabel xml:lang="fr">granitoïdes</skos:prefLabel>
		<skos:prefLabel xml:lang="it">granitoide</skos:prefLabel>
		<skos:prefLabel xml:lang="en">granitic rock</skos:prefLabel>
		<skos:inScheme rdf:resource="urn:cgi:classifierScheme:CGI:SimpleLithology:2008"/>
		<skos:broader
			rdf:resource="urn:cgi:classifier:CGI:SimpleLithology:2008:phaneritic_igneous_rock"/>
	</skos:Concept>
	<skos:Concept rdf:about="urn:cgi:classifier:CGI:SimpleLithology:2008:granodiorite">
		<skos:inScheme rdf:resource="urn:cgi:classifierScheme:CGI:SimpleLithology:2008"/>
		<skos:definition>Phaneritic crystalline rock consisting essentially of quartz, sodic plagioclase and lesser amounts of alkali feldspar with minor hornblende and biotite. Includes rocks defined modally in QAPF field 4. (LeMaitre et al. 2002)</skos:definition>
		<skos:prefLabel xml:lang="fr">granodiorites</skos:prefLabel>
		<skos:prefLabel xml:lang="it">granodiorite</skos:prefLabel>
		<skos:prefLabel xml:lang="en">granodiorite</skos:prefLabel>
		<skos:inScheme rdf:resource="urn:cgi:classifierScheme:CGI:SimpleLithology:2008"/>
		<skos:broader rdf:resource="urn:cgi:classifier:CGI:SimpleLithology:2008:granitic_rock"/>
	</skos:Concept>
	<skos:Concept rdf:about="urn:cgi:classifier:CGI:SimpleLithology:2008:granofels">
		<skos:inScheme rdf:resource="urn:cgi:classifierScheme:CGI:SimpleLithology:2008"/>
		<skos:definition>Phaneritic metamorphic rock with granoblastic fabric and very little or no foliation (less than 10 percent of the mineral grains in the rock are elements in a planar or linear fabric). (NADM SLTTm 2004)</skos:definition>
		<skos:prefLabel xml:lang="fr">schiste tacheté (?)</skos:prefLabel>
		<skos:prefLabel xml:lang="it">granofels</skos:prefLabel>
		<skos:prefLabel xml:lang="en">granofels</skos:prefLabel>
		<skos:inScheme rdf:resource="urn:cgi:classifierScheme:CGI:SimpleLithology:2008"/>
		<skos:broader rdf:resource="urn:cgi:classifier:CGI:SimpleLithology:2008:metamorphic_rock"/>
	</skos:Concept>
	<skos:Concept rdf:about="urn:cgi:classifier:CGI:SimpleLithology:2008:gravel">
		<skos:inScheme rdf:resource="urn:cgi:classifierScheme:CGI:SimpleLithology:2008"/>
		<skos:definition>Sediment containing greater than 30 percent gravel-size particles (greater than 2.0 mm diameter). (NADM SLTTs 2004)</skos:definition>
		<skos:prefLabel xml:lang="fr">graviers</skos:prefLabel>
		<skos:prefLabel xml:lang="it">ghiaia</skos:prefLabel>
		<skos:prefLabel xml:lang="en">gravel</skos:prefLabel>
		<skos:inScheme rdf:resource="urn:cgi:classifierScheme:CGI:SimpleLithology:2008"/>
		<skos:broader rdf:resource="urn:cgi:classifier:CGI:SimpleLithology:2008:clastic_sediment"/>
	</skos:Concept>
	<skos:Concept rdf:about="urn:cgi:classifier:CGI:SimpleLithology:2008:hornblendite">
		<skos:inScheme rdf:resource="urn:cgi:classifierScheme:CGI:SimpleLithology:2008"/>
		<skos:definition>Ultramafic rock that consists of greater than 40 percent hornblende plus pyroxene and has a hornblende to pyroxene ratio greater than 1. Includes olivine hornblendite, olivine-pyroxene hornblendite, pyroxene hornblendite, and hornblendite. (LeMaitre et al. 2002)</skos:definition>
		<skos:prefLabel xml:lang="fr">hornblendite</skos:prefLabel>
		<skos:prefLabel xml:lang="it">hornblendite</skos:prefLabel>
		<skos:prefLabel xml:lang="en">hornblendite</skos:prefLabel>
		<skos:inScheme rdf:resource="urn:cgi:classifierScheme:CGI:SimpleLithology:2008"/>
		<skos:broader
			rdf:resource="urn:cgi:classifier:CGI:SimpleLithology:2008:ultrabasic_igneous_rock"/>
	</skos:Concept>
	<skos:Concept rdf:about="urn:cgi:classifier:CGI:SimpleLithology:2008:hornfels">
		<skos:inScheme rdf:resource="urn:cgi:classifierScheme:CGI:SimpleLithology:2008"/>
		<skos:definition>Granofels composed of a mosaic of equidimensional grains in a characteristically granoblastic or decussate matrix; porphyroblasts or relict phenocrysts may be present. Typically formed by contact metamorphism. (IUGS SCMR 2007 (http://www.bgs.ac.uk/SCMR/))</skos:definition>
		<skos:prefLabel xml:lang="fr">cornéennes</skos:prefLabel>
		<skos:prefLabel xml:lang="it">hornfels (o granofels)</skos:prefLabel>
		<skos:prefLabel xml:lang="en">hornfels</skos:prefLabel>
		<skos:inScheme rdf:resource="urn:cgi:classifierScheme:CGI:SimpleLithology:2008"/>
		<skos:broader rdf:resource="urn:cgi:classifier:CGI:SimpleLithology:2008:granofels"/>
	</skos:Concept>
	<skos:Concept rdf:about="urn:cgi:classifier:CGI:SimpleLithology:2008:igneous_material">
		<skos:inScheme rdf:resource="urn:cgi:classifierScheme:CGI:SimpleLithology:2008"/>
		<skos:definition>Earth material formed as a result of igneous processes, eg. intrusion and cooling of magma in the crust, volcanic eruption. (CGI concepts task group)</skos:definition>
		<skos:prefLabel xml:lang="fr">matériel igné</skos:prefLabel>
		<skos:prefLabel xml:lang="it">materiale igneo</skos:prefLabel>
		<skos:prefLabel xml:lang="en">igneous material</skos:prefLabel>
		<skos:inScheme rdf:resource="urn:cgi:classifierScheme:CGI:SimpleLithology:2008"/>
		<skos:broader rdf:resource="urn:cgi:classifier:CGI:SimpleLithology:2008:compound_material"/>
	</skos:Concept>
	<skos:Concept rdf:about="urn:cgi:classifier:CGI:SimpleLithology:2008:igneous_rock">
		<skos:inScheme rdf:resource="urn:cgi:classifierScheme:CGI:SimpleLithology:2008"/>
		<skos:definition>Rock formed as a result of igneous processes, for example intrusion and cooling of magma in the crust, or volcanic eruption. (NGMDB 2008)</skos:definition>
		<skos:prefLabel xml:lang="fr">roche ignée</skos:prefLabel>
		<skos:prefLabel xml:lang="it">roccia ignea</skos:prefLabel>
		<skos:prefLabel xml:lang="en">igneous rock</skos:prefLabel>
		<skos:inScheme rdf:resource="urn:cgi:classifierScheme:CGI:SimpleLithology:2008"/>
		<skos:broader rdf:resource="urn:cgi:classifier:CGI:SimpleLithology:2008:rock"/>
	</skos:Concept>
	<skos:Concept rdf:about="urn:cgi:classifier:CGI:SimpleLithology:2008:impact_metamorphic_rock">
		<skos:inScheme rdf:resource="urn:cgi:classifierScheme:CGI:SimpleLithology:2008"/>
		<skos:definition>Rock that contains features indicative of shock metamorphism, such as microscopic planar deformation features within grains or shatter cones. Includes breccias and melt rocks. (Stöffler and Grieve 2007; Jackson 1997)</skos:definition>
		<skos:prefLabel xml:lang="fr">impactite</skos:prefLabel>
		<skos:prefLabel xml:lang="it">roccia metamorfica da impatto</skos:prefLabel>
		<skos:prefLabel xml:lang="en">impact metamorphic rock</skos:prefLabel>
		<skos:inScheme rdf:resource="urn:cgi:classifierScheme:CGI:SimpleLithology:2008"/>
		<skos:broader
			rdf:resource="urn:cgi:classifier:CGI:SimpleLithology:2008:composite_genesis_rock"/>
	</skos:Concept>
	<skos:Concept
		rdf:about="urn:cgi:classifier:CGI:SimpleLithology:2008:intermediate_composition_igneous_material">
		<skos:inScheme rdf:resource="urn:cgi:classifierScheme:CGI:SimpleLithology:2008"/>
		<skos:definition>Igneous material with between 52 and 63 percent SiO2. (after LeMaitre et al. 2002)</skos:definition>
		<skos:prefLabel xml:lang="fr">matériel igné de composition intermédiaire</skos:prefLabel>
		<skos:prefLabel xml:lang="it">materiale igneo a composizione intermedia</skos:prefLabel>
		<skos:prefLabel xml:lang="en">intermediate composition igneous material</skos:prefLabel>
		<skos:inScheme rdf:resource="urn:cgi:classifierScheme:CGI:SimpleLithology:2008"/>
		<skos:broader rdf:resource="urn:cgi:classifier:CGI:SimpleLithology:2008:igneous_material"/>
	</skos:Concept>
	<skos:Concept
		rdf:about="urn:cgi:classifier:CGI:SimpleLithology:2008:intermediate_composition_igneous_rock">
		<skos:inScheme rdf:resource="urn:cgi:classifierScheme:CGI:SimpleLithology:2008"/>
		<skos:definition>Igneous rock with between 52 and 63 percent SiO2. (after LeMaitre et al. 2002)</skos:definition>
		<skos:prefLabel xml:lang="fr">roche ignés de composition intermédiaire</skos:prefLabel>
		<skos:prefLabel xml:lang="it">roccia ignea a composizione intermedia</skos:prefLabel>
		<skos:prefLabel xml:lang="en">intermediate composition igneous rock</skos:prefLabel>
		<skos:inScheme rdf:resource="urn:cgi:classifierScheme:CGI:SimpleLithology:2008"/>
		<skos:broader rdf:resource="urn:cgi:classifier:CGI:SimpleLithology:2008:igneous_rock"/>
	</skos:Concept>
	<skos:Concept rdf:about="urn:cgi:classifier:CGI:SimpleLithology:2008:iron_rich_sediment">
		<skos:inScheme rdf:resource="urn:cgi:classifierScheme:CGI:SimpleLithology:2008"/>
		<skos:definition>Sediment that consists of at least 50 percent iron-bearing minerals (hematite, magnetite, limonite-group, siderite, iron-sulfides), as determined by hand-lens or petrographic analysis. Corresponds to a rock typically containing 15 percent iron by weight. (NGMDB 2008)</skos:definition>
		<skos:prefLabel xml:lang="fr">sédiment ferrugineux</skos:prefLabel>
		<skos:prefLabel xml:lang="it">sedimento ferrifero</skos:prefLabel>
		<skos:prefLabel xml:lang="en">iron rich sediment</skos:prefLabel>
		<skos:inScheme rdf:resource="urn:cgi:classifierScheme:CGI:SimpleLithology:2008"/>
		<skos:broader rdf:resource="urn:cgi:classifier:CGI:SimpleLithology:2008:sediment"/>
	</skos:Concept>
	<skos:Concept
		rdf:about="urn:cgi:classifier:CGI:SimpleLithology:2008:iron_rich_sedimentary_material">
		<skos:inScheme rdf:resource="urn:cgi:classifierScheme:CGI:SimpleLithology:2008"/>
		<skos:definition>Sedimentary material of unspecified consolidation state that consists of at least 50 percent iron-bearing minerals (hematite, magnetite, limonite-group, siderite, iron-sulfides), as determined by hand-lens or petrographic analysis. Corresponds to a rock typically containing 15 percent iron by weight. (NGMDB 2008)</skos:definition>
		<skos:prefLabel xml:lang="fr">matériel sédimentaire ferrugineux</skos:prefLabel>
		<skos:prefLabel xml:lang="it">materiale sedimentario ferrifero</skos:prefLabel>
		<skos:prefLabel xml:lang="en">iron rich sedimentary material</skos:prefLabel>
		<skos:inScheme rdf:resource="urn:cgi:classifierScheme:CGI:SimpleLithology:2008"/>
		<skos:broader
			rdf:resource="urn:cgi:classifier:CGI:SimpleLithology:2008:sedimentary_material"/>
	</skos:Concept>
	<skos:Concept rdf:about="urn:cgi:classifier:CGI:SimpleLithology:2008:iron_rich_sedimentary_rock">
		<skos:inScheme rdf:resource="urn:cgi:classifierScheme:CGI:SimpleLithology:2008"/>
		<skos:definition>Sedimentary rock that consists of at least 50 percent iron-bearing minerals (hematite, magnetite, limonite-group, siderite, iron-sulfides), as determined by hand-lens or petrographic analysis. Corresponds to a rock typically containing 15 percent iron by weight. (Hallsworth and Knox 1999; NADM SLTT sedimentary)</skos:definition>
		<skos:prefLabel xml:lang="fr">roche sédimentaire ferrugineux</skos:prefLabel>
		<skos:prefLabel xml:lang="it">roccia sedimentaria ferrifera</skos:prefLabel>
		<skos:prefLabel xml:lang="en">iron rich sedimentary rock</skos:prefLabel>
		<skos:inScheme rdf:resource="urn:cgi:classifierScheme:CGI:SimpleLithology:2008"/>
		<skos:broader rdf:resource="urn:cgi:classifier:CGI:SimpleLithology:2008:sedimentary_rock"/>
	</skos:Concept>
	<skos:Concept rdf:about="urn:cgi:classifier:CGI:SimpleLithology:2008:komatiitic_rock">
		<skos:inScheme rdf:resource="urn:cgi:classifierScheme:CGI:SimpleLithology:2008"/>
		<skos:definition>Ultramafic volcanic rock, typically with spinifex texture of intergrown skeletal and bladed olivine and pyroxene crystals set in abundant glass. Includes picrite, komatiite and meimechite. (LeMaitre et al. 2002)</skos:definition>
		<skos:prefLabel xml:lang="fr">roche komatitique</skos:prefLabel>
		<skos:prefLabel xml:lang="it">komatiite</skos:prefLabel>
		<skos:prefLabel xml:lang="en">komatiitic rock</skos:prefLabel>
		<skos:inScheme rdf:resource="urn:cgi:classifierScheme:CGI:SimpleLithology:2008"/>
		<skos:broader
			rdf:resource="urn:cgi:classifier:CGI:SimpleLithology:2008:ultrabasic_igneous_rock"/>
	</skos:Concept>
	<skos:Concept rdf:about="urn:cgi:classifier:CGI:SimpleLithology:2008:marble">
		<skos:inScheme rdf:resource="urn:cgi:classifierScheme:CGI:SimpleLithology:2008"/>
		<skos:definition>Metamorphic rock consisting of greater than 75 percent fine- to coarse-grained recrystallized calcite and/or dolomite; usually with a granoblastic, saccharoidal texture. (IUGS SCMR 2007 (http://www.bgs.ac.uk/SCMR/), SLTTm1.0 2004)</skos:definition>
		<skos:prefLabel xml:lang="fr">marbres</skos:prefLabel>
		<skos:prefLabel xml:lang="it">marmo</skos:prefLabel>
		<skos:prefLabel xml:lang="en">marble</skos:prefLabel>
		<skos:inScheme rdf:resource="urn:cgi:classifierScheme:CGI:SimpleLithology:2008"/>
		<skos:broader rdf:resource="urn:cgi:classifier:CGI:SimpleLithology:2008:metamorphic_rock"/>
	</skos:Concept>
	<skos:Concept rdf:about="urn:cgi:classifier:CGI:SimpleLithology:2008:metamorphic_rock">
		<skos:inScheme rdf:resource="urn:cgi:classifierScheme:CGI:SimpleLithology:2008"/>
		<skos:definition>Rock formed by solid-state mineralogical, chemical and/or structural changes to a pre-existing rock, in response to marked changes in temperature, pressure, shearing stress and chemical environment; generally at depth in the crust. (Jackson 1997)</skos:definition>
		<skos:prefLabel xml:lang="fr">métamorphites indifférenciées</skos:prefLabel>
		<skos:prefLabel xml:lang="it">roccia metamorfica</skos:prefLabel>
		<skos:prefLabel xml:lang="en">metamorphic rock</skos:prefLabel>
		<skos:inScheme rdf:resource="urn:cgi:classifierScheme:CGI:SimpleLithology:2008"/>
		<skos:broader
			rdf:resource="urn:cgi:classifier:CGI:SimpleLithology:2008:composite_genesis_rock"/>
	</skos:Concept>
	<skos:Concept rdf:about="urn:cgi:classifier:CGI:SimpleLithology:2008:migmatite">
		<skos:inScheme rdf:resource="urn:cgi:classifierScheme:CGI:SimpleLithology:2008"/>
		<skos:definition>Silicate metamorphic rock that is pervasively heterogeneous on a meso- to megascopic scale that typically consists of darker and lighter parts; the darker parts usually exhibit features of metamorphic rocks whereas the lighter parts are of igneous-looking appearance. (after IUGS SCMR 2007 (http://www.bgs.ac.uk/SCMR/))</skos:definition>
		<skos:prefLabel xml:lang="fr">migmatites</skos:prefLabel>
		<skos:prefLabel xml:lang="it">migmatite</skos:prefLabel>
		<skos:prefLabel xml:lang="en">migmatite</skos:prefLabel>
		<skos:inScheme rdf:resource="urn:cgi:classifierScheme:CGI:SimpleLithology:2008"/>
		<skos:broader rdf:resource="urn:cgi:classifier:CGI:SimpleLithology:2008:metamorphic_rock"/>
	</skos:Concept>
	<skos:Concept rdf:about="urn:cgi:classifier:CGI:SimpleLithology:2008:monzodiorite">
		<skos:inScheme rdf:resource="urn:cgi:classifierScheme:CGI:SimpleLithology:2008"/>
		<skos:definition>Phaneritic crystalline igneous rock consisting of sodic plagioclase (An0 to An50), alkali feldspar, hornblende and biotite, with or without pyroxene. Includes rocks defined modally in QAPF field 9 as monzodiorite. (CGI concepts task group)</skos:definition>
		<skos:prefLabel xml:lang="fr">monzodiorite</skos:prefLabel>
		<skos:prefLabel xml:lang="it">monzodiorite</skos:prefLabel>
		<skos:prefLabel xml:lang="en">monzodiorite</skos:prefLabel>
		<skos:inScheme rdf:resource="urn:cgi:classifierScheme:CGI:SimpleLithology:2008"/>
		<skos:broader rdf:resource="urn:cgi:classifier:CGI:SimpleLithology:2008:dioritic_rock"/>
	</skos:Concept>
	<skos:Concept rdf:about="urn:cgi:classifier:CGI:SimpleLithology:2008:monzogabbro">
		<skos:inScheme rdf:resource="urn:cgi:classifierScheme:CGI:SimpleLithology:2008"/>
		<skos:definition>Phaneritic crystalline igneous rock consisting of calcic plagioclase (An50 to An100), alkali feldspar, hornblende and biotite, with or without pyroxene. Includes rocks defined modally in QAPF field 9 as monzogabbro. (CGI concepts task group)</skos:definition>
		<skos:prefLabel xml:lang="fr">monzogabbro</skos:prefLabel>
		<skos:prefLabel xml:lang="it">monzogabbro</skos:prefLabel>
		<skos:prefLabel xml:lang="en">monzogabbro</skos:prefLabel>
		<skos:inScheme rdf:resource="urn:cgi:classifierScheme:CGI:SimpleLithology:2008"/>
		<skos:broader rdf:resource="urn:cgi:classifier:CGI:SimpleLithology:2008:gabbroic_rock"/>
	</skos:Concept>
	<skos:Concept rdf:about="urn:cgi:classifier:CGI:SimpleLithology:2008:monzonite">
		<skos:inScheme rdf:resource="urn:cgi:classifierScheme:CGI:SimpleLithology:2008"/>
		<skos:definition>Phaneritic crystalline rock containing almost equal amounts of plagioclase and alkali feldspar with minor amphibole and/or pyroxene and little or no quartz. Includes rocks defined modally in QAPF Field 8. (LeMaitre et al. 2002)</skos:definition>
		<skos:prefLabel xml:lang="fr">monzonite</skos:prefLabel>
		<skos:prefLabel xml:lang="it">monzonite</skos:prefLabel>
		<skos:prefLabel xml:lang="en">monzonite</skos:prefLabel>
		<skos:inScheme rdf:resource="urn:cgi:classifierScheme:CGI:SimpleLithology:2008"/>
		<skos:broader
			rdf:resource="urn:cgi:classifier:CGI:SimpleLithology:2008:phaneritic_igneous_rock"/>
	</skos:Concept>
	<skos:Concept rdf:about="urn:cgi:classifier:CGI:SimpleLithology:2008:mud">
		<skos:inScheme rdf:resource="urn:cgi:classifierScheme:CGI:SimpleLithology:2008"/>
		<skos:definition>Clastic sediment consisting of less than 30 percent gravel-size (2 mm) particles and with a mud to sand ratio greater than 1. Clasts may be of any composition or origin. (based on NADM SLTT sedimentary; Neuendorf et al. 2005; particle size from Wentworth grade scale)</skos:definition>
		<skos:prefLabel xml:lang="fr">boue </skos:prefLabel>
		<skos:prefLabel xml:lang="it">fango</skos:prefLabel>
		<skos:prefLabel xml:lang="en">mud</skos:prefLabel>
		<skos:inScheme rdf:resource="urn:cgi:classifierScheme:CGI:SimpleLithology:2008"/>
		<skos:broader rdf:resource="urn:cgi:classifier:CGI:SimpleLithology:2008:clastic_sediment"/>
	</skos:Concept>
	<skos:Concept rdf:about="urn:cgi:classifier:CGI:SimpleLithology:2008:mudstone">
		<skos:inScheme rdf:resource="urn:cgi:classifierScheme:CGI:SimpleLithology:2008"/>
		<skos:definition>Clastic sedimentary rock consisting of less than 30 percent gravel-size (2 mm) particles and with a mud to sand ratio greater than 1. Clasts may be of any composition or origin. (Pettijohn et al. 1987 referenced in Hallsworth and Knox 1999; extrapolated from Folk, 1954, Figure 1a)</skos:definition>
		<skos:prefLabel xml:lang="fr">mudstone</skos:prefLabel>
		<skos:prefLabel xml:lang="it">mudstone</skos:prefLabel>
		<skos:prefLabel xml:lang="en">mudstone</skos:prefLabel>
		<skos:inScheme rdf:resource="urn:cgi:classifierScheme:CGI:SimpleLithology:2008"/>
		<skos:broader
			rdf:resource="urn:cgi:classifier:CGI:SimpleLithology:2008:clastic_sedimentary_rock"/>
	</skos:Concept>
	<skos:Concept rdf:about="urn:cgi:classifier:CGI:SimpleLithology:2008:mylonitic_rock">
		<skos:inScheme rdf:resource="urn:cgi:classifierScheme:CGI:SimpleLithology:2008"/>
		<skos:definition>Metamorphic rock characterised by a foliation resulting from tectonic grain size reduction, in which more than 10 percent of the rock volume has undergone grain size reduction. Includes protomylonite, mylonite, ultramylonite, phyllonite and blastomylonite. (Marshak and Mitra 1988)</skos:definition>
		<skos:prefLabel xml:lang="fr">mylonites</skos:prefLabel>
		<skos:prefLabel xml:lang="it">milonite</skos:prefLabel>
		<skos:prefLabel xml:lang="en">mylonitic rock</skos:prefLabel>
		<skos:inScheme rdf:resource="urn:cgi:classifierScheme:CGI:SimpleLithology:2008"/>
		<skos:broader
			rdf:resource="urn:cgi:classifier:CGI:SimpleLithology:2008:foliated_metamorphic_rock"/>
	</skos:Concept>
	<skos:Concept
		rdf:about="urn:cgi:classifier:CGI:SimpleLithology:2008:natural_unconsolidated_material">
		<skos:inScheme rdf:resource="urn:cgi:classifierScheme:CGI:SimpleLithology:2008"/>
		<skos:definition>Unconsolidated material known to have natural, ie. not human-made, origin. (NGMDB vocabulary)</skos:definition>
		<skos:prefLabel xml:lang="fr">matériel naturel non consolidé</skos:prefLabel>
		<skos:prefLabel xml:lang="it">materiale naturale non consolidato</skos:prefLabel>
		<skos:prefLabel xml:lang="en">natural unconsolidated material</skos:prefLabel>
		<skos:inScheme rdf:resource="urn:cgi:classifierScheme:CGI:SimpleLithology:2008"/>
		<skos:broader
			rdf:resource="urn:cgi:classifier:CGI:SimpleLithology:2008:unconsolidated_material"/>
	</skos:Concept>
	<skos:Concept
		rdf:about="urn:cgi:classifier:CGI:SimpleLithology:2008:non_clastic_siliceous_sediment">
		<skos:inScheme rdf:resource="urn:cgi:classifierScheme:CGI:SimpleLithology:2008"/>
		<skos:definition>Sediment that consists of at least 50 percent silicate mineral material, deposited directly by chemical or biological processes at the depositional surface, or in particles formed by chemical or biological processes within the basin of deposition. (NGMDB 2008; Hallsworth and Knox 1999)</skos:definition>
		<skos:prefLabel xml:lang="fr">sédiment siliceux non-clastique</skos:prefLabel>
		<skos:prefLabel xml:lang="it">sedimento siliceo non clastico</skos:prefLabel>
		<skos:prefLabel xml:lang="en">non-clastic siliceous sediment</skos:prefLabel>
		<skos:inScheme rdf:resource="urn:cgi:classifierScheme:CGI:SimpleLithology:2008"/>
		<skos:broader rdf:resource="urn:cgi:classifier:CGI:SimpleLithology:2008:sediment"/>
	</skos:Concept>
	<skos:Concept
		rdf:about="urn:cgi:classifier:CGI:SimpleLithology:2008:non_clastic_siliceous_sedimentary_material">
		<skos:inScheme rdf:resource="urn:cgi:classifierScheme:CGI:SimpleLithology:2008"/>
		<skos:definition>Sedimentary material that consists of at least 50 percent silicate mineral material, deposited directly by chemical or biological processes at the depositional surface, or in particles formed by chemical or biological processes within the basin of deposition. (NGMDB 2008)</skos:definition>
		<skos:prefLabel xml:lang="fr">matériel sédimentaire siliceux non-clastique</skos:prefLabel>
		<skos:prefLabel xml:lang="it">materiale sedimentario siliceo non-clastico</skos:prefLabel>
		<skos:prefLabel xml:lang="en">non-clastic siliceous sedimentary material</skos:prefLabel>
		<skos:inScheme rdf:resource="urn:cgi:classifierScheme:CGI:SimpleLithology:2008"/>
		<skos:broader
			rdf:resource="urn:cgi:classifier:CGI:SimpleLithology:2008:sedimentary_material"/>
	</skos:Concept>
	<skos:Concept
		rdf:about="urn:cgi:classifier:CGI:SimpleLithology:2008:non_clastic_siliceous_sedimentary_rock">
		<skos:inScheme rdf:resource="urn:cgi:classifierScheme:CGI:SimpleLithology:2008"/>
		<skos:definition>Sedimentary rock that consists of at least 50 percent silicate mineral material, deposited directly by chemical or biological processes at the depositional surface, or in particles formed by chemical or biological processes within the basin of deposition. (NGMDB 2008)</skos:definition>
		<skos:prefLabel xml:lang="fr">roche sédimentaire siliceuse non-clastique</skos:prefLabel>
		<skos:prefLabel xml:lang="it">roccia sedimentaria silicea non clastica</skos:prefLabel>
		<skos:prefLabel xml:lang="en">non-clastic siliceous sedimentary rock</skos:prefLabel>
		<skos:inScheme rdf:resource="urn:cgi:classifierScheme:CGI:SimpleLithology:2008"/>
		<skos:broader rdf:resource="urn:cgi:classifier:CGI:SimpleLithology:2008:sedimentary_rock"/>
	</skos:Concept>
	<skos:Concept rdf:about="urn:cgi:classifier:CGI:SimpleLithology:2008:ooze">
		<skos:inScheme rdf:resource="urn:cgi:classifierScheme:CGI:SimpleLithology:2008"/>
		<skos:definition>Mud with a sand to mud ratio less than 1 to 9 that contains at least 30 percent skeletal remains of pelagic organisms. Less than 1 percent gravel and less than 50 percent carbonate minerals. (based on Bates and Jackson 1987 and Hallsworth and Knox 1999)</skos:definition>
		<skos:prefLabel xml:lang="fr">vases</skos:prefLabel>
		<skos:prefLabel xml:lang="it">ooze</skos:prefLabel>
		<skos:prefLabel xml:lang="en">ooze</skos:prefLabel>
		<skos:inScheme rdf:resource="urn:cgi:classifierScheme:CGI:SimpleLithology:2008"/>
		<skos:broader rdf:resource="urn:cgi:classifier:CGI:SimpleLithology:2008:biogenic_sediment"/>
	</skos:Concept>
	<skos:Concept rdf:about="urn:cgi:classifier:CGI:SimpleLithology:2008:organic_rich_sediment">
		<skos:inScheme rdf:resource="urn:cgi:classifierScheme:CGI:SimpleLithology:2008"/>
		<skos:definition>Sediment with color, composition, texture and apparent density indicating greater than 50 percent organic content by weight on a moisture-free basis. (NADM SLTT sedimentary)</skos:definition>
		<skos:prefLabel xml:lang="fr">sédiment enrichie en matière organique</skos:prefLabel>
		<skos:prefLabel xml:lang="it">sedimento arricchito di materia organica</skos:prefLabel>
		<skos:prefLabel xml:lang="en">organic rich sediment</skos:prefLabel>
		<skos:inScheme rdf:resource="urn:cgi:classifierScheme:CGI:SimpleLithology:2008"/>
		<skos:broader rdf:resource="urn:cgi:classifier:CGI:SimpleLithology:2008:sediment"/>
	</skos:Concept>
	<skos:Concept
		rdf:about="urn:cgi:classifier:CGI:SimpleLithology:2008:organic_rich_sedimentary_material">
		<skos:inScheme rdf:resource="urn:cgi:classifierScheme:CGI:SimpleLithology:2008"/>
		<skos:definition>Sedimentary material in which 50 percent or more of the primary sedimentary material is organic carbon. (NADM SLTT sedimentary)</skos:definition>
		<skos:prefLabel xml:lang="fr"
			>matériel sédimentaire enrichie en matière
						organique</skos:prefLabel>
		<skos:prefLabel xml:lang="it"
			>materiale sedimentario arricchito di materia organica </skos:prefLabel>
		<skos:prefLabel xml:lang="en">organic rich sedimentary material</skos:prefLabel>
		<skos:inScheme rdf:resource="urn:cgi:classifierScheme:CGI:SimpleLithology:2008"/>
		<skos:broader
			rdf:resource="urn:cgi:classifier:CGI:SimpleLithology:2008:sedimentary_material"/>
	</skos:Concept>
	<skos:Concept
		rdf:about="urn:cgi:classifier:CGI:SimpleLithology:2008:organic_rich_sedimentary_rock">
		<skos:inScheme rdf:resource="urn:cgi:classifierScheme:CGI:SimpleLithology:2008"/>
		<skos:definition>Sedimentary rock with color, composition, texture and apparent density indicating greater than 50 percent organic content by weight on a moisture-free basis. (NADM SLTT sedimentary)</skos:definition>
		<skos:prefLabel xml:lang="fr"
			>roche sédimentaire enrichie en matière organique</skos:prefLabel>
		<skos:prefLabel xml:lang="it">roccia sedimentaria ricca di materia organica</skos:prefLabel>
		<skos:prefLabel xml:lang="en">organic rich sedimentary rock</skos:prefLabel>
		<skos:inScheme rdf:resource="urn:cgi:classifierScheme:CGI:SimpleLithology:2008"/>
		<skos:broader rdf:resource="urn:cgi:classifier:CGI:SimpleLithology:2008:sedimentary_rock"/>
	</skos:Concept>
	<skos:Concept rdf:about="urn:cgi:classifier:CGI:SimpleLithology:2008:packstone">
		<skos:inScheme rdf:resource="urn:cgi:classifierScheme:CGI:SimpleLithology:2008"/>
		<skos:definition>Carbonate sedimentary rock with discernible grain supported depositional texture, containing greater than 10 percent grains; intergranular spaces are filled by matrix. (Hallsworth and Knox 1999)</skos:definition>
		<skos:prefLabel xml:lang="fr">packstone</skos:prefLabel>
		<skos:prefLabel xml:lang="it">packstone</skos:prefLabel>
		<skos:prefLabel xml:lang="en">packstone</skos:prefLabel>
		<skos:inScheme rdf:resource="urn:cgi:classifierScheme:CGI:SimpleLithology:2008"/>
		<skos:broader
			rdf:resource="urn:cgi:classifier:CGI:SimpleLithology:2008:carbonate_sedimentary_rock"/>
	</skos:Concept>
	<skos:Concept rdf:about="urn:cgi:classifier:CGI:SimpleLithology:2008:peat">
		<skos:inScheme rdf:resource="urn:cgi:classifierScheme:CGI:SimpleLithology:2008"/>
		<skos:definition>Unconsolidated organic-rich sediment composed of at least 50 percent semi-carbonised plant remains; individual remains commonly seen with unaided eye; yellowish brown to brownish black; generally fibrous texture; can be plastic or friable. In its natural state it can be readily cut and has a very high moisture content, generally greater than 90 percent. (Hallsworth and Knox 1999)</skos:definition>
		<skos:prefLabel xml:lang="fr">tourbe</skos:prefLabel>
		<skos:prefLabel xml:lang="it">torba</skos:prefLabel>
		<skos:prefLabel xml:lang="en">peat</skos:prefLabel>
		<skos:inScheme rdf:resource="urn:cgi:classifierScheme:CGI:SimpleLithology:2008"/>
		<skos:broader
			rdf:resource="urn:cgi:classifier:CGI:SimpleLithology:2008:organic_rich_sediment"/>
	</skos:Concept>
	<skos:Concept rdf:about="urn:cgi:classifier:CGI:SimpleLithology:2008:pegmatite">
		<skos:inScheme rdf:resource="urn:cgi:classifierScheme:CGI:SimpleLithology:2008"/>
		<skos:definition>Exceptionally coarse grained crystalline rock with interlocking crystals; most grains are 1cm or more diameter; composition is generally that of granite, but the term may refer to the coarse grained facies of any type of igneous rock;usually found as irregular dikes, lenses, or veins associated with plutons or batholiths. (Neuendorf et al. 2005)</skos:definition>
		<skos:prefLabel xml:lang="fr">pegmatite</skos:prefLabel>
		<skos:prefLabel xml:lang="it">pegmatite</skos:prefLabel>
		<skos:prefLabel xml:lang="en">pegmatite</skos:prefLabel>
		<skos:inScheme rdf:resource="urn:cgi:classifierScheme:CGI:SimpleLithology:2008"/>
		<skos:broader
			rdf:resource="urn:cgi:classifier:CGI:SimpleLithology:2008:phaneritic_igneous_rock"/>
	</skos:Concept>
	<skos:Concept rdf:about="urn:cgi:classifier:CGI:SimpleLithology:2008:peridotite">
		<skos:inScheme rdf:resource="urn:cgi:classifierScheme:CGI:SimpleLithology:2008"/>
		<skos:definition>Ultramafic rock consisting of more than 40 percent (by volume) olivine with pyroxene and/or amphibole and little or no feldspar. Commonly altered to serpentinite. Includes rocks defined modally in the ultramafic rock classification as dunite, harzburgite, lherzolite, wehrlite, olivinite, pyroxene peridotite, pyroxene hornblende peridotite or hornblende peridotite. (LeMaitre et al. 2002)</skos:definition>
		<skos:prefLabel xml:lang="fr">péridotites</skos:prefLabel>
		<skos:prefLabel xml:lang="it">peridotite</skos:prefLabel>
		<skos:prefLabel xml:lang="en">peridotite</skos:prefLabel>
		<skos:inScheme rdf:resource="urn:cgi:classifierScheme:CGI:SimpleLithology:2008"/>
		<skos:broader
			rdf:resource="urn:cgi:classifier:CGI:SimpleLithology:2008:ultrabasic_igneous_rock"/>
	</skos:Concept>
	<skos:Concept rdf:about="urn:cgi:classifier:CGI:SimpleLithology:2008:phaneritic_igneous_rock">
		<skos:inScheme rdf:resource="urn:cgi:classifierScheme:CGI:SimpleLithology:2008"/>
		<skos:definition>Igneous rock in which greater than 10 percent of rock is individual crystals that can be discerned with the unaided eye. Bounding grain size is on the order of 32 to 100 microns. Igneous rocks with 'exotic' composition are excluded from this concept. (Neuendorf et al. 2005)</skos:definition>
		<skos:prefLabel xml:lang="fr">roche ignée phanéritique</skos:prefLabel>
		<skos:prefLabel xml:lang="it">roccia ignea faneritica</skos:prefLabel>
		<skos:prefLabel xml:lang="en">phaneritic igneous rock</skos:prefLabel>
		<skos:inScheme rdf:resource="urn:cgi:classifierScheme:CGI:SimpleLithology:2008"/>
		<skos:broader rdf:resource="urn:cgi:classifier:CGI:SimpleLithology:2008:igneous_rock"/>
	</skos:Concept>
	<skos:Concept rdf:about="urn:cgi:classifier:CGI:SimpleLithology:2008:phonolitic_rock">
		<skos:inScheme rdf:resource="urn:cgi:classifierScheme:CGI:SimpleLithology:2008"/>
		<skos:definition>Fine grained igneous rock containing feldspathoids and in which alkali feldspar is thought to be more abundant than plagioclase. Includes rocks defined modally in QAPF fields 11 and 12, and TAS field Ph. (LeMaitre et al. 2002)</skos:definition>
		<skos:prefLabel xml:lang="fr">phonolites</skos:prefLabel>
		<skos:prefLabel xml:lang="it">fonolite</skos:prefLabel>
		<skos:prefLabel xml:lang="en">phonolitic rock</skos:prefLabel>
		<skos:inScheme rdf:resource="urn:cgi:classifierScheme:CGI:SimpleLithology:2008"/>
		<skos:broader
			rdf:resource="urn:cgi:classifier:CGI:SimpleLithology:2008:fine_grained_igneous_rock"/>
	</skos:Concept>
	<skos:Concept
		rdf:about="urn:cgi:classifier:CGI:SimpleLithology:2008:phosphate_rich_sedimentary_material">
		<skos:inScheme rdf:resource="urn:cgi:classifierScheme:CGI:SimpleLithology:2008"/>
		<skos:definition>Sedimentary material in which at least 50 percent of the primary and/or recrystallized constituents are phosphate minerals. (NGMDB 2008)</skos:definition>
		<skos:prefLabel xml:lang="fr">matériel sédimentaire phosphaté</skos:prefLabel>
		<skos:prefLabel xml:lang="it">materiale sedimentario ricco di fosfati</skos:prefLabel>
		<skos:prefLabel xml:lang="en">phosphate rich sedimentary material</skos:prefLabel>
		<skos:inScheme rdf:resource="urn:cgi:classifierScheme:CGI:SimpleLithology:2008"/>
		<skos:broader
			rdf:resource="urn:cgi:classifier:CGI:SimpleLithology:2008:sedimentary_material"/>
	</skos:Concept>
	<skos:Concept rdf:about="urn:cgi:classifier:CGI:SimpleLithology:2008:phosphatic_sediment">
		<skos:inScheme rdf:resource="urn:cgi:classifierScheme:CGI:SimpleLithology:2008"/>
		<skos:definition>Sediment in which at least 50 percent of the primary and/or recrystallized constituents are phosphate minerals. (NGMDB 2008)</skos:definition>
		<skos:prefLabel xml:lang="fr">sédiment phosphaté</skos:prefLabel>
		<skos:prefLabel xml:lang="it">sedimento fosfatico</skos:prefLabel>
		<skos:prefLabel xml:lang="en">phosphatic sediment</skos:prefLabel>
		<skos:inScheme rdf:resource="urn:cgi:classifierScheme:CGI:SimpleLithology:2008"/>
		<skos:broader rdf:resource="urn:cgi:classifier:CGI:SimpleLithology:2008:sediment"/>
	</skos:Concept>
	<skos:Concept rdf:about="urn:cgi:classifier:CGI:SimpleLithology:2008:phosphorite">
		<skos:inScheme rdf:resource="urn:cgi:classifierScheme:CGI:SimpleLithology:2008"/>
		<skos:definition>Sedimentary rock in which at least 50 percent of the primary or recrystallized constituents are phosphate minerals. Most commonly occurs as a bedded primary or reworked secondary marine rock, composed of microcrystalline carbonate fluorapatite in the form of lamina, pellets, oolites and nodules, and skeletal, shell and bone fragments. (HallsworthandKnox 1999, Jackson 1997)</skos:definition>
		<skos:prefLabel xml:lang="fr">phosphorite</skos:prefLabel>
		<skos:prefLabel xml:lang="it">fosforite</skos:prefLabel>
		<skos:prefLabel xml:lang="en">phosphorite</skos:prefLabel>
		<skos:inScheme rdf:resource="urn:cgi:classifierScheme:CGI:SimpleLithology:2008"/>
		<skos:broader rdf:resource="urn:cgi:classifier:CGI:SimpleLithology:2008:sedimentary_rock"/>
	</skos:Concept>
	<skos:Concept rdf:about="urn:cgi:classifier:CGI:SimpleLithology:2008:phyllite">
		<skos:inScheme rdf:resource="urn:cgi:classifierScheme:CGI:SimpleLithology:2008"/>
		<skos:definition>Rock with a well developed, continuous schistosity, an average grain size between 0.1 and 0.5 millimeters, and a silvery sheen on cleavage surfaces. Individual phyllosilicate grains are barely visible with the unaided eye. (IUGS SCMR 2007 (http://www.bgs.ac.uk/SCMR/))</skos:definition>
		<skos:prefLabel xml:lang="fr">phyllite</skos:prefLabel>
		<skos:prefLabel xml:lang="it">fillade</skos:prefLabel>
		<skos:prefLabel xml:lang="en">phyllite</skos:prefLabel>
		<skos:inScheme rdf:resource="urn:cgi:classifierScheme:CGI:SimpleLithology:2008"/>
		<skos:broader
			rdf:resource="urn:cgi:classifier:CGI:SimpleLithology:2008:foliated_metamorphic_rock"/>
	</skos:Concept>
	<skos:Concept rdf:about="urn:cgi:classifier:CGI:SimpleLithology:2008:phyllonite">
		<skos:inScheme rdf:resource="urn:cgi:classifierScheme:CGI:SimpleLithology:2008"/>
		<skos:definition>Mylonitic rock composed largely of fine-grained mica that imparts a sheen to foliation surfaces; may have flaser lamination, isoclinal folding, and deformed veins, which indicate significant shearing. Macroscopically resembles phyllite, but formed by mechanical degradation of initially coarser rock. (NADM metamorphic rock vocabulary SLTTm1.0; Marshak and Mitra 1988)</skos:definition>
		<skos:prefLabel xml:lang="fr">phyllonite</skos:prefLabel>
		<skos:prefLabel xml:lang="it">fillonite</skos:prefLabel>
		<skos:prefLabel xml:lang="en">phyllonite</skos:prefLabel>
		<skos:inScheme rdf:resource="urn:cgi:classifierScheme:CGI:SimpleLithology:2008"/>
		<skos:broader rdf:resource="urn:cgi:classifier:CGI:SimpleLithology:2008:mylonitic_rock"/>
	</skos:Concept>
	<skos:Concept rdf:about="urn:cgi:classifier:CGI:SimpleLithology:2008:porphyry">
		<skos:inScheme rdf:resource="urn:cgi:classifierScheme:CGI:SimpleLithology:2008"/>
		<skos:definition>Igneous rock that contains conspicuous phenocrysts in a finer grained groundmass; groundmass itself may be phaneritic or fine-grained. (LeMaitre et al. 2002)</skos:definition>
		<skos:prefLabel xml:lang="fr">porphyre</skos:prefLabel>
		<skos:prefLabel xml:lang="it">porfirite</skos:prefLabel>
		<skos:prefLabel xml:lang="en">porphyry</skos:prefLabel>
		<skos:inScheme rdf:resource="urn:cgi:classifierScheme:CGI:SimpleLithology:2008"/>
		<skos:broader rdf:resource="urn:cgi:classifier:CGI:SimpleLithology:2008:igneous_rock"/>
	</skos:Concept>
	<skos:Concept rdf:about="urn:cgi:classifier:CGI:SimpleLithology:2008:pyroclastic_material">
		<skos:inScheme rdf:resource="urn:cgi:classifierScheme:CGI:SimpleLithology:2008"/>
		<skos:definition>Fragmental igneous material that consists of more than 75 percent of particles formed by disruption as a direct result of volcanic action. (LeMaitre et al. 2002)</skos:definition>
		<skos:prefLabel xml:lang="fr">matériel pyroclastique</skos:prefLabel>
		<skos:prefLabel xml:lang="it">materiale piroclastico</skos:prefLabel>
		<skos:prefLabel xml:lang="en">pyroclastic material</skos:prefLabel>
		<skos:inScheme rdf:resource="urn:cgi:classifierScheme:CGI:SimpleLithology:2008"/>
		<skos:broader
			rdf:resource="urn:cgi:classifier:CGI:SimpleLithology:2008:fragmental_igneous_material"/>
	</skos:Concept>
	<skos:Concept rdf:about="urn:cgi:classifier:CGI:SimpleLithology:2008:pyroclastic_rock">
		<skos:inScheme rdf:resource="urn:cgi:classifierScheme:CGI:SimpleLithology:2008"/>
		<skos:definition>Fragmental igneous rock that consists of greater than 75 percent fragments produced as a direct result of eruption or extrusion of magma from within the earth onto its surface. Includes autobreccia associated with lava flows and excludes deposits reworked by epiclastic processes. ()</skos:definition>
		<skos:prefLabel xml:lang="fr">pyroclastites</skos:prefLabel>
		<skos:prefLabel xml:lang="it">piroclastite</skos:prefLabel>
		<skos:prefLabel xml:lang="en">pyroclastic rock</skos:prefLabel>
		<skos:inScheme rdf:resource="urn:cgi:classifierScheme:CGI:SimpleLithology:2008"/>
		<skos:broader
			rdf:resource="urn:cgi:classifier:CGI:SimpleLithology:2008:fragmental_igneous_rock"/>
	</skos:Concept>
	<skos:Concept rdf:about="urn:cgi:classifier:CGI:SimpleLithology:2008:pyroxenite">
		<skos:inScheme rdf:resource="urn:cgi:classifierScheme:CGI:SimpleLithology:2008"/>
		<skos:definition>Ultramafic phaneritic igneous rock composed almost entirely of one or more pyroxenes and occasionally biotite, hornblende and olivine. Includes rocks defined modally in the ultramafic rock classification as olivine pyroxenite, olivine-hornblende pyroxenite, pyroxenite, orthopyroxenite, clinopyroxenite and websterite. (LeMaitre et al. 2002)</skos:definition>
		<skos:prefLabel xml:lang="fr">pyroxénite</skos:prefLabel>
		<skos:prefLabel xml:lang="it">pirossenite</skos:prefLabel>
		<skos:prefLabel xml:lang="en">pyroxenite</skos:prefLabel>
		<skos:inScheme rdf:resource="urn:cgi:classifierScheme:CGI:SimpleLithology:2008"/>
		<skos:broader
			rdf:resource="urn:cgi:classifier:CGI:SimpleLithology:2008:ultrabasic_igneous_rock"/>
	</skos:Concept>
	<skos:Concept
		rdf:about="urn:cgi:classifier:CGI:SimpleLithology:2008:quartz_rich_phaneritic_igneous_rock">
		<skos:inScheme rdf:resource="urn:cgi:classifierScheme:CGI:SimpleLithology:2008"/>
		<skos:definition>Phaneritic crystalline igneous rock that contains greater than 60 percent quartz. (Gillespie and Styles 1999; LeMaitre et al. 2002)</skos:definition>
		<skos:prefLabel xml:lang="fr">roche ignée quartzique phanéritique </skos:prefLabel>
		<skos:prefLabel xml:lang="it">roccia ignea faneritica ricca in quarzo</skos:prefLabel>
		<skos:prefLabel xml:lang="en">quartz rich phaneritic igneous rock</skos:prefLabel>
		<skos:inScheme rdf:resource="urn:cgi:classifierScheme:CGI:SimpleLithology:2008"/>
		<skos:broader
			rdf:resource="urn:cgi:classifier:CGI:SimpleLithology:2008:phaneritic_igneous_rock"/>
	</skos:Concept>
	<skos:Concept rdf:about="urn:cgi:classifier:CGI:SimpleLithology:2008:quartzite">
		<skos:inScheme rdf:resource="urn:cgi:classifierScheme:CGI:SimpleLithology:2008"/>
		<skos:definition>Metamorphic rock consisting of greater than or equal to 75 percent quartz; typically granoblastic texture. (after Neuendorf et al. 2005)</skos:definition>
		<skos:prefLabel xml:lang="fr">quartzites</skos:prefLabel>
		<skos:prefLabel xml:lang="it">quarzite</skos:prefLabel>
		<skos:prefLabel xml:lang="en">quartzite</skos:prefLabel>
		<skos:inScheme rdf:resource="urn:cgi:classifierScheme:CGI:SimpleLithology:2008"/>
		<skos:broader rdf:resource="urn:cgi:classifier:CGI:SimpleLithology:2008:metamorphic_rock"/>
	</skos:Concept>
	<skos:Concept rdf:about="urn:cgi:classifier:CGI:SimpleLithology:2008:rhyolitic_rock">
		<skos:inScheme rdf:resource="urn:cgi:classifierScheme:CGI:SimpleLithology:2008"/>
		<skos:definition>Fine-grained igneous rock, typically porphyritic, consisting of quartz and alkali feldspar (often as phenocrysts), with minor plagioclase and biotite, in a microcrystalline, cryptocrystalline or glassy groundmass. Flow texture is common. Includes rocks defined modally in QAPF fields 2 and 3 or chemically in TAS Field R as rhyolite. (LeMaitre et al. 2002)</skos:definition>
		<skos:prefLabel xml:lang="fr">rhyolites</skos:prefLabel>
		<skos:prefLabel xml:lang="it">riolite</skos:prefLabel>
		<skos:prefLabel xml:lang="en">rhyolitic rock</skos:prefLabel>
		<skos:inScheme rdf:resource="urn:cgi:classifierScheme:CGI:SimpleLithology:2008"/>
		<skos:broader
			rdf:resource="urn:cgi:classifier:CGI:SimpleLithology:2008:fine_grained_igneous_rock"/>
	</skos:Concept>
	<skos:Concept rdf:about="urn:cgi:classifier:CGI:SimpleLithology:2008:rock">
		<skos:inScheme rdf:resource="urn:cgi:classifierScheme:CGI:SimpleLithology:2008"/>
		<skos:definition>Consolidated aggregate of one or more EarthMaterials, or a body of undifferentiated mineral matter, or of solid organic material. Includes mineral aggregates such as granite, shale, marble; glassy matter such as obsidian; and organic material such a coal. Excludes unconsolidated materials. (Jackson, 1997; NADM C1 2004; Neuendorf et al 2005)</skos:definition>
		<skos:prefLabel xml:lang="fr">roche</skos:prefLabel>
		<skos:prefLabel xml:lang="it">roccia</skos:prefLabel>
		<skos:prefLabel xml:lang="en">rock</skos:prefLabel>
		<skos:inScheme rdf:resource="urn:cgi:classifierScheme:CGI:SimpleLithology:2008"/>
		<skos:broader rdf:resource="urn:cgi:classifier:CGI:SimpleLithology:2008:compound_material"/>
	</skos:Concept>
	<skos:Concept rdf:about="urn:cgi:classifier:CGI:SimpleLithology:2008:sand">
		<skos:inScheme rdf:resource="urn:cgi:classifierScheme:CGI:SimpleLithology:2008"/>
		<skos:definition>Clastic sediment in which less than 30 percent of particles are gravel (greater than 2 mm in diameter) and the sand to mud ratio is at least 1. (Neuendorf et al. 2005; NGMDB)</skos:definition>
		<skos:prefLabel xml:lang="fr">sables</skos:prefLabel>
		<skos:prefLabel xml:lang="it">sabbia</skos:prefLabel>
		<skos:prefLabel xml:lang="en">sand</skos:prefLabel>
		<skos:inScheme rdf:resource="urn:cgi:classifierScheme:CGI:SimpleLithology:2008"/>
		<skos:broader rdf:resource="urn:cgi:classifier:CGI:SimpleLithology:2008:clastic_sediment"/>
	</skos:Concept>
	<skos:Concept rdf:about="urn:cgi:classifier:CGI:SimpleLithology:2008:sandstone">
		<skos:inScheme rdf:resource="urn:cgi:classifierScheme:CGI:SimpleLithology:2008"/>
		<skos:definition>Clastic sedimentary rock in which less than 30 percent of particles are greater than 2 mm in diameter (gravel) and the sand to mud ratio is at least 1. (NGMDB; Neuendorf et al. 2005; particle size from Wentworth grade scale)</skos:definition>
		<skos:prefLabel xml:lang="fr">grès</skos:prefLabel>
		<skos:prefLabel xml:lang="it">arenaria</skos:prefLabel>
		<skos:prefLabel xml:lang="en">sandstone</skos:prefLabel>
		<skos:inScheme rdf:resource="urn:cgi:classifierScheme:CGI:SimpleLithology:2008"/>
		<skos:broader
			rdf:resource="urn:cgi:classifier:CGI:SimpleLithology:2008:clastic_sedimentary_rock"/>
	</skos:Concept>
	<skos:Concept rdf:about="urn:cgi:classifier:CGI:SimpleLithology:2008:schist">
		<skos:inScheme rdf:resource="urn:cgi:classifierScheme:CGI:SimpleLithology:2008"/>
		<skos:definition>Foliated phaneritic metamorphic rock with well developed, continuous schistosity (greater than 50 percent of mineral grains with a tabular, lamellar, or prismatic crystallographic habit that are oriented in a continuous planar or linear fabric). (NADM metamorphic rock vocabulary SLTTm1.0; Neuendorf et al. 2005)</skos:definition>
		<skos:prefLabel xml:lang="fr">schistes</skos:prefLabel>
		<skos:prefLabel xml:lang="it">scisto</skos:prefLabel>
		<skos:prefLabel xml:lang="en">schist</skos:prefLabel>
		<skos:inScheme rdf:resource="urn:cgi:classifierScheme:CGI:SimpleLithology:2008"/>
		<skos:broader
			rdf:resource="urn:cgi:classifier:CGI:SimpleLithology:2008:foliated_metamorphic_rock"/>
	</skos:Concept>
	<skos:Concept rdf:about="urn:cgi:classifier:CGI:SimpleLithology:2008:sediment">
		<skos:inScheme rdf:resource="urn:cgi:classifierScheme:CGI:SimpleLithology:2008"/>
		<skos:definition>Unconsolidated material consisting of an aggregation of particles transported or deposited by air, water or ice, or that accumulated by other natural agents, such as chemical precipitation, and that forms in layers on the Earth's surface. Includes epiclastic deposits. (NADM SLTT sedimentary)</skos:definition>
		<skos:prefLabel xml:lang="fr">sédiments</skos:prefLabel>
		<skos:prefLabel xml:lang="it">sedimento</skos:prefLabel>
		<skos:prefLabel xml:lang="en">sediment</skos:prefLabel>
		<skos:inScheme rdf:resource="urn:cgi:classifierScheme:CGI:SimpleLithology:2008"/>
		<skos:broader
			rdf:resource="urn:cgi:classifier:CGI:SimpleLithology:2008:unconsolidated_material"/>
	</skos:Concept>
	<skos:Concept rdf:about="urn:cgi:classifier:CGI:SimpleLithology:2008:sedimentary_material">
		<skos:inScheme rdf:resource="urn:cgi:classifierScheme:CGI:SimpleLithology:2008"/>
		<skos:definition>Material formed by accumulation of solid fragmental material deposited by air, water or ice, or material that accumulated by other natural agents such as chemical precipitation from solution or secretion by organisms. Includes both sediment and sedimentary rock. Includes epiclastic deposits. (SLTTs [2004])</skos:definition>
		<skos:prefLabel xml:lang="fr">matériel sédimentaire</skos:prefLabel>
		<skos:prefLabel xml:lang="it">materiale sedimentario</skos:prefLabel>
		<skos:prefLabel xml:lang="en">sedimentary material</skos:prefLabel>
		<skos:inScheme rdf:resource="urn:cgi:classifierScheme:CGI:SimpleLithology:2008"/>
		<skos:broader rdf:resource="urn:cgi:classifier:CGI:SimpleLithology:2008:compound_material"/>
	</skos:Concept>
	<skos:Concept rdf:about="urn:cgi:classifier:CGI:SimpleLithology:2008:sedimentary_rock">
		<skos:inScheme rdf:resource="urn:cgi:classifierScheme:CGI:SimpleLithology:2008"/>
		<skos:definition>Rock formed by accumulation and cementation of solid fragmental material deposited by air, water or ice, or as a result of other natural agents, such as precipitation from solution, the accumulation of organic material, or from biogenic processes, including secretion by organisms. Includes epiclastic deposits. (SLTTs [2004])</skos:definition>
		<skos:prefLabel xml:lang="fr">roche sédimentaire</skos:prefLabel>
		<skos:prefLabel xml:lang="it">roccia sedimentaria</skos:prefLabel>
		<skos:prefLabel xml:lang="en">sedimentary rock</skos:prefLabel>
		<skos:inScheme rdf:resource="urn:cgi:classifierScheme:CGI:SimpleLithology:2008"/>
		<skos:broader rdf:resource="urn:cgi:classifier:CGI:SimpleLithology:2008:rock"/>
	</skos:Concept>
	<skos:Concept rdf:about="urn:cgi:classifier:CGI:SimpleLithology:2008:serpentinite">
		<skos:inScheme rdf:resource="urn:cgi:classifierScheme:CGI:SimpleLithology:2008"/>
		<skos:definition>Rock consisting of more than 75 percent serpentine-group minerals, eg. antigorite, chrysotile or lizardite; accessory chlorite, talc and magnetite may be present; derived from hydration of ferromagnesian silicate minerals such as olivine and pyroxene. (Neuendorf et al. 2005)</skos:definition>
		<skos:prefLabel xml:lang="fr">serpentinites</skos:prefLabel>
		<skos:prefLabel xml:lang="it">serpentinite</skos:prefLabel>
		<skos:prefLabel xml:lang="en">serpentinite</skos:prefLabel>
		<skos:inScheme rdf:resource="urn:cgi:classifierScheme:CGI:SimpleLithology:2008"/>
		<skos:broader rdf:resource="urn:cgi:classifier:CGI:SimpleLithology:2008:metamorphic_rock"/>
	</skos:Concept>
	<skos:Concept rdf:about="urn:cgi:classifier:CGI:SimpleLithology:2008:shale">
		<skos:inScheme rdf:resource="urn:cgi:classifierScheme:CGI:SimpleLithology:2008"/>
		<skos:definition>Laminated mudstone that will part or break along thin, closely spaced layers parallel to stratification. (NADM SLTT sedimentary; Neuendorf et al. 2005)</skos:definition>
		<skos:prefLabel xml:lang="fr">shale</skos:prefLabel>
		<skos:prefLabel xml:lang="it">argillite o scisto</skos:prefLabel>
		<skos:prefLabel xml:lang="en">shale</skos:prefLabel>
		<skos:inScheme rdf:resource="urn:cgi:classifierScheme:CGI:SimpleLithology:2008"/>
		<skos:broader rdf:resource="urn:cgi:classifier:CGI:SimpleLithology:2008:mudstone"/>
	</skos:Concept>
	<skos:Concept rdf:about="urn:cgi:classifier:CGI:SimpleLithology:2008:slate">
		<skos:inScheme rdf:resource="urn:cgi:classifierScheme:CGI:SimpleLithology:2008"/>
		<skos:definition>Compact, fine grained rock with an average grain size less than 0.032 millimeter and a well developed schistosity (slaty cleavage), and hence can be split into slabs or thin plates. (NADM metamorphic rock vocabulary SLTTm1.0; Neuendorf et al. 2005)</skos:definition>
		<skos:prefLabel xml:lang="fr">ardoise</skos:prefLabel>
		<skos:prefLabel xml:lang="it">ardesia</skos:prefLabel>
		<skos:prefLabel xml:lang="en">slate</skos:prefLabel>
		<skos:inScheme rdf:resource="urn:cgi:classifierScheme:CGI:SimpleLithology:2008"/>
		<skos:broader
			rdf:resource="urn:cgi:classifier:CGI:SimpleLithology:2008:foliated_metamorphic_rock"/>
	</skos:Concept>
	<skos:Concept rdf:about="urn:cgi:classifier:CGI:SimpleLithology:2008:syenite">
		<skos:inScheme rdf:resource="urn:cgi:classifierScheme:CGI:SimpleLithology:2008"/>
		<skos:definition>Coarse grained crystalline rock consisting mainly of alkali feldspar with subordinate sodic plagioclase, biotite, pyroxene, amphibole and occasional fayalite; minor quartz or nepheline may be present. Defined modally in QAPF Field 7. ()</skos:definition>
		<skos:prefLabel xml:lang="fr">syénite</skos:prefLabel>
		<skos:prefLabel xml:lang="it">sienite</skos:prefLabel>
		<skos:prefLabel xml:lang="en">syenite</skos:prefLabel>
		<skos:inScheme rdf:resource="urn:cgi:classifierScheme:CGI:SimpleLithology:2008"/>
		<skos:broader rdf:resource="urn:cgi:classifier:CGI:SimpleLithology:2008:compound_material"/>
	</skos:Concept>
	<skos:Concept rdf:about="urn:cgi:classifier:CGI:SimpleLithology:2008:syenitic_rock">
		<skos:inScheme rdf:resource="urn:cgi:classifierScheme:CGI:SimpleLithology:2008"/>
		<skos:definition>Phaneritic crystalline igneous rock with M less than 90, consisting mainly of alkali feldspar and plagioclase; minor quartz or nepheline may be present, along with pyroxene, amphibole or biotite. Includes rocks classified in QAPF fields 6, 7 and 8 as syenite or monzonite. (LeMaitre et al. 2002)</skos:definition>
		<skos:prefLabel xml:lang="fr">syénite</skos:prefLabel>
		<skos:prefLabel xml:lang="it">roccia sienitica</skos:prefLabel>
		<skos:prefLabel xml:lang="en">syenitic rock</skos:prefLabel>
		<skos:inScheme rdf:resource="urn:cgi:classifierScheme:CGI:SimpleLithology:2008"/>
		<skos:broader
			rdf:resource="urn:cgi:classifier:CGI:SimpleLithology:2008:phaneritic_igneous_rock"/>
	</skos:Concept>
	<skos:Concept rdf:about="urn:cgi:classifier:CGI:SimpleLithology:2008:tephra">
		<skos:inScheme rdf:resource="urn:cgi:classifierScheme:CGI:SimpleLithology:2008"/>
		<skos:definition>Unconsolidated pyroclastic material in which greater than 75 percent of the fragments are deposited as a direct result of volcanic processes and the deposit has not been reworked by epiclastic processes. Includes ash, lapilli tephra, bomb tephra, block tephra and unconsolidated agglomerate. (Hallsworth and Knox 1999; LeMaitre et al. 2002)</skos:definition>
		<skos:prefLabel xml:lang="fr">téphra</skos:prefLabel>
		<skos:prefLabel xml:lang="it">tefra</skos:prefLabel>
		<skos:prefLabel xml:lang="en">tephra</skos:prefLabel>
		<skos:inScheme rdf:resource="urn:cgi:classifierScheme:CGI:SimpleLithology:2008"/>
		<skos:broader
			rdf:resource="urn:cgi:classifier:CGI:SimpleLithology:2008:pyroclastic_material"/>
	</skos:Concept>
	<skos:Concept rdf:about="urn:cgi:classifier:CGI:SimpleLithology:2008:tephritic_rock">
		<skos:inScheme rdf:resource="urn:cgi:classifierScheme:CGI:SimpleLithology:2008"/>
		<skos:definition>Fine grained crystalline igneous rock containing essential feldspathoids and in which plagioclase is more abundant than alkali feldspar. Includes rocks classified in QAPF field 14 or chemically in TAS field U1 as basanite or tephrite. (LeMaitre et al. 2002)</skos:definition>
		<skos:prefLabel xml:lang="fr">téphrites</skos:prefLabel>
		<skos:prefLabel xml:lang="it">roccia tefritica</skos:prefLabel>
		<skos:prefLabel xml:lang="en">tephritic rock</skos:prefLabel>
		<skos:inScheme rdf:resource="urn:cgi:classifierScheme:CGI:SimpleLithology:2008"/>
		<skos:broader
			rdf:resource="urn:cgi:classifier:CGI:SimpleLithology:2008:fine_grained_igneous_rock"/>
	</skos:Concept>
	<skos:Concept rdf:about="urn:cgi:classifier:CGI:SimpleLithology:2008:tonalite">
		<skos:inScheme rdf:resource="urn:cgi:classifierScheme:CGI:SimpleLithology:2008"/>
		<skos:definition>Phaneritic crystalline rock consisting of quartz and intermediate plagioclase, usually with biotite and amphibole. Includes rocks defined modally in QAPF field 5. (LeMaitre et al. 2002)</skos:definition>
		<skos:prefLabel xml:lang="fr">tonalites</skos:prefLabel>
		<skos:prefLabel xml:lang="it">tonalite</skos:prefLabel>
		<skos:prefLabel xml:lang="en">tonalite</skos:prefLabel>
		<skos:inScheme rdf:resource="urn:cgi:classifierScheme:CGI:SimpleLithology:2008"/>
		<skos:broader
			rdf:resource="urn:cgi:classifier:CGI:SimpleLithology:2008:phaneritic_igneous_rock"/>
	</skos:Concept>
	<skos:Concept rdf:about="urn:cgi:classifier:CGI:SimpleLithology:2008:trachytic_rock">
		<skos:inScheme rdf:resource="urn:cgi:classifierScheme:CGI:SimpleLithology:2008"/>
		<skos:definition>Fine-grained volcanic rock consisting of alkali feldspar and minor mafic minerals, typically amphibole or mica; typically porphyritic. Includes rocks defined modally in QAPF fields 6, 7 and 8 or chemically in TAS Field T as trachyte or latite. (LeMaitre et al. 2002)</skos:definition>
		<skos:prefLabel xml:lang="fr">trachytes</skos:prefLabel>
		<skos:prefLabel xml:lang="it">trachite</skos:prefLabel>
		<skos:prefLabel xml:lang="en">trachytic rock</skos:prefLabel>
		<skos:inScheme rdf:resource="urn:cgi:classifierScheme:CGI:SimpleLithology:2008"/>
		<skos:broader
			rdf:resource="urn:cgi:classifier:CGI:SimpleLithology:2008:fine_grained_igneous_rock"/>
	</skos:Concept>
	<skos:Concept
		rdf:about="urn:cgi:classifier:CGI:SimpleLithology:2008:tuff_breccia_agglomerate_or_pyroclastic_breccia">
		<skos:inScheme rdf:resource="urn:cgi:classifierScheme:CGI:SimpleLithology:2008"/>
		<skos:definition>Pyroclastic rock in which greater than 25 percent of particles are greater than 64 mm in largest dimension. Includes agglomerate, pyroclastic breccia of Gillespie and Styles (1999) (Schmid 1981; LeMaitre et al. 2002)</skos:definition>
		<skos:prefLabel xml:lang="fr"
			>brèche tuffacée, agglomérat, ou brêche
						pyroclastique</skos:prefLabel>
		<skos:prefLabel xml:lang="it"
			>tufo a blocchi agglomerato, breccia piroclastica</skos:prefLabel>
		<skos:prefLabel xml:lang="en"
			>tuff-breccia, agglomerate, or pyroclastic breccia</skos:prefLabel>
		<skos:inScheme rdf:resource="urn:cgi:classifierScheme:CGI:SimpleLithology:2008"/>
		<skos:broader rdf:resource="urn:cgi:classifier:CGI:SimpleLithology:2008:pyroclastic_rock"/>
	</skos:Concept>
	<skos:Concept rdf:about="urn:cgi:classifier:CGI:SimpleLithology:2008:ultrabasic_igneous_rock">
		<skos:inScheme rdf:resource="urn:cgi:classifierScheme:CGI:SimpleLithology:2008"/>
		<skos:definition>Igneous rock with less than 45 percent SiO2. (after LeMaitre et al. 2002)</skos:definition>
		<skos:prefLabel xml:lang="fr">roche ignée ultrabasique</skos:prefLabel>
		<skos:prefLabel xml:lang="it">roccia ignea ultrabasica</skos:prefLabel>
		<skos:prefLabel xml:lang="en">ultrabasic igneous rock</skos:prefLabel>
		<skos:inScheme rdf:resource="urn:cgi:classifierScheme:CGI:SimpleLithology:2008"/>
		<skos:broader rdf:resource="urn:cgi:classifier:CGI:SimpleLithology:2008:igneous_rock"/>
	</skos:Concept>
	<skos:Concept rdf:about="urn:cgi:classifier:CGI:SimpleLithology:2008:unconsolidated_material">
		<skos:inScheme rdf:resource="urn:cgi:classifierScheme:CGI:SimpleLithology:2008"/>
		<skos:definition>CompoundMaterial composed of an aggregation of particles that do not adhere to each other strongly enough that the aggregate can be considered a solid in its own right. (NGMDB)</skos:definition>
		<skos:prefLabel xml:lang="fr">matériel non consolidé</skos:prefLabel>
		<skos:prefLabel xml:lang="it">materiale non consolidato</skos:prefLabel>
		<skos:prefLabel xml:lang="en">unconsolidated material</skos:prefLabel>
		<skos:inScheme rdf:resource="urn:cgi:classifierScheme:CGI:SimpleLithology:2008"/>
		<skos:broader rdf:resource="urn:cgi:classifier:CGI:SimpleLithology:2008:compound_material"/>
	</skos:Concept>
	<skos:Concept rdf:about="urn:cgi:classifier:CGI:SimpleLithology:2008:wackestone">
		<skos:inScheme rdf:resource="urn:cgi:classifierScheme:CGI:SimpleLithology:2008"/>
		<skos:definition>Sandstone that contains between 15 and 75 percent matrix of unspecified origin. (CGI concepts task group)</skos:definition>
		<skos:prefLabel xml:lang="fr">wackestone</skos:prefLabel>
		<skos:prefLabel xml:lang="it">wackestone</skos:prefLabel>
		<skos:prefLabel xml:lang="en">wackestone</skos:prefLabel>
		<skos:inScheme rdf:resource="urn:cgi:classifierScheme:CGI:SimpleLithology:2008"/>
		<skos:broader rdf:resource="urn:cgi:classifier:CGI:SimpleLithology:2008:sandstone"/>
	</skos:Concept>
	<skos:Concept rdf:about="urn:cgi:classifier:CGI:SimpleLithology:2008:compound_material">
		<skos:inScheme rdf:resource="urn:cgi:classifierScheme:CGI:SimpleLithology:2008"/>
		<skos:definition>An Earth Material composed of an aggregation of particles of Earth Material, possibly including other Compound Materials. This is 'top' of lithology category hierarchy, and should be used to indicate 'any rock or unconsolidated material'.</skos:definition>
		<skos:prefLabel xml:lang="en">compound material</skos:prefLabel>
		<skos:inScheme rdf:resource="urn:cgi:classifierScheme:CGI:SimpleLithology:2008"/>
	</skos:Concept>
</rdf:RDF>
