<?xml version="1.0" encoding="UTF-8"?>
<rdf:RDF xmlns:gml="http://www.opengis.net/gml" xmlns:gsml="urn:cgi:xmlns:CGI:GeoSciML:2.0" xmlns:gsmlCC="http://geosciml.org/release/3.0_alpha/rdf/gsmlCC#" xmlns:owl="http://www.w3.org/2002/07/owl#" xmlns:rdf="http://www.w3.org/1999/02/22-rdf-syntax-ns#" xmlns:rdfs="http://www.w3.org/2000/01/rdf-schema#" xmlns:skos="http://www.w3.org/2004/02/skos/core#" xmlns:xlink="http://www.w3.org/1999/xlink">
	<owl:Ontology rdf:about="urn:cgi:classifierScheme:CGI:SimpleLithology:200811">
		<owl:imports rdf:resource="./GSMLControlledConceptSKOS.rdf"/>
	</owl:Ontology>
	<skos:ConceptScheme rdf:about="urn:cgi:classifierScheme:CGI:SimpleLithology:200811"/>
	<skos:Concept rdf:about="urn:cgi:classifierScheme:CGI:SimpleLithology:200811:compound_material">
		<skos:definition>An Earth Material composed of an aggregation of particles of Earth Material, possibly including other Compound Materials. This is 'top' of lithology category hierarchy, and should be used to indicate 'any rock or unconsolidated material'. Source: NADM C1, 2004</skos:definition>
		<skos:prefLabel xml:lang="en">Compound material</skos:prefLabel>
		<skos:inScheme rdf:resource="urn:cgi:classifierScheme:CGI:SimpleLithology:200811"/>
	</skos:Concept>
	<skos:Concept rdf:about="urn:cgi:classifierScheme:CGI:SimpleLithology:200811:breccia">
		<skos:definition>Coarse-grained material composed of angular broken rock fragments; the fragments typically have sharp edges and unworn corners. The fragments may be held together by a mineral cement, or in a fine-grained matrix. Clasts may be of any composition or origin. Source: Neuendorf et al. 2005</skos:definition>
		<skos:prefLabel xml:lang="en">Breccia</skos:prefLabel>
		<skos:prefLabel xml:lang="fr">brèches</skos:prefLabel>
		<skos:prefLabel xml:lang="it">breccia</skos:prefLabel>
		<skos:inScheme rdf:resource="urn:cgi:classifierScheme:CGI:SimpleLithology:200811"/>
		<skos:broader rdf:resource="urn:cgi:classifierScheme:CGI:SimpleLithology:200811:compound_material"/>
	</skos:Concept>
	<skos:Concept rdf:about="urn:cgi:classifierScheme:CGI:SimpleLithology:200811:composite_genesis_material">
		<skos:definition>Material of unspecified consolidation state formed by geological modification of pre-existing materials outside the realm of igneous and sedimentary processes. Includes rocks formed by impact metamorphism, standard dynamothermal metamorphism, brittle deformation, weathering, metasomatism and hydrothermal alteration (diagenesis is a sedimentary process in this context). Source: SLTTm 2004</skos:definition>
		<skos:prefLabel xml:lang="en">Composite genesis material</skos:prefLabel>
		<skos:prefLabel xml:lang="fr">matériel modifié et/ou transformé</skos:prefLabel>
		<skos:prefLabel xml:lang="it">materiale modificato o trasformato</skos:prefLabel>
		<skos:inScheme rdf:resource="urn:cgi:classifierScheme:CGI:SimpleLithology:200811"/>
		<skos:broader rdf:resource="urn:cgi:classifierScheme:CGI:SimpleLithology:200811:compound_material"/>
	</skos:Concept>
	<skos:Concept rdf:about="urn:cgi:classifierScheme:CGI:SimpleLithology:200811:fault_related_material">
		<skos:definition>Material formed as a result brittle faulting, composed of greater than 10 percent matrix; matrix is fine-grained material caused by tectonic grainsize reduction. Includes cohesive (cataclasite series) and non-cohesive (breccia-gouge series) material. Source: this vocabulary; SLTTm 2004</skos:definition>
		<skos:prefLabel xml:lang="en">Fault-related material</skos:prefLabel>
		<skos:prefLabel xml:lang="fr">brèches de faille</skos:prefLabel>
		<skos:prefLabel xml:lang="it">breccia di faglia</skos:prefLabel>
		<skos:inScheme rdf:resource="urn:cgi:classifierScheme:CGI:SimpleLithology:200811"/>
	</skos:Concept>
	<skos:Concept rdf:about="urn:cgi:classifierScheme:CGI:SimpleLithology:200811:breccia_gouge_series">
		<skos:definition>Fault material with features such as void spaces (filled or unfilled), or unconsolidated matrix material between fragments, indicating loss of cohesion during deformation. Includes fault-related breccia and gouge. Source: SLTTm 2004</skos:definition>
		<skos:prefLabel xml:lang="en">Breccia-gouge series</skos:prefLabel>
		<skos:prefLabel xml:lang="fr">brèche de faille</skos:prefLabel>
		<skos:prefLabel xml:lang="it">breccia di faglia</skos:prefLabel>
		<skos:inScheme rdf:resource="urn:cgi:classifierScheme:CGI:SimpleLithology:200811"/>
		<skos:broader rdf:resource="urn:cgi:classifierScheme:CGI:SimpleLithology:200811:fault_related_material"/>
	</skos:Concept>
	<skos:Concept rdf:about="urn:cgi:classifierScheme:CGI:SimpleLithology:200811:cataclasite_series">
		<skos:definition>Fault-related rock that maintained primary cohesion during deformation, with matrix comprising 50 to 90 percent of rock mass; matrix is fine-grained material caused by tectonic grainsize reduction. Includes cataclasite, protocataclasite and ultracataclasite. Source: Sibson, 1977; Scholz, 1990; Snoke and Tullis, 1998; Barker, 1998 Appendix II; NADM SLTTm, 2004</skos:definition>
		<skos:prefLabel xml:lang="en">Cataclasite series</skos:prefLabel>
		<skos:prefLabel xml:lang="fr">cataclasites</skos:prefLabel>
		<skos:prefLabel xml:lang="it">cataclasite</skos:prefLabel>
		<skos:inScheme rdf:resource="urn:cgi:classifierScheme:CGI:SimpleLithology:200811"/>
	</skos:Concept>
	<skos:Concept rdf:about="urn:cgi:classifierScheme:CGI:SimpleLithology:200811:duricrust">
		<skos:definition>Rock forming a hard crust or layer at or near the Earth's surface at the time of formation, e.g. in the upper horizons of a soil, characterized by structures indicative of pedogenic origin. Source: this vocabulary</skos:definition>
		<skos:prefLabel xml:lang="en">Duricrust</skos:prefLabel>
		<skos:prefLabel xml:lang="fr">calcrète</skos:prefLabel>
		<skos:prefLabel xml:lang="it">duricrust (o orizzonte indurito)</skos:prefLabel>
		<skos:inScheme rdf:resource="urn:cgi:classifierScheme:CGI:SimpleLithology:200811"/>
	</skos:Concept>
	<skos:Concept rdf:about="urn:cgi:classifierScheme:CGI:SimpleLithology:200811:bauxite">
		<skos:definition>Highly aluminous material containing abundant aluminium hydroxides (gibbsite, less commonly boehmite, diaspore) and aluminium-substituted iron oxides or hydroxides and generally minor or negligible kaolin minerals; may contain up to 20 percent quartz. Commonly has a pisolitic or nodular texture, and may be cemented. Source: Eggleton, 2001</skos:definition>
		<skos:prefLabel xml:lang="en">Bauxite</skos:prefLabel>
		<skos:prefLabel xml:lang="fr">bauxite</skos:prefLabel>
		<skos:prefLabel xml:lang="it">bauxite</skos:prefLabel>
		<skos:inScheme rdf:resource="urn:cgi:classifierScheme:CGI:SimpleLithology:200811"/>
		<skos:broader rdf:resource="urn:cgi:classifierScheme:CGI:SimpleLithology:200811:composite_genesis_material"/>
	</skos:Concept>
	<skos:Concept rdf:about="urn:cgi:classifierScheme:CGI:SimpleLithology:200811:anthropogenic_unconsolidated_material">
		<skos:definition>Unconsolidated material known to have artificial (human-related) origin. Source: this vocabulary</skos:definition>
		<skos:prefLabel xml:lang="en">Anthropogenic unconsolidated material</skos:prefLabel>
		<skos:prefLabel xml:lang="fr">marériel anthropique non consolidé</skos:prefLabel>
		<skos:prefLabel xml:lang="it">materiale antropico non consolidato</skos:prefLabel>
		<skos:inScheme rdf:resource="urn:cgi:classifierScheme:CGI:SimpleLithology:200811"/>
	</skos:Concept>
	<skos:Concept rdf:about="urn:cgi:classifierScheme:CGI:SimpleLithology:200811:unconsolidated_material">
		<skos:definition>CompoundMaterial composed of an aggregation of particles that do not adhere to each other strongly enough that the aggregate can be considered a solid in its own right. Source: NGMDB</skos:definition>
		<skos:prefLabel xml:lang="en">Unconsolidated material</skos:prefLabel>
		<skos:prefLabel xml:lang="fr">matériel non consolidé</skos:prefLabel>
		<skos:prefLabel xml:lang="it">materiale non consolidato</skos:prefLabel>
		<skos:inScheme rdf:resource="urn:cgi:classifierScheme:CGI:SimpleLithology:200811"/>
		<skos:broader rdf:resource="urn:cgi:classifierScheme:CGI:SimpleLithology:200811:compound_material"/>
	</skos:Concept>
	<skos:Concept rdf:about="urn:cgi:classifierScheme:CGI:SimpleLithology:200811:natural_unconsolidated_material">
		<skos:definition>Unconsolidated material known to have natural, ie. not human-made, origin. Source: this vocabulary</skos:definition>
		<skos:prefLabel xml:lang="en">Natural unconsolidated material</skos:prefLabel>
		<skos:prefLabel xml:lang="fr">matériel naturel non consolidé</skos:prefLabel>
		<skos:prefLabel xml:lang="it">materiale naturale non consolidato</skos:prefLabel>
		<skos:inScheme rdf:resource="urn:cgi:classifierScheme:CGI:SimpleLithology:200811"/>
	</skos:Concept>
	<skos:Concept rdf:about="urn:cgi:classifierScheme:CGI:SimpleLithology:200811:sediment">
		<skos:definition>Unconsolidated material consisting of an aggregation of particles transported or deposited by air, water or ice, or that accumulated by other natural agents, such as chemical precipitation, and that forms in layers on the Earth's surface. Includes epiclastic deposits. Source: SLTTs 2004</skos:definition>
		<skos:prefLabel xml:lang="en">Sediment</skos:prefLabel>
		<skos:prefLabel xml:lang="fr">sédiments</skos:prefLabel>
		<skos:prefLabel xml:lang="it">sedimento</skos:prefLabel>
		<skos:inScheme rdf:resource="urn:cgi:classifierScheme:CGI:SimpleLithology:200811"/>
	</skos:Concept>
	<skos:Concept rdf:about="urn:cgi:classifierScheme:CGI:SimpleLithology:200811:clastic_sediment">
		<skos:definition>Sediment in which at least 50 percent of the constituent particles were derived from erosion, weathering, or mass-wasting of pre-existing earth materials, and transported to the place of deposition by mechanical agents such as water, wind, ice and gravity. Source: SLTTs, 2004; Neuendorf et al., 2005</skos:definition>
		<skos:prefLabel xml:lang="en">Clastic sediment</skos:prefLabel>
		<skos:prefLabel xml:lang="fr">sédiment clastique</skos:prefLabel>
		<skos:prefLabel xml:lang="it">sedimento clastico</skos:prefLabel>
		<skos:inScheme rdf:resource="urn:cgi:classifierScheme:CGI:SimpleLithology:200811"/>
	</skos:Concept>
	<skos:Concept rdf:about="urn:cgi:classifierScheme:CGI:SimpleLithology:200811:diamicton">
		<skos:definition>Unsorted or poorly sorted, clastic sediment with a wide range of particle sizes such that it cannot be assigned to any other class. Source: Fairbridge and Bourgeois 1978</skos:definition>
		<skos:prefLabel xml:lang="en">Diamicton</skos:prefLabel>
		<skos:prefLabel xml:lang="fr">diamictite</skos:prefLabel>
		<skos:prefLabel xml:lang="it">diamicton</skos:prefLabel>
		<skos:inScheme rdf:resource="urn:cgi:classifierScheme:CGI:SimpleLithology:200811"/>
	</skos:Concept>
	<skos:Concept rdf:about="urn:cgi:classifierScheme:CGI:SimpleLithology:200811:gravel">
		<skos:definition>Sediment containing greater than 30 percent gravel-size particles (greater than 2.0 mm diameter). Source: SLTTs 2004</skos:definition>
		<skos:prefLabel xml:lang="en">Gravel</skos:prefLabel>
		<skos:prefLabel xml:lang="fr">graviers</skos:prefLabel>
		<skos:prefLabel xml:lang="it">ghiaia</skos:prefLabel>
		<skos:inScheme rdf:resource="urn:cgi:classifierScheme:CGI:SimpleLithology:200811"/>
	</skos:Concept>
	<skos:Concept rdf:about="urn:cgi:classifierScheme:CGI:SimpleLithology:200811:sand">
		<skos:definition>Clastic sediment in which less than 30 percent of particles are gravel (greater than 2 mm in diameter) and the sand to mud ratio is at least 1. Source: Neuendorf et al. 2005; NGMDB</skos:definition>
		<skos:prefLabel xml:lang="en">Sand</skos:prefLabel>
		<skos:prefLabel xml:lang="fr">sables</skos:prefLabel>
		<skos:prefLabel xml:lang="it">sabbia</skos:prefLabel>
		<skos:inScheme rdf:resource="urn:cgi:classifierScheme:CGI:SimpleLithology:200811"/>
	</skos:Concept>
	<skos:Concept rdf:about="urn:cgi:classifierScheme:CGI:SimpleLithology:200811:mud">
		<skos:definition>Clastic sediment consisting of less than 30 percent gravel-size (2 mm) particles and with a mud to sand ratio greater than 1. Clasts may be of any composition or origin. Source: based on SLTTs 2004; Neuendorf et al. 2005; particle size from Wentworth grade scale</skos:definition>
		<skos:prefLabel xml:lang="en">Mud</skos:prefLabel>
		<skos:prefLabel xml:lang="fr">boue </skos:prefLabel>
		<skos:prefLabel xml:lang="it">fango</skos:prefLabel>
		<skos:inScheme rdf:resource="urn:cgi:classifierScheme:CGI:SimpleLithology:200811"/>
	</skos:Concept>
	<skos:Concept rdf:about="urn:cgi:classifierScheme:CGI:SimpleLithology:200811:chemical_sediment">
		<skos:definition>Sediment that consists of at least 50 percent material produced by chemical (organic or inorganic) processes within the basin of deposition. Includes organic-rich, non-clastic siliceous, carbonate, evaporite, iron-rich, and phosphatic sediment classes. Source: SLTTs 2004</skos:definition>
		<skos:prefLabel xml:lang="en">Chemical sediment</skos:prefLabel>
		<skos:prefLabel xml:lang="fr">sédiment chimique</skos:prefLabel>
		<skos:prefLabel xml:lang="it">sedimento chimico</skos:prefLabel>
		<skos:inScheme rdf:resource="urn:cgi:classifierScheme:CGI:SimpleLithology:200811"/>
	</skos:Concept>
	<skos:Concept rdf:about="urn:cgi:classifierScheme:CGI:SimpleLithology:200811:biogenic_sediment">
		<skos:definition>Sediment composed of greater than 50 percent material of biogenic origin. Source: SLTTs 2004</skos:definition>
		<skos:prefLabel xml:lang="en">Biogenic sediment</skos:prefLabel>
		<skos:prefLabel xml:lang="fr">sédiment biogénique</skos:prefLabel>
		<skos:prefLabel xml:lang="it">sedimento biogenico</skos:prefLabel>
		<skos:inScheme rdf:resource="urn:cgi:classifierScheme:CGI:SimpleLithology:200811"/>
	</skos:Concept>
	<skos:Concept rdf:about="urn:cgi:classifierScheme:CGI:SimpleLithology:200811:ooze">
		<skos:definition>Mud with a sand to mud ratio less than 1 to 9 that contains at least 30 percent skeletal remains of pelagic organisms. Less than 1 percent gravel and less than 50 percent carbonate minerals. Source: based on Bates and Jackson 1987 &amp; Hallsworth &amp; Knox 1999</skos:definition>
		<skos:prefLabel xml:lang="en">Ooze</skos:prefLabel>
		<skos:prefLabel xml:lang="fr">vases</skos:prefLabel>
		<skos:prefLabel xml:lang="it">ooze</skos:prefLabel>
		<skos:inScheme rdf:resource="urn:cgi:classifierScheme:CGI:SimpleLithology:200811"/>
	</skos:Concept>
	<skos:Concept rdf:about="urn:cgi:classifierScheme:CGI:SimpleLithology:200811:iron_rich_sediment">
		<skos:definition>Sediment that consists of at least 50 percent iron-bearing minerals (hematite, magnetite, limonite-group, siderite, iron-sulfides), as determined by hand-lens or petrographic analysis. Corresponds to a rock typically containing 15 percent iron by weight. Source: SLTTs 2004</skos:definition>
		<skos:prefLabel xml:lang="en">Iron rich sediment</skos:prefLabel>
		<skos:prefLabel xml:lang="fr">sédiment ferrugineux</skos:prefLabel>
		<skos:prefLabel xml:lang="it">sedimento ferrifero</skos:prefLabel>
		<skos:inScheme rdf:resource="urn:cgi:classifierScheme:CGI:SimpleLithology:200811"/>
	</skos:Concept>
	<skos:Concept rdf:about="urn:cgi:classifierScheme:CGI:SimpleLithology:200811:phosphatic_sediment">
		<skos:definition>Sediment in which at least 50 percent of the primary and/or recrystallized constituents are phosphate minerals. Source: SLTTs 2004</skos:definition>
		<skos:prefLabel xml:lang="en">Phosphatic sediment</skos:prefLabel>
		<skos:prefLabel xml:lang="fr">sédiment phosphaté</skos:prefLabel>
		<skos:prefLabel xml:lang="it">sedimento fosfatico</skos:prefLabel>
		<skos:inScheme rdf:resource="urn:cgi:classifierScheme:CGI:SimpleLithology:200811"/>
	</skos:Concept>
	<skos:Concept rdf:about="urn:cgi:classifierScheme:CGI:SimpleLithology:200811:non_clastic_siliceous_sediment">
		<skos:definition>Sediment that consists of at least 50 percent silicate mineral material, deposited directly by chemical or biological processes at the depositional surface, or in particles formed by chemical or biological processes within the basin of deposition. Source: NGMDB 2008; Hallsworth and Knox 1999</skos:definition>
		<skos:prefLabel xml:lang="en">Non-clastic siliceous sediment</skos:prefLabel>
		<skos:prefLabel xml:lang="fr">sédiment siliceux non-clastique</skos:prefLabel>
		<skos:prefLabel xml:lang="it">sedimento siliceo non clastico</skos:prefLabel>
		<skos:inScheme rdf:resource="urn:cgi:classifierScheme:CGI:SimpleLithology:200811"/>
	</skos:Concept>
	<skos:Concept rdf:about="urn:cgi:classifierScheme:CGI:SimpleLithology:200811:organic_rich_sediment">
		<skos:definition>Sediment with color, composition, texture and apparent density indicating greater than 50 percent organic content by weight on a moisture-free basis. Source: SLTTs 2004</skos:definition>
		<skos:prefLabel xml:lang="en">Organic rich sediment</skos:prefLabel>
		<skos:prefLabel xml:lang="fr">sédiment enrichie en matière organique</skos:prefLabel>
		<skos:prefLabel xml:lang="it">sedimento arricchito di materia organica</skos:prefLabel>
		<skos:inScheme rdf:resource="urn:cgi:classifierScheme:CGI:SimpleLithology:200811"/>
	</skos:Concept>
	<skos:Concept rdf:about="urn:cgi:classifierScheme:CGI:SimpleLithology:200811:peat">
		<skos:definition>Unconsolidated organic-rich sediment composed of at least 50 percent semi-carbonised plant remains; individual remains commonly seen with unaided eye; yellowish brown to brownish black; generally fibrous texture; can be plastic or friable. In its natural state it can be readily cut and has a very high moisture content, generally greater than 90 percent. Source: Hallsworth &amp; Knox 1999</skos:definition>
		<skos:prefLabel xml:lang="en">Peat</skos:prefLabel>
		<skos:prefLabel xml:lang="fr">tourbe</skos:prefLabel>
		<skos:prefLabel xml:lang="it">torba</skos:prefLabel>
		<skos:inScheme rdf:resource="urn:cgi:classifierScheme:CGI:SimpleLithology:200811"/>
	</skos:Concept>
	<skos:Concept rdf:about="urn:cgi:classifierScheme:CGI:SimpleLithology:200811:carbonate_sediment">
		<skos:definition>Sediment in which at least 50 percent of the primary and/or recrystallized constituents are composed of one (or more) of the carbonate minerals calcite, aragonite and dolomite, in particles of intrabasinal origin. Source: SLTTs 2004</skos:definition>
		<skos:prefLabel xml:lang="en">Carbonate sediment</skos:prefLabel>
		<skos:prefLabel xml:lang="fr">sédiment carbonaté</skos:prefLabel>
		<skos:prefLabel xml:lang="it">sedimento carbonatico</skos:prefLabel>
		<skos:inScheme rdf:resource="urn:cgi:classifierScheme:CGI:SimpleLithology:200811"/>
	</skos:Concept>
	<skos:Concept rdf:about="urn:cgi:classifierScheme:CGI:SimpleLithology:200811:dolomitic_sediment">
		<skos:definition>Carbonate sediment with a ratio of magnesium carbonate to calcite (plus aragonite) greater than 1 to 1. Source: after SLTTs 2004, Hallsworth and Knox 1999</skos:definition>
		<skos:prefLabel xml:lang="en">Dolomitic sediment</skos:prefLabel>
		<skos:prefLabel xml:lang="fr">sédiment dolomitique</skos:prefLabel>
		<skos:prefLabel xml:lang="it">sedimento dolomitico</skos:prefLabel>
		<skos:inScheme rdf:resource="urn:cgi:classifierScheme:CGI:SimpleLithology:200811"/>
	</skos:Concept>
	<skos:Concept rdf:about="urn:cgi:classifierScheme:CGI:SimpleLithology:200811:calcareous_carbonate_sediment">
		<skos:definition>Carbonate sediment with a calcite (plus aragonite) to dolomite ratio greater than 1 to 1. Includes lime-sediments. Source: after Hallsworth &amp; Knox 1999</skos:definition>
		<skos:prefLabel xml:lang="en">Calcareous carbonate sediment</skos:prefLabel>
		<skos:prefLabel xml:lang="fr">sédiment carbonaté calcaire</skos:prefLabel>
		<skos:prefLabel xml:lang="it">sedimento calcareo carbonatico</skos:prefLabel>
		<skos:inScheme rdf:resource="urn:cgi:classifierScheme:CGI:SimpleLithology:200811"/>
	</skos:Concept>
	<skos:Concept rdf:about="urn:cgi:classifierScheme:CGI:SimpleLithology:200811:carbonate_gravel">
		<skos:definition>Carbonate sediment composed of more than 25 percent gravel-sized clasts (maximum diameter more than 2 mm). Source: Hallsworth &amp; Knox 1999</skos:definition>
		<skos:prefLabel xml:lang="en">Carbonate gravel</skos:prefLabel>
		<skos:prefLabel xml:lang="fr">gravier carbonaté</skos:prefLabel>
		<skos:prefLabel xml:lang="it">ghiaia calcarea</skos:prefLabel>
		<skos:inScheme rdf:resource="urn:cgi:classifierScheme:CGI:SimpleLithology:200811"/>
	</skos:Concept>
	<skos:Concept rdf:about="urn:cgi:classifierScheme:CGI:SimpleLithology:200811:carbonate_sand">
		<skos:definition>Carbonate sediment composed of more than 75 percent sand-sized clasts (maximum diameter between 32 microns and 2 mm). Source: Hallsworth &amp; Knox 1999</skos:definition>
		<skos:prefLabel xml:lang="en">Carbonate sand</skos:prefLabel>
		<skos:prefLabel xml:lang="fr">sable carbonaté</skos:prefLabel>
		<skos:prefLabel xml:lang="it">sabbia calcarea</skos:prefLabel>
		<skos:inScheme rdf:resource="urn:cgi:classifierScheme:CGI:SimpleLithology:200811"/>
	</skos:Concept>
	<skos:Concept rdf:about="urn:cgi:classifierScheme:CGI:SimpleLithology:200811:carbonate_mud">
		<skos:definition>Carbonate sediment composed of more than 75 percent mud-sized clasts (maximum diameter less than 32 microns). Source: Hallsworth &amp; Knox 1999</skos:definition>
		<skos:prefLabel xml:lang="en">Carbonate mud</skos:prefLabel>
		<skos:prefLabel xml:lang="fr">boue carbonatée</skos:prefLabel>
		<skos:prefLabel xml:lang="it">fango calcareo</skos:prefLabel>
		<skos:inScheme rdf:resource="urn:cgi:classifierScheme:CGI:SimpleLithology:200811"/>
	</skos:Concept>
	<skos:Concept rdf:about="urn:cgi:classifierScheme:CGI:SimpleLithology:200811:tephra">
		<skos:definition>Unconsolidated pyroclastic material in which greater than 75 percent of the fragments are deposited as a direct result of volcanic processes and the deposit has not been reworked by epiclastic processes. Includes ash, lapilli tephra, bomb tephra, block tephra and unconsolidated agglomerate. Source: Hallsworth &amp; Knox 1999; LeMaitre et al. 2002</skos:definition>
		<skos:prefLabel xml:lang="en">Tephra</skos:prefLabel>
		<skos:prefLabel xml:lang="fr">téphra</skos:prefLabel>
		<skos:prefLabel xml:lang="it">tefra</skos:prefLabel>
		<skos:inScheme rdf:resource="urn:cgi:classifierScheme:CGI:SimpleLithology:200811"/>
	</skos:Concept>
	<skos:Concept rdf:about="urn:cgi:classifierScheme:CGI:SimpleLithology:200811:ash_and_lapilli">
		<skos:definition>Tephra in which less than 25 percent of fragments are greater than 64 mm in longest dimension Source: Schmid 1981; LeMaitre et al. 2002</skos:definition>
		<skos:prefLabel xml:lang="en">Ash and lapilli</skos:prefLabel>
		<skos:prefLabel xml:lang="fr">cendre et lapilli</skos:prefLabel>
		<skos:prefLabel xml:lang="it">cenere e lapilli</skos:prefLabel>
		<skos:inScheme rdf:resource="urn:cgi:classifierScheme:CGI:SimpleLithology:200811"/>
	</skos:Concept>
	<skos:Concept rdf:about="urn:cgi:classifierScheme:CGI:SimpleLithology:200811:ash_breccia_bomb_or_block_tephra">
		<skos:definition>Tephra in which more than 25 percent of particles are greater than 64 mm in largest dimension. Includes ash breccia, bomb tephra and block tephra of Gillespie and Styles (1999) Source: Schmid 1981; LeMaitre et al. 2002</skos:definition>
		<skos:prefLabel xml:lang="en">Ash breccia, bomb, or block tephra</skos:prefLabel>
		<skos:prefLabel xml:lang="fr">brèche cendreuse , bombe, ou bloques de téphra</skos:prefLabel>
		<skos:prefLabel xml:lang="it">tephra a brecce cineritiche, a bombe vulcaniche, a blocchi</skos:prefLabel>
		<skos:inScheme rdf:resource="urn:cgi:classifierScheme:CGI:SimpleLithology:200811"/>
	</skos:Concept>
	<skos:Concept rdf:about="urn:cgi:classifierScheme:CGI:SimpleLithology:200811:rock">
		<skos:definition>Consolidated aggregate of one or more EarthMaterials, or a body of undifferentiated mineral matter, or of solid organic material. Includes mineral aggregates such as granite, shale, marble; glassy matter such as obsidian; and organic material such a coal. Excludes unconsolidated materials. Source: Jackson, 1997; NADM C1 2004; Neuendorf et al 2005</skos:definition>
		<skos:prefLabel xml:lang="en">Rock</skos:prefLabel>
		<skos:prefLabel xml:lang="fr">roche</skos:prefLabel>
		<skos:prefLabel xml:lang="it">roccia</skos:prefLabel>
		<skos:inScheme rdf:resource="urn:cgi:classifierScheme:CGI:SimpleLithology:200811"/>
		<skos:broader rdf:resource="urn:cgi:classifierScheme:CGI:SimpleLithology:200811:compound_material"/>
	</skos:Concept>
	<skos:Concept rdf:about="urn:cgi:classifierScheme:CGI:SimpleLithology:200811:aphanite">
		<skos:definition>Rock that is too fine grained to categorize in more detail. Source: this vocabulary</skos:definition>
		<skos:prefLabel xml:lang="en">Aphanite</skos:prefLabel>
		<skos:prefLabel xml:lang="fr">roche aphanitique</skos:prefLabel>
		<skos:prefLabel xml:lang="it">roccia afanitica</skos:prefLabel>
		<skos:inScheme rdf:resource="urn:cgi:classifierScheme:CGI:SimpleLithology:200811"/>
	</skos:Concept>
	<skos:Concept rdf:about="urn:cgi:classifierScheme:CGI:SimpleLithology:200811:igneous_rock">
		<skos:definition>Rock formed as a result of igneous processes, for example intrusion and cooling of magma in the crust, or volcanic eruption. Source: Neuendorf et al 2005</skos:definition>
		<skos:prefLabel xml:lang="en">Igneous rock</skos:prefLabel>
		<skos:prefLabel xml:lang="fr">roche ignée</skos:prefLabel>
		<skos:prefLabel xml:lang="it">roccia ignea</skos:prefLabel>
		<skos:inScheme rdf:resource="urn:cgi:classifierScheme:CGI:SimpleLithology:200811"/>
	</skos:Concept>
	<skos:Concept rdf:about="urn:cgi:classifierScheme:CGI:SimpleLithology:200811:glassy_igneous_rock">
		<skos:definition>Igneous rock that consists of greater than 90 percent glass. Source: This vocabulary</skos:definition>
		<skos:prefLabel xml:lang="en">Glassy igneous rock</skos:prefLabel>
		<skos:prefLabel xml:lang="fr">roche ignée vitreuse</skos:prefLabel>
		<skos:prefLabel xml:lang="it">roccia ignea vetrosa</skos:prefLabel>
		<skos:inScheme rdf:resource="urn:cgi:classifierScheme:CGI:SimpleLithology:200811"/>
	</skos:Concept>
	<skos:Concept rdf:about="urn:cgi:classifierScheme:CGI:SimpleLithology:200811:exotic_composition_igneous_rock">
		<skos:definition>Rock with 'exotic' mineralogical, textural or field setting characteristics; typically dark colored, with abundant phenocrysts. Criteria include: presence of greater than 10 percent melilite or leucite; presence of kalsilite; greater than 50 percent carbonate minerals. Source: Gillespie and Styles 1999; LeMaitre et al. 2002</skos:definition>
		<skos:prefLabel xml:lang="en">Exotic composition igneous rock</skos:prefLabel>
		<skos:prefLabel xml:lang="fr">roche ignée de composition exotique</skos:prefLabel>
		<skos:prefLabel xml:lang="it">roccia ignea a composizione esotica</skos:prefLabel>
		<skos:inScheme rdf:resource="urn:cgi:classifierScheme:CGI:SimpleLithology:200811"/>
	</skos:Concept>
	<skos:Concept rdf:about="urn:cgi:classifierScheme:CGI:SimpleLithology:200811:exotic_alkaline_rock">
		<skos:definition>Kimberlite, lamproite, or lamprophyre. Generally are potassic, mafic or ultramafic rocks. Olivine (commonly serpentinized in kimberlite), and phlogopite are significant constituents. Source: based on LeMaitre et al. 2002</skos:definition>
		<skos:prefLabel xml:lang="en">Exotic alkaline rock</skos:prefLabel>
		<skos:prefLabel xml:lang="fr">roche exotique alcaline </skos:prefLabel>
		<skos:prefLabel xml:lang="it">roccia esotica alcalina</skos:prefLabel>
		<skos:inScheme rdf:resource="urn:cgi:classifierScheme:CGI:SimpleLithology:200811"/>
	</skos:Concept>
	<skos:Concept rdf:about="urn:cgi:classifierScheme:CGI:SimpleLithology:200811:exotic_alkalic_igneous_rock">
		<skos:definition>Igneous rock containing greater than 10 percent melilite or kalsilite. Typically undersaturated, ultrapotassic (kalsilitic rocks) or calcium-rich (melilitic rocks) mafic or ultramafic rocks. Source: based on LeMaitre et al. 2002</skos:definition>
		<skos:prefLabel xml:lang="en">Exotic alkalic igneous rock</skos:prefLabel>
		<skos:prefLabel xml:lang="fr">roche ignée exotique alcaline</skos:prefLabel>
		<skos:prefLabel xml:lang="it">roccia ignea esotica alcalina</skos:prefLabel>
		<skos:inScheme rdf:resource="urn:cgi:classifierScheme:CGI:SimpleLithology:200811"/>
	</skos:Concept>
	<skos:Concept rdf:about="urn:cgi:classifierScheme:CGI:SimpleLithology:200811:carbonatite">
		<skos:definition>Igneous rock composed of more than 50 percent modal carbonate minerals. Source: LeMaitre et al. 2002</skos:definition>
		<skos:prefLabel xml:lang="en">Carbonatite</skos:prefLabel>
		<skos:prefLabel xml:lang="fr">carbonatite</skos:prefLabel>
		<skos:prefLabel xml:lang="it">carbonatite</skos:prefLabel>
		<skos:inScheme rdf:resource="urn:cgi:classifierScheme:CGI:SimpleLithology:200811"/>
	</skos:Concept>
	<skos:Concept rdf:about="urn:cgi:classifierScheme:CGI:SimpleLithology:200811:ultrabasic_igneous_rock">
		<skos:definition>Igneous rock with less than 45 percent SiO2. Source: after LeMaitre et al. 2002</skos:definition>
		<skos:prefLabel xml:lang="en">Ultrabasic igneous rock</skos:prefLabel>
		<skos:prefLabel xml:lang="fr">roche ignée ultrabasique</skos:prefLabel>
		<skos:prefLabel xml:lang="it">roccia ignea ultrabasica</skos:prefLabel>
		<skos:inScheme rdf:resource="urn:cgi:classifierScheme:CGI:SimpleLithology:200811"/>
	</skos:Concept>
	<skos:Concept rdf:about="urn:cgi:classifierScheme:CGI:SimpleLithology:200811:hornblendite">
		<skos:definition>Ultramafic rock that consists of greater than 40 percent hornblende plus pyroxene and has a hornblende to pyroxene ratio greater than 1. Includes olivine hornblendite, olivine-pyroxene hornblendite, pyroxene hornblendite, and hornblendite. Source: LeMaitre et al. 2002</skos:definition>
		<skos:prefLabel xml:lang="en">Hornblendite</skos:prefLabel>
		<skos:prefLabel xml:lang="fr">hornblendite</skos:prefLabel>
		<skos:prefLabel xml:lang="it">hornblendite</skos:prefLabel>
		<skos:inScheme rdf:resource="urn:cgi:classifierScheme:CGI:SimpleLithology:200811"/>
	</skos:Concept>
	<skos:Concept rdf:about="urn:cgi:classifierScheme:CGI:SimpleLithology:200811:pyroxenite">
		<skos:definition>Ultramafic phaneritic igneous rock composed almost entirely of one or more pyroxenes and occasionally biotite, hornblende and olivine. Includes rocks defined modally in the ultramafic rock classification as olivine pyroxenite, olivine-hornblende pyroxenite, pyroxenite, orthopyroxenite, clinopyroxenite and websterite. Source: LeMaitre et al. 2002</skos:definition>
		<skos:prefLabel xml:lang="en">Pyroxenite</skos:prefLabel>
		<skos:prefLabel xml:lang="fr">pyroxénite</skos:prefLabel>
		<skos:prefLabel xml:lang="it">pirossenite</skos:prefLabel>
		<skos:inScheme rdf:resource="urn:cgi:classifierScheme:CGI:SimpleLithology:200811"/>
	</skos:Concept>
	<skos:Concept rdf:about="urn:cgi:classifierScheme:CGI:SimpleLithology:200811:komatiitic_rock">
		<skos:definition>Ultramafic volcanic rock, typically with spinifex texture of intergrown skeletal and bladed olivine and pyroxene crystals set in abundant glass. Includes picrite, komatiite and meimechite. Source: LeMaitre et al. 2002</skos:definition>
		<skos:prefLabel xml:lang="en">Komatiitic rock</skos:prefLabel>
		<skos:prefLabel xml:lang="fr">roche komatitique</skos:prefLabel>
		<skos:prefLabel xml:lang="it">komatiite</skos:prefLabel>
		<skos:inScheme rdf:resource="urn:cgi:classifierScheme:CGI:SimpleLithology:200811"/>
	</skos:Concept>
	<skos:Concept rdf:about="urn:cgi:classifierScheme:CGI:SimpleLithology:200811:peridotite">
		<skos:definition>Ultramafic rock consisting of more than 40 percent (by volume) olivine with pyroxene and/or amphibole and little or no feldspar. Commonly altered to serpentinite. Includes rocks defined modally in the ultramafic rock classification as dunite, harzburgite, lherzolite, wehrlite, olivinite, pyroxene peridotite, pyroxene hornblende peridotite or hornblende peridotite. Source: LeMaitre et al. 2002</skos:definition>
		<skos:prefLabel xml:lang="en">Peridotite</skos:prefLabel>
		<skos:prefLabel xml:lang="fr">péridotites</skos:prefLabel>
		<skos:prefLabel xml:lang="it">peridotite</skos:prefLabel>
		<skos:inScheme rdf:resource="urn:cgi:classifierScheme:CGI:SimpleLithology:200811"/>
	</skos:Concept>
	<skos:Concept rdf:about="urn:cgi:classifierScheme:CGI:SimpleLithology:200811:fragmental_igneous_rock">
		<skos:definition>Igneous rock in which greater than 75 percent of the rock consists of fragments produced as a result of igneous rock-forming process. Includes pyroclastic rocks, autobreccia associated with lava flows and intrusive breccias. Excludes deposits reworked by epiclastic processes. Source: NGMDB 2008</skos:definition>
		<skos:prefLabel xml:lang="en">Fragmental igneous rock</skos:prefLabel>
		<skos:prefLabel xml:lang="fr">roche ignée fragmentée</skos:prefLabel>
		<skos:prefLabel xml:lang="it">roccia ignea brecciata</skos:prefLabel>
		<skos:inScheme rdf:resource="urn:cgi:classifierScheme:CGI:SimpleLithology:200811"/>
	</skos:Concept>
	<skos:Concept rdf:about="urn:cgi:classifierScheme:CGI:SimpleLithology:200811:pyroclastic_rock">
		<skos:definition>Fragmental igneous rock that consists of greater than 75 percent fragments produced as a direct result of eruption or extrusion of magma from within the earth onto its surface. Includes autobreccia associated with lava flows and excludes deposits reworked by epiclastic processes. Source: based on LeMaitre et al. 2002</skos:definition>
		<skos:prefLabel xml:lang="en">Pyroclastic rock</skos:prefLabel>
		<skos:prefLabel xml:lang="fr">pyroclastites</skos:prefLabel>
		<skos:prefLabel xml:lang="it">piroclastite</skos:prefLabel>
		<skos:inScheme rdf:resource="urn:cgi:classifierScheme:CGI:SimpleLithology:200811"/>
	</skos:Concept>
	<skos:Concept rdf:about="urn:cgi:classifierScheme:CGI:SimpleLithology:200811:tuff_breccia_agglomerate_or_pyroclastic_breccia">
		<skos:definition>Pyroclastic rock in which greater than 25 percent of particles are greater than 64 mm in largest dimension. Includes agglomerate, pyroclastic breccia of Gillespie and Styles (1999) Source: Schmid 1981; LeMaitre et al. 2002</skos:definition>
		<skos:prefLabel xml:lang="en">Tuff-breccia, agglomerate, or pyroclastic breccia</skos:prefLabel>
		<skos:prefLabel xml:lang="fr">brèche tuffacée, agglomérat, ou brêche pyroclastique</skos:prefLabel>
		<skos:prefLabel xml:lang="it">tufo a blocchi agglomerato, breccia piroclastica</skos:prefLabel>
		<skos:inScheme rdf:resource="urn:cgi:classifierScheme:CGI:SimpleLithology:200811"/>
	</skos:Concept>
	<skos:Concept rdf:about="urn:cgi:classifierScheme:CGI:SimpleLithology:200811:ash_tuff_lapillistone_and_lapilli_tuff">
		<skos:definition>Pyroclastic rock in which less than 25 percent of rock by volume are more than 64 mm in longest diameter. Includes tuff, lapilli tuff, and lapillistone. Source: Schmid 1981; LeMaitre et al. 2002</skos:definition>
		<skos:prefLabel xml:lang="en">Ash tuff, lapillistone, and lapilli tuff</skos:prefLabel>
		<skos:prefLabel xml:lang="fr">cendre tuffacé, lapilli, et tuf lapillitique</skos:prefLabel>
		<skos:prefLabel xml:lang="it">tufo cineritico, tufo a lapilli</skos:prefLabel>
		<skos:inScheme rdf:resource="urn:cgi:classifierScheme:CGI:SimpleLithology:200811"/>
	</skos:Concept>
	<skos:Concept rdf:about="urn:cgi:classifierScheme:CGI:SimpleLithology:200811:phaneritic_igneous_rock">
		<skos:definition>Igneous rock in which greater than 10 percent of rock is individual crystals that can be discerned with the unaided eye. Bounding grain size is on the order of 32 to 100 microns. Igneous rocks with 'exotic' composition are excluded from this concept. Source: Neuendorf et al. 2005</skos:definition>
		<skos:prefLabel xml:lang="en">Phaneritic igneous rock</skos:prefLabel>
		<skos:prefLabel xml:lang="fr">roche ignée phanéritique</skos:prefLabel>
		<skos:prefLabel xml:lang="it">roccia ignea faneritica</skos:prefLabel>
		<skos:inScheme rdf:resource="urn:cgi:classifierScheme:CGI:SimpleLithology:200811"/>
	</skos:Concept>
	<skos:Concept rdf:about="urn:cgi:classifierScheme:CGI:SimpleLithology:200811:granitic_rock">
		<skos:definition>Phaneritic crystalline igneous rock consisting of quartz, alkali feldspar and/or plagioclase. Includes rocks defined modally in QAPF fields 2, 3, 4 and 5 as alkali granite, granite, granodiorite or tonalite. Source: LeMaitre et al. 2002</skos:definition>
		<skos:prefLabel xml:lang="en">Granitic rock</skos:prefLabel>
		<skos:prefLabel xml:lang="fr">granitoïdes</skos:prefLabel>
		<skos:prefLabel xml:lang="it">granitoide</skos:prefLabel>
		<skos:inScheme rdf:resource="urn:cgi:classifierScheme:CGI:SimpleLithology:200811"/>
	</skos:Concept>
	<skos:Concept rdf:about="urn:cgi:classifierScheme:CGI:SimpleLithology:200811:tonalite">
		<skos:definition>Phaneritic crystalline rock consisting of quartz and intermediate plagioclase, usually with biotite and amphibole. Includes rocks defined modally in QAPF field 5. Source: LeMaitre et al. 2002</skos:definition>
		<skos:prefLabel xml:lang="en">Tonalite</skos:prefLabel>
		<skos:prefLabel xml:lang="fr">tonalites</skos:prefLabel>
		<skos:prefLabel xml:lang="it">tonalite</skos:prefLabel>
		<skos:inScheme rdf:resource="urn:cgi:classifierScheme:CGI:SimpleLithology:200811"/>
	</skos:Concept>
	<skos:Concept rdf:about="urn:cgi:classifierScheme:CGI:SimpleLithology:200811:granite">
		<skos:definition>Phaneritic crystalline rock consisting of quartz, alkali feldspar and plagioclase (typically sodic) in variable amounts, usually with biotite and/or hornblende. Includes rocks defined modally in QAPF Field 3. Source: LeMaitre et al. 2002</skos:definition>
		<skos:prefLabel xml:lang="en">Granite</skos:prefLabel>
		<skos:prefLabel xml:lang="fr">granite</skos:prefLabel>
		<skos:prefLabel xml:lang="it">granito</skos:prefLabel>
		<skos:inScheme rdf:resource="urn:cgi:classifierScheme:CGI:SimpleLithology:200811"/>
	</skos:Concept>
	<skos:Concept rdf:about="urn:cgi:classifierScheme:CGI:SimpleLithology:200811:granodiorite">
		<skos:definition>Phaneritic crystalline rock consisting essentially of quartz, sodic plagioclase and lesser amounts of alkali feldspar with minor hornblende and biotite. Includes rocks defined modally in QAPF field 4. Source: LeMaitre et al. 2002</skos:definition>
		<skos:prefLabel xml:lang="en">Granodiorite</skos:prefLabel>
		<skos:prefLabel xml:lang="fr">granodiorites</skos:prefLabel>
		<skos:prefLabel xml:lang="it">granodiorite</skos:prefLabel>
		<skos:inScheme rdf:resource="urn:cgi:classifierScheme:CGI:SimpleLithology:200811"/>
	</skos:Concept>
	<skos:Concept rdf:about="urn:cgi:classifierScheme:CGI:SimpleLithology:200811:aplite">
		<skos:definition>Light coloured crystalline rock, characterized by a fine grained allotriomorphic-granular (aplitic, saccharoidal or xenomorphic) texture; typically granitic composition, consisting of quartz, K-feldspar and sodic plagioclase. Source: Neuendorf et al. 2005</skos:definition>
		<skos:prefLabel xml:lang="en">Aplite</skos:prefLabel>
		<skos:prefLabel xml:lang="fr">aplite</skos:prefLabel>
		<skos:prefLabel xml:lang="it">aplite</skos:prefLabel>
		<skos:inScheme rdf:resource="urn:cgi:classifierScheme:CGI:SimpleLithology:200811"/>
	</skos:Concept>
	<skos:Concept rdf:about="urn:cgi:classifierScheme:CGI:SimpleLithology:200811:syenitic_rock">
		<skos:definition>Phaneritic crystalline igneous rock with M less than 90, consisting mainly of alkali feldspar and plagioclase; minor quartz or nepheline may be present, along with pyroxene, amphibole or biotite. Includes rocks classified in QAPF fields 6, 7 and 8 as syenite or monzonite. Source: LeMaitre et al. 2002</skos:definition>
		<skos:prefLabel xml:lang="en">Syenitic rock</skos:prefLabel>
		<skos:prefLabel xml:lang="fr">syénite</skos:prefLabel>
		<skos:prefLabel xml:lang="it">roccia sienitica</skos:prefLabel>
		<skos:inScheme rdf:resource="urn:cgi:classifierScheme:CGI:SimpleLithology:200811"/>
	</skos:Concept>
	<skos:Concept rdf:about="urn:cgi:classifierScheme:CGI:SimpleLithology:200811:monzonite">
		<skos:definition>Phaneritic crystalline rock containing almost equal amounts of plagioclase and alkali feldspar with minor amphibole and/or pyroxene and little or no quartz. Includes rocks defined modally in QAPF Field 8. Source: LeMaitre et al. 2002</skos:definition>
		<skos:prefLabel xml:lang="en">Monzonite</skos:prefLabel>
		<skos:prefLabel xml:lang="fr">monzonite</skos:prefLabel>
		<skos:prefLabel xml:lang="it">monzonite</skos:prefLabel>
		<skos:inScheme rdf:resource="urn:cgi:classifierScheme:CGI:SimpleLithology:200811"/>
	</skos:Concept>
	<skos:Concept rdf:about="urn:cgi:classifierScheme:CGI:SimpleLithology:200811:syenite">
		<skos:definition>Coarse grained crystalline rock consisting mainly of alkali feldspar with subordinate sodic plagioclase, biotite, pyroxene, amphibole and occasional fayalite; minor quartz or nepheline may be present. Defined modally in QAPF Field 7. Source: LeMaitre et al. 2002</skos:definition>
		<skos:prefLabel xml:lang="en">Syenite</skos:prefLabel>
		<skos:prefLabel xml:lang="fr">syénite</skos:prefLabel>
		<skos:prefLabel xml:lang="it">sienite</skos:prefLabel>
		<skos:inScheme rdf:resource="urn:cgi:classifierScheme:CGI:SimpleLithology:200811"/>
	</skos:Concept>
	<skos:Concept rdf:about="urn:cgi:classifierScheme:CGI:SimpleLithology:200811:pegmatite">
		<skos:definition>Exceptionally coarse grained crystalline rock with interlocking crystals; most grains are 1cm or more diameter; composition is generally that of granite, but the term may refer to the coarse grained facies of any type of igneous rock;usually found as irregular dikes, lenses, or veins associated with plutons or batholiths. Source: Neuendorf et al. 2005</skos:definition>
		<skos:prefLabel xml:lang="en">Pegmatite</skos:prefLabel>
		<skos:prefLabel xml:lang="fr">pegmatite</skos:prefLabel>
		<skos:prefLabel xml:lang="it">pegmatite</skos:prefLabel>
		<skos:inScheme rdf:resource="urn:cgi:classifierScheme:CGI:SimpleLithology:200811"/>
	</skos:Concept>
	<skos:Concept rdf:about="urn:cgi:classifierScheme:CGI:SimpleLithology:200811:dioritic_rock">
		<skos:definition>Phaneritic crystalline rock with M less than 90, consisting of intermediate plagioclase, commonly with hornblende and often with biotite or augite. Includes rocks defined modally in QAPF fields 9 and 10 as diorite, monzodiorite. Source: LeMaitre et al. 2002</skos:definition>
		<skos:prefLabel xml:lang="en">Dioritic rock</skos:prefLabel>
		<skos:prefLabel xml:lang="fr">diorites</skos:prefLabel>
		<skos:prefLabel xml:lang="it">roccia dioritica</skos:prefLabel>
		<skos:inScheme rdf:resource="urn:cgi:classifierScheme:CGI:SimpleLithology:200811"/>
	</skos:Concept>
	<skos:Concept rdf:about="urn:cgi:classifierScheme:CGI:SimpleLithology:200811:diorite">
		<skos:definition>Phaneritic crystalline rock consisting of intermediate plagioclase, commonly with hornblende and often with biotite or augite; colour index M less than 90, sodic plagioclase (An0-An50). Includes rocks defined modally in QAPF field 10 as diorite. Source: LeMaitre et al. 2002</skos:definition>
		<skos:prefLabel xml:lang="en">Diorite</skos:prefLabel>
		<skos:prefLabel xml:lang="fr">diorites</skos:prefLabel>
		<skos:prefLabel xml:lang="it">diorite</skos:prefLabel>
		<skos:inScheme rdf:resource="urn:cgi:classifierScheme:CGI:SimpleLithology:200811"/>
	</skos:Concept>
	<skos:Concept rdf:about="urn:cgi:classifierScheme:CGI:SimpleLithology:200811:monzodiorite">
		<skos:definition>Phaneritic crystalline igneous rock consisting of sodic plagioclase (An0 to An50), alkali feldspar, hornblende and biotite, with or without pyroxene. Includes rocks defined modally in QAPF field 9 as monzodiorite. Source: LeMaitre et al. 2002</skos:definition>
		<skos:prefLabel xml:lang="en">Monzodiorite</skos:prefLabel>
		<skos:prefLabel xml:lang="fr">monzodiorite</skos:prefLabel>
		<skos:prefLabel xml:lang="it">monzodiorite</skos:prefLabel>
		<skos:inScheme rdf:resource="urn:cgi:classifierScheme:CGI:SimpleLithology:200811"/>
	</skos:Concept>
	<skos:Concept rdf:about="urn:cgi:classifierScheme:CGI:SimpleLithology:200811:gabbroic_rock">
		<skos:definition>Phaneritic crystalline rock composed of 65 percent or more of calcic plagioclase and up to 20 percent quartz or up to 10 percent feldspathoid. Includes rocks defined modally in QAPF fields 9 and 10 as gabbro or monzogabbro and foid-bearing varieties. Source: LeMaitre et al. 2002</skos:definition>
		<skos:prefLabel xml:lang="en">Gabbroic rock</skos:prefLabel>
		<skos:prefLabel xml:lang="fr">roche gabbroïque</skos:prefLabel>
		<skos:prefLabel xml:lang="it">roccia gabbrica</skos:prefLabel>
		<skos:inScheme rdf:resource="urn:cgi:classifierScheme:CGI:SimpleLithology:200811"/>
	</skos:Concept>
	<skos:Concept rdf:about="urn:cgi:classifierScheme:CGI:SimpleLithology:200811:monzogabbro">
		<skos:definition>Phaneritic crystalline igneous rock consisting of calcic plagioclase (An50 to An100), alkali feldspar, hornblende and biotite, with or without pyroxene. Includes rocks defined modally in QAPF field 9 as monzogabbro. Source: LeMaitre et al. 2002</skos:definition>
		<skos:prefLabel xml:lang="en">Monzogabbro</skos:prefLabel>
		<skos:prefLabel xml:lang="fr">monzogabbro</skos:prefLabel>
		<skos:prefLabel xml:lang="it">monzogabbro</skos:prefLabel>
		<skos:inScheme rdf:resource="urn:cgi:classifierScheme:CGI:SimpleLithology:200811"/>
	</skos:Concept>
	<skos:Concept rdf:about="urn:cgi:classifierScheme:CGI:SimpleLithology:200811:gabbro">
		<skos:definition>Phaneritic crystalline rock composed essentially of calcic plagioclase (An50 to An100), pyroxene and iron oxides. Includes rocks defined modally in QAPF Field 10 as gabbro. Source: LeMaitre et al. 2002</skos:definition>
		<skos:prefLabel xml:lang="en">Gabbro</skos:prefLabel>
		<skos:prefLabel xml:lang="fr">gabbros</skos:prefLabel>
		<skos:prefLabel xml:lang="it">gabbro</skos:prefLabel>
		<skos:inScheme rdf:resource="urn:cgi:classifierScheme:CGI:SimpleLithology:200811"/>
	</skos:Concept>
	<skos:Concept rdf:about="urn:cgi:classifierScheme:CGI:SimpleLithology:200811:foid_gabbroic_rock">
		<skos:definition>Phaneritic crystalline rock in which M is less than 90, composed of feldspathoids as 10-60 percent of the felsic minerals, calcic plagioclase (An50-An100) and large amounts of mafic minerals. Includes rocks defined modally in QAPF field 14. Source: LeMaitre et al. 2002</skos:definition>
		<skos:prefLabel xml:lang="en">Foid gabbroic rock</skos:prefLabel>
		<skos:prefLabel xml:lang="fr">gabbros foïdique</skos:prefLabel>
		<skos:prefLabel xml:lang="it">gabbro foiditico</skos:prefLabel>
		<skos:inScheme rdf:resource="urn:cgi:classifierScheme:CGI:SimpleLithology:200811"/>
	</skos:Concept>
	<skos:Concept rdf:about="urn:cgi:classifierScheme:CGI:SimpleLithology:200811:foid_dioritic_rock">
		<skos:definition>Phaneritic crystalline rock in which M is less than 90, composed of feldspathoids as 10-60 percent of the felsic minerals, sodic plagioclase (An0-An50) and large amounts of mafic minerals. Includes rocks defined modally in QAPF field 14. Source:LeMaitre et al. 2002</skos:definition>
		<skos:prefLabel xml:lang="en">Foid dioritic rock</skos:prefLabel>
		<skos:prefLabel xml:lang="fr">diorites foïdique</skos:prefLabel>
		<skos:prefLabel xml:lang="it">diorite foiditica</skos:prefLabel>
		<skos:inScheme rdf:resource="urn:cgi:classifierScheme:CGI:SimpleLithology:200811"/>
	</skos:Concept>
	<skos:Concept rdf:about="urn:cgi:classifierScheme:CGI:SimpleLithology:200811:foid_syenitic_rock">
		<skos:definition>Leucocratic, phaneritic crystalline rock composed of feldspathoids as 10-60 percent of the felsic minerals, alkali feldspar and mafic minerals. Includes rocks defined modally in QAPF field 11. Source: LeMaitre et al. 2002</skos:definition>
		<skos:prefLabel xml:lang="en">Foid syenitic rock</skos:prefLabel>
		<skos:prefLabel xml:lang="fr">syénites foïdique</skos:prefLabel>
		<skos:prefLabel xml:lang="it">sienite foiditica</skos:prefLabel>
		<skos:inScheme rdf:resource="urn:cgi:classifierScheme:CGI:SimpleLithology:200811"/>
	</skos:Concept>
	<skos:Concept rdf:about="urn:cgi:classifierScheme:CGI:SimpleLithology:200811:anorthositic_rock">
		<skos:definition>General term for a leucocratic phaneritic crystalline rock consisting essentially of plagioclase, often with small amounts of pyroxene; colour index M less than 10. Includes rocks defined modally in QAPF field 10 as anorthosite. Source: after LeMaitre et al. 2002</skos:definition>
		<skos:prefLabel xml:lang="en">Anorthositic rock</skos:prefLabel>
		<skos:prefLabel xml:lang="fr">anorthosite</skos:prefLabel>
		<skos:prefLabel xml:lang="it">anortosite</skos:prefLabel>
		<skos:inScheme rdf:resource="urn:cgi:classifierScheme:CGI:SimpleLithology:200811"/>
	</skos:Concept>
	<skos:Concept rdf:about="urn:cgi:classifierScheme:CGI:SimpleLithology:200811:foiditic_rock">
		<skos:definition>Fine grained crystalline rock containing more than 60 percent feldspathoids in total light-coloured constituents. Includes rocks defined modally in QAPF field 15 or chemically in TAS field F. Source: LeMaitre et al. 2002</skos:definition>
		<skos:prefLabel xml:lang="en">Foiditic rock</skos:prefLabel>
		<skos:prefLabel xml:lang="fr">roche foïdique</skos:prefLabel>
		<skos:prefLabel xml:lang="it">roccia foiditica</skos:prefLabel>
		<skos:inScheme rdf:resource="urn:cgi:classifierScheme:CGI:SimpleLithology:200811"/>
	</skos:Concept>
	<skos:Concept rdf:about="urn:cgi:classifierScheme:CGI:SimpleLithology:200811:foidolite">
		<skos:definition>Phaneritic crystalline rock containing more than 60 percent feldspathoids in total light-coloured constituents. Includes rocks defined modally in QAPF field 15 Source: LeMaitre et al. 2002</skos:definition>
		<skos:prefLabel xml:lang="en">Foidolite</skos:prefLabel>
		<skos:prefLabel xml:lang="fr">foïdolite</skos:prefLabel>
		<skos:prefLabel xml:lang="it">foidolite</skos:prefLabel>
		<skos:inScheme rdf:resource="urn:cgi:classifierScheme:CGI:SimpleLithology:200811"/>
	</skos:Concept>
	<skos:Concept rdf:about="urn:cgi:classifierScheme:CGI:SimpleLithology:200811:quartz_rich_phaneritic_igneous_rock">
		<skos:definition>Phaneritic crystalline igneous rock that contains greater than 60 percent quartz. Source: Gillespie and Styles 1999; LeMaitre et al. 2002</skos:definition>
		<skos:prefLabel xml:lang="en">Quartz rich phaneritic igneous rock</skos:prefLabel>
		<skos:prefLabel xml:lang="fr">roche ignée quartzique phanéritique </skos:prefLabel>
		<skos:prefLabel xml:lang="it">roccia ignea faneritica ricca in quarzo</skos:prefLabel>
		<skos:inScheme rdf:resource="urn:cgi:classifierScheme:CGI:SimpleLithology:200811"/>
	</skos:Concept>
	<skos:Concept rdf:about="urn:cgi:classifierScheme:CGI:SimpleLithology:200811:porphyry">
		<skos:definition>Igneous rock that contains conspicuous phenocrysts in a finer grained groundmass; groundmass itself may be phaneritic or fine-grained. Source: LeMaitre et al. 2002</skos:definition>
		<skos:prefLabel xml:lang="en">Porphyry</skos:prefLabel>
		<skos:prefLabel xml:lang="fr">porphyre</skos:prefLabel>
		<skos:prefLabel xml:lang="it">porfirite</skos:prefLabel>
		<skos:inScheme rdf:resource="urn:cgi:classifierScheme:CGI:SimpleLithology:200811"/>
	</skos:Concept>
	<skos:Concept rdf:about="urn:cgi:classifierScheme:CGI:SimpleLithology:200811:doleritic_rock">
		<skos:definition>Dark colored gabbroic (basaltic) or dioritic (andesitic) rock intermediate in grain size between basalt and gabbro and composed of plagioclase, pyroxene and opaque minerals; often with ophitic texture. Typically occurs as hypabyssal intrusions. Includes dolerite, microdiorite, diabase and microgabbro. Source: Neuendorf et al 2005; LeMaitre et al 2002; Gillespie and Styles, 1999</skos:definition>
		<skos:prefLabel xml:lang="en">Doleritic rock</skos:prefLabel>
		<skos:prefLabel xml:lang="fr">dolérites</skos:prefLabel>
		<skos:prefLabel xml:lang="it">dolerite</skos:prefLabel>
		<skos:inScheme rdf:resource="urn:cgi:classifierScheme:CGI:SimpleLithology:200811"/>
	</skos:Concept>
	<skos:Concept rdf:about="urn:cgi:classifierScheme:CGI:SimpleLithology:200811:fine_grained_igneous_rock">
		<skos:definition>Aphanitic or porphyritic igneous rock composed of greater than 10 percent groundmass, in which most of the crystals cannot be distinguished with the unaided eye; grainsize is typically less than 1mm. Igneous rocks with 'exotic' composition are excluded from this concept. Source: Gillespie and Styles 1999; LeMaitre et al. 2002</skos:definition>
		<skos:prefLabel xml:lang="en">Fine grained igneous rock</skos:prefLabel>
		<skos:prefLabel xml:lang="fr">roche ignée à grain fin</skos:prefLabel>
		<skos:prefLabel xml:lang="it">roccia ignea a grana fine</skos:prefLabel>
		<skos:inScheme rdf:resource="urn:cgi:classifierScheme:CGI:SimpleLithology:200811"/>
	</skos:Concept>
	<skos:Concept rdf:about="urn:cgi:classifierScheme:CGI:SimpleLithology:200811:andesitic_rock">
		<skos:definition>Fine grained crystalline rock, usually porphyritic, consisting of plagioclase (frequently zoned from labradorite to oligoclase), pyroxene, hornblende and/or biotite; color index M less than 35. Includes rocks defined modally in QAPF fields 9 and 10 or chemically in TAS field O2 as andesite. Fine grained equivalent of dioritic rock. Source: after LeMaitre et al. 2002</skos:definition>
		<skos:prefLabel xml:lang="en">Andesitic rock</skos:prefLabel>
		<skos:prefLabel xml:lang="fr">andésites</skos:prefLabel>
		<skos:prefLabel xml:lang="it">andesite</skos:prefLabel>
		<skos:inScheme rdf:resource="urn:cgi:classifierScheme:CGI:SimpleLithology:200811"/>
	</skos:Concept>
	<skos:Concept rdf:about="urn:cgi:classifierScheme:CGI:SimpleLithology:200811:dacitic_rock">
		<skos:definition>Fine grained or porphyritic crystalline rock composed of quartz and sodic plagioclase with minor amounts of biotite and/or hornblende and/or pyroxene; volcanic equivalent of granodiorite and tonalite. Includes rocks defined modally in QAPF fields 4 and 5 or chemically in TAS Field O3. Source: LeMaitre et al. 2002</skos:definition>
		<skos:prefLabel xml:lang="en">Dacitic rock</skos:prefLabel>
		<skos:prefLabel xml:lang="fr">dacites</skos:prefLabel>
		<skos:prefLabel xml:lang="it">dacite</skos:prefLabel>
		<skos:inScheme rdf:resource="urn:cgi:classifierScheme:CGI:SimpleLithology:200811"/>
	</skos:Concept>
	<skos:Concept rdf:about="urn:cgi:classifierScheme:CGI:SimpleLithology:200811:trachytic_rock">
		<skos:definition>Fine-grained volcanic rock consisting of alkali feldspar and minor mafic minerals, typically amphibole or mica; typically porphyritic. Includes rocks defined modally in QAPF fields 6, 7 and 8 or chemically in TAS Field T as trachyte or latite. Source: LeMaitre et al. 2002</skos:definition>
		<skos:prefLabel xml:lang="en">Trachytic rock</skos:prefLabel>
		<skos:prefLabel xml:lang="fr">trachytes</skos:prefLabel>
		<skos:prefLabel xml:lang="it">trachite</skos:prefLabel>
		<skos:inScheme rdf:resource="urn:cgi:classifierScheme:CGI:SimpleLithology:200811"/>
	</skos:Concept>
	<skos:Concept rdf:about="urn:cgi:classifierScheme:CGI:SimpleLithology:200811:rhyolitic_rock">
		<skos:definition>Fine-grained igneous rock, typically porphyritic, consisting of quartz and alkali feldspar (often as phenocrysts), with minor plagioclase and biotite, in a microcrystalline, cryptocrystalline or glassy groundmass. Flow texture is common. Includes rocks defined modally in QAPF fields 2 and 3 or chemically in TAS Field R as rhyolite. Source: LeMaitre et al. 2002</skos:definition>
		<skos:prefLabel xml:lang="en">Rhyolitic rock</skos:prefLabel>
		<skos:prefLabel xml:lang="fr">rhyolites</skos:prefLabel>
		<skos:prefLabel xml:lang="it">riolite</skos:prefLabel>
		<skos:inScheme rdf:resource="urn:cgi:classifierScheme:CGI:SimpleLithology:200811"/>
	</skos:Concept>
	<skos:Concept rdf:about="urn:cgi:classifierScheme:CGI:SimpleLithology:200811:phonolitic_rock">
		<skos:definition>Fine grained igneous rock containing feldspathoids and in which alkali feldspar is thought to be more abundant than plagioclase. Includes rocks defined modally in QAPF fields 11 and 12, and TAS field Ph. Source: LeMaitre et al. 2002</skos:definition>
		<skos:prefLabel xml:lang="en">Phonolitic rock</skos:prefLabel>
		<skos:prefLabel xml:lang="fr">phonolites</skos:prefLabel>
		<skos:prefLabel xml:lang="it">fonolite</skos:prefLabel>
		<skos:inScheme rdf:resource="urn:cgi:classifierScheme:CGI:SimpleLithology:200811"/>
	</skos:Concept>
	<skos:Concept rdf:about="urn:cgi:classifierScheme:CGI:SimpleLithology:200811:basaltic_rock">
		<skos:definition>Fine-grained or porphyritic igneous rock with less than 20 percent quartz, and less than 10 percent feldspathoid minerals, in which the ratio of plagioclase to alkali feldspar is greater than 66 percent, and the color index is greater than 35. Typically composed of calcic plagioclase and clinopyroxene; phenocrysts typically include one or more of calcic plagioclase, clinopyroxene, orthopyroxene, and olivine. Includes rocks defined modally in QAPF fields 9 and 10 or chemically in TAS field B as basalt. Source: after LeMaitre et al. 2002</skos:definition>
		<skos:prefLabel xml:lang="en">Basaltic rock</skos:prefLabel>
		<skos:prefLabel xml:lang="fr">basaltes</skos:prefLabel>
		<skos:prefLabel xml:lang="it">basalto</skos:prefLabel>
		<skos:inScheme rdf:resource="urn:cgi:classifierScheme:CGI:SimpleLithology:200811"/>
	</skos:Concept>
	<skos:Concept rdf:about="urn:cgi:classifierScheme:CGI:SimpleLithology:200811:tephritic_rock">
		<skos:definition>Fine grained crystalline igneous rock containing essential feldspathoids and in which plagioclase is more abundant than alkali feldspar. Includes rocks classified in QAPF field 14 or chemically in TAS field U1 as basanite or tephrite. Source: LeMaitre et al. 2002</skos:definition>
		<skos:prefLabel xml:lang="en">Tephritic rock</skos:prefLabel>
		<skos:prefLabel xml:lang="fr">téphrites</skos:prefLabel>
		<skos:prefLabel xml:lang="it">roccia tefritica</skos:prefLabel>
		<skos:inScheme rdf:resource="urn:cgi:classifierScheme:CGI:SimpleLithology:200811"/>
	</skos:Concept>
	<skos:Concept rdf:about="urn:cgi:classifierScheme:CGI:SimpleLithology:200811:acidic_igneous_rock">
		<skos:definition>Igneous rock with more than 63 percent SiO2. Source: after LeMaitre et al. 2002</skos:definition>
		<skos:prefLabel xml:lang="en">Acidic igneous rock</skos:prefLabel>
		<skos:prefLabel xml:lang="fr">roche ignée acide</skos:prefLabel>
		<skos:prefLabel xml:lang="it">roccia ignea acida</skos:prefLabel>
		<skos:inScheme rdf:resource="urn:cgi:classifierScheme:CGI:SimpleLithology:200811"/>
		<skos:broader rdf:resource="urn:cgi:classifierScheme:CGI:SimpleLithology:200811:igneous_rock"/>
	</skos:Concept>
	<skos:Concept rdf:about="urn:cgi:classifierScheme:CGI:SimpleLithology:200811:intermediate_composition_igneous_rock">
		<skos:definition>Igneous rock with between 52 and 63 percent SiO2. Source: after LeMaitre et al. 2002</skos:definition>
		<skos:prefLabel xml:lang="en">intermediate composition igneous rock</skos:prefLabel>
		<skos:prefLabel xml:lang="fr">roche ignés de composition intermédiaire</skos:prefLabel>
		<skos:prefLabel xml:lang="it">roccia ignea a composizione intermedia</skos:prefLabel>
		<skos:inScheme rdf:resource="urn:cgi:classifierScheme:CGI:SimpleLithology:200811"/>
	</skos:Concept>
	<skos:Concept rdf:about="urn:cgi:classifierScheme:CGI:SimpleLithology:200811:basic_igneous_rock">
		<skos:definition>Igneous rock with between 45 and 52 percent SiO2. Source: after LeMaitre et al. 2002</skos:definition>
		<skos:prefLabel xml:lang="en">Basic igneous rock</skos:prefLabel>
		<skos:prefLabel xml:lang="fr">roche ignée basique</skos:prefLabel>
		<skos:prefLabel xml:lang="it">roccia ignea basica</skos:prefLabel>
		<skos:inScheme rdf:resource="urn:cgi:classifierScheme:CGI:SimpleLithology:200811"/>
	</skos:Concept>
	<skos:Concept rdf:about="urn:cgi:classifierScheme:CGI:SimpleLithology:200811:composite_genesis_rock">
		<skos:definition>Rock formed by geological modification of pre-existing rocks outside the realm of igneous and sedimentary processes. Includes rocks formed by impact metamorphism, standard dynamothermal metamorphism, brittle deformation, weathering, metasomatism and hydrothermal alteration (diagenesis is a sedimentary process in this context). Source: SLTTm 2004</skos:definition>
		<skos:prefLabel xml:lang="en">Composite genesis rock</skos:prefLabel>
		<skos:prefLabel xml:lang="fr">roche modifiée et/ou transformée</skos:prefLabel>
		<skos:prefLabel xml:lang="it">roccia modificata o trasformata</skos:prefLabel>
		<skos:inScheme rdf:resource="urn:cgi:classifierScheme:CGI:SimpleLithology:200811"/>
	</skos:Concept>
	<skos:Concept rdf:about="urn:cgi:classifierScheme:CGI:SimpleLithology:200811:impact_metamorphic_rock">
		<skos:definition>Rock that contains features indicative of shock metamorphism, such as microscopic planar deformation features within grains or shatter cones. Includes breccias and melt rocks. Source: Stöffler and Grieve 2007; Jackson 1997</skos:definition>
		<skos:prefLabel xml:lang="en">Impact metamorphic rock</skos:prefLabel>
		<skos:prefLabel xml:lang="fr">impactite</skos:prefLabel>
		<skos:prefLabel xml:lang="it">roccia metamorfica da impatto</skos:prefLabel>
		<skos:inScheme rdf:resource="urn:cgi:classifierScheme:CGI:SimpleLithology:200811"/>
	</skos:Concept>
	<skos:Concept rdf:about="urn:cgi:classifierScheme:CGI:SimpleLithology:200811:metamorphic_rock">
		<skos:definition>Rock formed by solid-state mineralogical, chemical and/or structural changes to a pre-existing rock, in response to marked changes in temperature, pressure, shearing stress and chemical environment; generally at depth in the crust. Source: Jackson 1997</skos:definition>
		<skos:prefLabel xml:lang="en">Metamorphic rock</skos:prefLabel>
		<skos:prefLabel xml:lang="fr">métamorphites indifférenciées</skos:prefLabel>
		<skos:prefLabel xml:lang="it">roccia metamorfica</skos:prefLabel>
		<skos:inScheme rdf:resource="urn:cgi:classifierScheme:CGI:SimpleLithology:200811"/>
	</skos:Concept>
	<skos:Concept rdf:about="urn:cgi:classifierScheme:CGI:SimpleLithology:200811:migmatite">
		<skos:definition>Silicate metamorphic rock that is pervasively heterogeneous on a meso- to megascopic scale that typically consists of darker and lighter parts; the darker parts usually exhibit features of metamorphic rocks whereas the lighter parts are of igneous-looking appearance. Source: after IUGS SCMR 2007 (http://www.bgs.ac.uk/SCMR/)</skos:definition>
		<skos:prefLabel xml:lang="en">Migmatite</skos:prefLabel>
		<skos:prefLabel xml:lang="fr">migmatites</skos:prefLabel>
		<skos:prefLabel xml:lang="it">migmatite</skos:prefLabel>
		<skos:inScheme rdf:resource="urn:cgi:classifierScheme:CGI:SimpleLithology:200811"/>
	</skos:Concept>
	<skos:Concept rdf:about="urn:cgi:classifierScheme:CGI:SimpleLithology:200811:hornfels">
		<skos:definition>Granofels composed of a mosaic of equidimensional grains in a characteristically granoblastic or decussate matrix; porphyroblasts or relict phenocrysts may be present. Typically formed by contact metamorphism. Source: IUGS SCMR 2007 (http://www.bgs.ac.uk/SCMR/)</skos:definition>
		<skos:prefLabel xml:lang="en">Hornfels</skos:prefLabel>
		<skos:prefLabel xml:lang="fr">cornéennes</skos:prefLabel>
		<skos:prefLabel xml:lang="it">hornfels (o granofels)</skos:prefLabel>
		<skos:inScheme rdf:resource="urn:cgi:classifierScheme:CGI:SimpleLithology:200811"/>
	</skos:Concept>
	<skos:Concept rdf:about="urn:cgi:classifierScheme:CGI:SimpleLithology:200811:granofels">
		<skos:definition>Phaneritic metamorphic rock with granoblastic fabric and very little or no foliation (less than 10 percent of the mineral grains in the rock are elements in a planar or linear fabric). Source: SLTTm 2004</skos:definition>
		<skos:prefLabel xml:lang="en">Granofels</skos:prefLabel>
		<skos:prefLabel xml:lang="fr">schiste tacheté (?)</skos:prefLabel>
		<skos:prefLabel xml:lang="it">granofels</skos:prefLabel>
		<skos:inScheme rdf:resource="urn:cgi:classifierScheme:CGI:SimpleLithology:200811"/>
	</skos:Concept>
	<skos:Concept rdf:about="urn:cgi:classifierScheme:CGI:SimpleLithology:200811:foliated_metamorphic_rock">
		<skos:definition>Metamorphic rock in which 10 percent or more of the contained mineral grains are elements in a planar or linear fabric. Cataclastic or glassy character precludes classification with this concept. Source: based on NADM SLTT metamorphic</skos:definition>
		<skos:prefLabel xml:lang="en">Foliated metamorphic rock</skos:prefLabel>
		<skos:prefLabel xml:lang="fr">roche métamorphique foliée</skos:prefLabel>
		<skos:prefLabel xml:lang="it">roccia metamorfica foliata</skos:prefLabel>
		<skos:inScheme rdf:resource="urn:cgi:classifierScheme:CGI:SimpleLithology:200811"/>
	</skos:Concept>
	<skos:Concept rdf:about="urn:cgi:classifierScheme:CGI:SimpleLithology:200811:schist">
		<skos:definition>Foliated phaneritic metamorphic rock with well developed, continuous schistosity (greater than 50 percent of mineral grains with a tabular, lamellar, or prismatic crystallographic habit that are oriented in a continuous planar or linear fabric). Source: SLTTm 2004; Neuendorf et al. 2005</skos:definition>
		<skos:prefLabel xml:lang="en">Schist</skos:prefLabel>
		<skos:prefLabel xml:lang="fr">schistes</skos:prefLabel>
		<skos:prefLabel xml:lang="it">scisto</skos:prefLabel>
		<skos:inScheme rdf:resource="urn:cgi:classifierScheme:CGI:SimpleLithology:200811"/>
	</skos:Concept>
	<skos:Concept rdf:about="urn:cgi:classifierScheme:CGI:SimpleLithology:200811:slate">
		<skos:definition>Compact, fine grained rock with an average grain size less than 0.032 millimeter and a well developed schistosity (slaty cleavage), and hence can be split into slabs or thin plates. Source: NADM metamorphic rock vocabulary SLTTm1.0; Neuendorf et al. 2005</skos:definition>
		<skos:prefLabel xml:lang="en">Slate</skos:prefLabel>
		<skos:prefLabel xml:lang="fr">ardoise</skos:prefLabel>
		<skos:prefLabel xml:lang="it">ardesia</skos:prefLabel>
		<skos:inScheme rdf:resource="urn:cgi:classifierScheme:CGI:SimpleLithology:200811"/>
	</skos:Concept>
	<skos:Concept rdf:about="urn:cgi:classifierScheme:CGI:SimpleLithology:200811:phyllite">
		<skos:definition>Rock with a well developed, continuous schistosity, an average grain size between 0.1 and 0.5 millimeters, and a silvery sheen on cleavage surfaces. Individual phyllosilicate grains are barely visible with the unaided eye. Source: IUGS SCMR 2007 (http://www.bgs.ac.uk/SCMR/)</skos:definition>
		<skos:prefLabel xml:lang="en">Phyllite</skos:prefLabel>
		<skos:prefLabel xml:lang="fr">phyllite</skos:prefLabel>
		<skos:prefLabel xml:lang="it">fillade</skos:prefLabel>
		<skos:inScheme rdf:resource="urn:cgi:classifierScheme:CGI:SimpleLithology:200811"/>
	</skos:Concept>
	<skos:Concept rdf:about="urn:cgi:classifierScheme:CGI:SimpleLithology:200811:mylonitic_rock">
		<skos:definition>Metamorphic rock characterised by a foliation resulting from tectonic grain size reduction, in which more than 10 percent of the rock volume has undergone grain size reduction. Includes protomylonite, mylonite, ultramylonite, phyllonite and blastomylonite. Source: Marshak &amp; Mitra 1988</skos:definition>
		<skos:prefLabel xml:lang="en">Mylonitic rock</skos:prefLabel>
		<skos:prefLabel xml:lang="fr">mylonites</skos:prefLabel>
		<skos:prefLabel xml:lang="it">milonite</skos:prefLabel>
		<skos:inScheme rdf:resource="urn:cgi:classifierScheme:CGI:SimpleLithology:200811"/>
	</skos:Concept>
	<skos:Concept rdf:about="urn:cgi:classifierScheme:CGI:SimpleLithology:200811:phyllonite">
		<skos:definition>Mylonitic rock composed largely of fine-grained mica that imparts a sheen to foliation surfaces; may have flaser lamination, isoclinal folding, and deformed veins, which indicate significant shearing. Macroscopically resembles phyllite, but formed by mechanical degradation of initially coarser rock. Source: NADM metamorphic rock vocabulary SLTTm1.0; Marshak &amp; Mitra 1988</skos:definition>
		<skos:prefLabel xml:lang="en">Phyllonite</skos:prefLabel>
		<skos:prefLabel xml:lang="fr">phyllonite</skos:prefLabel>
		<skos:prefLabel xml:lang="it">fillonite</skos:prefLabel>
		<skos:inScheme rdf:resource="urn:cgi:classifierScheme:CGI:SimpleLithology:200811"/>
	</skos:Concept>
	<skos:Concept rdf:about="urn:cgi:classifierScheme:CGI:SimpleLithology:200811:gneiss">
		<skos:definition>Foliated metamorphic rock with bands or lenticles rich in granular minerals alternating with bands or lenticles rich in minerals with a flaky or elongate prismatic habit. Mylonitic foliation or well developed, continuous schistosity (greater than 50 percent of the rock consists of grains participate in a planar or linear fabric) precludes classification with this concept. Source: Neuendorf et al. 2005</skos:definition>
		<skos:prefLabel xml:lang="en">Gneiss</skos:prefLabel>
		<skos:prefLabel xml:lang="fr">orthogneiss</skos:prefLabel>
		<skos:prefLabel xml:lang="it">gneiss</skos:prefLabel>
		<skos:inScheme rdf:resource="urn:cgi:classifierScheme:CGI:SimpleLithology:200811"/>
	</skos:Concept>
	<skos:Concept rdf:about="urn:cgi:classifierScheme:CGI:SimpleLithology:200811:quartzite">
		<skos:definition>Metamorphic rock consisting of greater than or equal to 75 percent quartz; typically granoblastic texture. Source: after Neuendorf et al. 2005</skos:definition>
		<skos:prefLabel xml:lang="en">Quartzite</skos:prefLabel>
		<skos:prefLabel xml:lang="fr">quartzites</skos:prefLabel>
		<skos:prefLabel xml:lang="it">quarzite</skos:prefLabel>
		<skos:inScheme rdf:resource="urn:cgi:classifierScheme:CGI:SimpleLithology:200811"/>
	</skos:Concept>
	<skos:Concept rdf:about="urn:cgi:classifierScheme:CGI:SimpleLithology:200811:serpentinite">
		<skos:definition>Rock consisting of more than 75 percent serpentine-group minerals, eg. antigorite, chrysotile or lizardite; accessory chlorite, talc and magnetite may be present; derived from hydration of ferromagnesian silicate minerals such as olivine and pyroxene. Source: Neuendorf et al. 2005</skos:definition>
		<skos:prefLabel xml:lang="en">Serpentinite</skos:prefLabel>
		<skos:prefLabel xml:lang="fr">serpentinites</skos:prefLabel>
		<skos:prefLabel xml:lang="it">serpentinite</skos:prefLabel>
		<skos:inScheme rdf:resource="urn:cgi:classifierScheme:CGI:SimpleLithology:200811"/>
	</skos:Concept>
	<skos:Concept rdf:about="urn:cgi:classifierScheme:CGI:SimpleLithology:200811:eclogite">
		<skos:definition>Metamorphic rock composed of 75 percent or more (by volume) omphacite and garnet, both of which are present as major constituents, the amount of neither of them being higher than 75 percent (by volume); the presence of plagioclase precludes classification as an eclogite. Source: IUGS SCMR 2007 (http://www.bgs.ac.uk/SCMR/)</skos:definition>
		<skos:prefLabel xml:lang="en">Eclogite</skos:prefLabel>
		<skos:prefLabel xml:lang="fr">éclogites</skos:prefLabel>
		<skos:prefLabel xml:lang="it">eclogite</skos:prefLabel>
		<skos:inScheme rdf:resource="urn:cgi:classifierScheme:CGI:SimpleLithology:200811"/>
	</skos:Concept>
	<skos:Concept rdf:about="urn:cgi:classifierScheme:CGI:SimpleLithology:200811:amphibolite">
		<skos:definition>Metamorphic rock mainly consisting of green, brown or black amphibole and plagioclase (including albite), which combined form 75 percent or more of the rock, and both of which are present as major constituents. The amphibole constitutes 50 percent or more of the total mafic constituents and is present in an amount of 30 percent or more; other common minerals include quartz, clinopyroxene, garnet, epidote-group minerals, biotite, titanite and scapolite. Source: Coutinho et al. 2007, IUGS SCMR chapter 8 (http://www.bgs.ac.uk/SCMR/)</skos:definition>
		<skos:prefLabel xml:lang="en">Amphibolite</skos:prefLabel>
		<skos:prefLabel xml:lang="fr">amphibolites</skos:prefLabel>
		<skos:prefLabel xml:lang="it">anfibolite</skos:prefLabel>
		<skos:inScheme rdf:resource="urn:cgi:classifierScheme:CGI:SimpleLithology:200811"/>
	</skos:Concept>
	<skos:Concept rdf:about="urn:cgi:classifierScheme:CGI:SimpleLithology:200811:marble">
		<skos:definition>Metamorphic rock consisting of greater than 75 percent fine- to coarse-grained recrystallized calcite and/or dolomite; usually with a granoblastic, saccharoidal texture. Source: IUGS SCMR 2007 (http://www.bgs.ac.uk/SCMR/), SLTTm1.0 2004</skos:definition>
		<skos:prefLabel xml:lang="en">Marble</skos:prefLabel>
		<skos:prefLabel xml:lang="fr">marbres</skos:prefLabel>
		<skos:prefLabel xml:lang="it">marmo</skos:prefLabel>
		<skos:inScheme rdf:resource="urn:cgi:classifierScheme:CGI:SimpleLithology:200811"/>
	</skos:Concept>
	<skos:Concept rdf:about="urn:cgi:classifierScheme:CGI:SimpleLithology:200811:sedimentary_rock">
		<skos:definition>Rock formed by accumulation and cementation of solid fragmental material deposited by air, water or ice, or as a result of other natural agents, such as precipitation from solution, the accumulation of organic material, or from biogenic processes, including secretion by organisms. Includes epiclastic deposits. Source: SLTTs 2004</skos:definition>
		<skos:prefLabel xml:lang="en">Sedimentary rock</skos:prefLabel>
		<skos:prefLabel xml:lang="fr">roche sédimentaire</skos:prefLabel>
		<skos:prefLabel xml:lang="it">roccia sedimentaria</skos:prefLabel>
		<skos:inScheme rdf:resource="urn:cgi:classifierScheme:CGI:SimpleLithology:200811"/>
	</skos:Concept>
	<skos:Concept rdf:about="urn:cgi:classifierScheme:CGI:SimpleLithology:200811:clastic_sedimentary_rock">
		<skos:definition>Sedimentary rock in which at least 50 percent of the constituent particles were derived from erosion, weathering, or mass-wasting of pre-existing earth materials, and transported to the place of deposition by mechanical agents such as water, wind, ice and gravity. Source: SLTTs, 2004; Neuendorf et al., 2005</skos:definition>
		<skos:prefLabel xml:lang="en">Clastic sedimentary rock</skos:prefLabel>
		<skos:prefLabel xml:lang="fr">roche sédimentaire clastique</skos:prefLabel>
		<skos:prefLabel xml:lang="it">roccia detritica</skos:prefLabel>
		<skos:inScheme rdf:resource="urn:cgi:classifierScheme:CGI:SimpleLithology:200811"/>
	</skos:Concept>
	<skos:Concept rdf:about="urn:cgi:classifierScheme:CGI:SimpleLithology:200811:mudstone">
		<skos:definition>Clastic sedimentary rock consisting of less than 30 percent gravel-size (2 mm) particles and with a mud to sand ratio greater than 1. Clasts may be of any composition or origin. Source: Pettijohn et al. 1987 referenced in Hallsworth &amp; Knox 1999; extrapolated from Folk, 1954, Figure 1a</skos:definition>
		<skos:prefLabel xml:lang="en">Mudstone</skos:prefLabel>
		<skos:prefLabel xml:lang="fr">mudstone</skos:prefLabel>
		<skos:prefLabel xml:lang="it">mudstone</skos:prefLabel>
		<skos:inScheme rdf:resource="urn:cgi:classifierScheme:CGI:SimpleLithology:200811"/>
	</skos:Concept>
	<skos:Concept rdf:about="urn:cgi:classifierScheme:CGI:SimpleLithology:200811:shale">
		<skos:definition>Laminated mudstone that will part or break along thin, closely spaced layers parallel to stratification. Source: NADM SLTT sedimentary; Neuendorf et al. 2005</skos:definition>
		<skos:prefLabel xml:lang="en">Shale</skos:prefLabel>
		<skos:prefLabel xml:lang="fr">shale</skos:prefLabel>
		<skos:prefLabel xml:lang="it">argillite o scisto</skos:prefLabel>
		<skos:inScheme rdf:resource="urn:cgi:classifierScheme:CGI:SimpleLithology:200811"/>
	</skos:Concept>
	<skos:Concept rdf:about="urn:cgi:classifierScheme:CGI:SimpleLithology:200811:sandstone">
		<skos:definition>Clastic sedimentary rock in which less than 30 percent of particles are greater than 2 mm in diameter (gravel) and the sand to mud ratio is at least 1. Source: SLTTs 2004; Neuendorf et al. 2005; particle size from Wentworth grade scale</skos:definition>
		<skos:prefLabel xml:lang="en">Sandstone</skos:prefLabel>
		<skos:prefLabel xml:lang="fr">grès</skos:prefLabel>
		<skos:prefLabel xml:lang="it">arenaria</skos:prefLabel>
		<skos:inScheme rdf:resource="urn:cgi:classifierScheme:CGI:SimpleLithology:200811"/>
	</skos:Concept>
	<skos:Concept rdf:about="urn:cgi:classifierScheme:CGI:SimpleLithology:200811:conglomerate">
		<skos:definition>Coarse grained sedimentary rock composed of at least 30 percent rounded to subangular fragments larger than 2 mm in diameter; typically contains finer grained material in interstices between larger fragments. Source: Neuendorf et al. 2005; SLTTs 2004</skos:definition>
		<skos:prefLabel xml:lang="en">Conglomerate</skos:prefLabel>
		<skos:prefLabel xml:lang="fr">conglomérats</skos:prefLabel>
		<skos:prefLabel xml:lang="it">conglomerato</skos:prefLabel>
		<skos:inScheme rdf:resource="urn:cgi:classifierScheme:CGI:SimpleLithology:200811"/>
	</skos:Concept>
	<skos:Concept rdf:about="urn:cgi:classifierScheme:CGI:SimpleLithology:200811:wackestone">
		<skos:definition>Sandstone that contains between 15 and 75 percent matrix of unspecified origin. Source: this vocabulary</skos:definition>
		<skos:prefLabel xml:lang="en">Wackestone</skos:prefLabel>
		<skos:prefLabel xml:lang="fr">wackestone</skos:prefLabel>
		<skos:prefLabel xml:lang="it">wackestone</skos:prefLabel>
		<skos:inScheme rdf:resource="urn:cgi:classifierScheme:CGI:SimpleLithology:200811"/>
	</skos:Concept>
	<skos:Concept rdf:about="urn:cgi:classifierScheme:CGI:SimpleLithology:200811:diamictite">
		<skos:definition>Unsorted or poorly sorted, clastic sedimentary rock with a wide range of particle sizes such that it cannot be assigned to any other class. Source: Fairbridge and Bourgeois 1978</skos:definition>
		<skos:prefLabel xml:lang="en">Diamictite</skos:prefLabel>
		<skos:prefLabel xml:lang="fr">tillite</skos:prefLabel>
		<skos:prefLabel xml:lang="it">diamictite</skos:prefLabel>
		<skos:inScheme rdf:resource="urn:cgi:classifierScheme:CGI:SimpleLithology:200811"/>
	</skos:Concept>
	<skos:Concept rdf:about="urn:cgi:classifierScheme:CGI:SimpleLithology:200811:carbonate_sedimentary_rock">
		<skos:definition>Sedimentary rock in which at least 50 percent of the primary and/or recrystallized constituents are composed of one (or more) of the carbonate minerals calcite, aragonite and dolomite, in particles of intrabasinal origin. Source: SLTTs 2004</skos:definition>
		<skos:prefLabel xml:lang="en">Carbonate sedimentary rock</skos:prefLabel>
		<skos:prefLabel xml:lang="fr">roche sédimentaire carbonaté </skos:prefLabel>
		<skos:prefLabel xml:lang="it">roccia sedimentaria carbonatica</skos:prefLabel>
		<skos:inScheme rdf:resource="urn:cgi:classifierScheme:CGI:SimpleLithology:200811"/>
	</skos:Concept>
	<skos:Concept rdf:about="urn:cgi:classifierScheme:CGI:SimpleLithology:200811:calcareous_carbonate_sedimentary_rock">
		<skos:definition>Carbonate sedimentary rock with a calcite (plus aragonite) to dolomite ratio greater than 1 to 1. Includes limestone and dolomitic limestone. Source: SLTTs 2004; Hallsworth &amp; Knox 1999</skos:definition>
		<skos:prefLabel xml:lang="en">Calcareous carbonate sedimentary rock</skos:prefLabel>
		<skos:prefLabel xml:lang="fr">calcaires</skos:prefLabel>
		<skos:prefLabel xml:lang="it">calcare</skos:prefLabel>
		<skos:inScheme rdf:resource="urn:cgi:classifierScheme:CGI:SimpleLithology:200811"/>
	</skos:Concept>
	<skos:Concept rdf:about="urn:cgi:classifierScheme:CGI:SimpleLithology:200811:dolomitic_or_magnesian_sedimentary_rock">
		<skos:definition>Carbonate sedimentary rock with a ratio of magnesium carbonate to calcite (plus aragonite) greater than 1 to 1. Includes dolostone, lime dolostone and magnesite-stone. Source: after SLTTs 2004, Hallsworth and Knox 1999</skos:definition>
		<skos:prefLabel xml:lang="en">Dolomitic or magnesian sedimentary rock</skos:prefLabel>
		<skos:prefLabel xml:lang="fr">dolomies</skos:prefLabel>
		<skos:prefLabel xml:lang="it">dolomia</skos:prefLabel>
		<skos:inScheme rdf:resource="urn:cgi:classifierScheme:CGI:SimpleLithology:200811"/>
	</skos:Concept>
	<skos:Concept rdf:about="urn:cgi:classifierScheme:CGI:SimpleLithology:200811:boundstone">
		<skos:definition>Sedimentary carbonate rock with preserved biogenic texture, whose original components were bound and encrusted together during deposition by the action of plants and animals during deposition, and remained substantially in the position of growth. Source: Hallsworth and Knox 1999; SLTTs 2004</skos:definition>
		<skos:prefLabel xml:lang="en">Boundstone</skos:prefLabel>
		<skos:prefLabel xml:lang="fr">boundstone</skos:prefLabel>
		<skos:prefLabel xml:lang="it">boundstone</skos:prefLabel>
		<skos:inScheme rdf:resource="urn:cgi:classifierScheme:CGI:SimpleLithology:200811"/>
	</skos:Concept>
	<skos:Concept rdf:about="urn:cgi:classifierScheme:CGI:SimpleLithology:200811:carbonate_mudstone">
		<skos:definition>Carbonate sedimentary rock with matrix-supported fabric, composed of more than 75 percent mud-sized grains (maximum diameter less than 32 microns). The original depositional texture is preserved. Source: Hallsworth &amp; Knox 1999; SLTTs, 2004</skos:definition>
		<skos:prefLabel xml:lang="en">Carbonate mudstone</skos:prefLabel>
		<skos:prefLabel xml:lang="fr">mudstone carbonatée</skos:prefLabel>
		<skos:prefLabel xml:lang="it">mudstone carbonatico</skos:prefLabel>
		<skos:inScheme rdf:resource="urn:cgi:classifierScheme:CGI:SimpleLithology:200811"/>
	</skos:Concept>
	<skos:Concept rdf:about="urn:cgi:classifierScheme:CGI:SimpleLithology:200811:grainstone">
		<skos:definition>Carbonate sedimentary rock with recognizable depositional fabric that is grain-supported; contains little or no mud matrix. Source: Dunham 1962</skos:definition>
		<skos:prefLabel xml:lang="en">Grainstone</skos:prefLabel>
		<skos:prefLabel xml:lang="fr">grainstone</skos:prefLabel>
		<skos:prefLabel xml:lang="it">grainstone</skos:prefLabel>
		<skos:inScheme rdf:resource="urn:cgi:classifierScheme:CGI:SimpleLithology:200811"/>
	</skos:Concept>
	<skos:Concept rdf:about="urn:cgi:classifierScheme:CGI:SimpleLithology:200811:packstone">
		<skos:definition>Carbonate sedimentary rock with discernible grain supported depositional texture, containing greater than 10 percent grains; intergranular spaces are filled by matrix. Source: Hallsworth &amp; Knox 1999</skos:definition>
		<skos:prefLabel xml:lang="en">Packstone</skos:prefLabel>
		<skos:prefLabel xml:lang="fr">packstone</skos:prefLabel>
		<skos:prefLabel xml:lang="it">packstone</skos:prefLabel>
		<skos:inScheme rdf:resource="urn:cgi:classifierScheme:CGI:SimpleLithology:200811"/>
	</skos:Concept>
	<skos:Concept rdf:about="urn:cgi:classifierScheme:CGI:SimpleLithology:200811:crystalline_carbonate">
		<skos:definition>Carbonate rock of indeterminate mineralogy in which diagenetic processes have obliterated any original depositional texture. Source: SLTTs 2004</skos:definition>
		<skos:prefLabel xml:lang="en">Crystalline carbonate</skos:prefLabel>
		<skos:prefLabel xml:lang="fr">calcaire cristallin</skos:prefLabel>
		<skos:prefLabel xml:lang="it">calcare cristallino</skos:prefLabel>
		<skos:inScheme rdf:resource="urn:cgi:classifierScheme:CGI:SimpleLithology:200811"/>
	</skos:Concept>
	<skos:Concept rdf:about="urn:cgi:classifierScheme:CGI:SimpleLithology:200811:framestone">
		<skos:definition>Carbonate reef rock consisting of a rigid framework of colonies, shells or skeletons, with internal cavities filled with fine sediment; usually created through the activities of colonial organisms. Source: Hallsworth &amp; Knox 1999; SLTTs, 2004, Table 15-3-1</skos:definition>
		<skos:prefLabel xml:lang="en">Framestone</skos:prefLabel>
		<skos:prefLabel xml:lang="fr">framestone</skos:prefLabel>
		<skos:prefLabel xml:lang="it">framestone</skos:prefLabel>
		<skos:inScheme rdf:resource="urn:cgi:classifierScheme:CGI:SimpleLithology:200811"/>
	</skos:Concept>
	<skos:Concept rdf:about="urn:cgi:classifierScheme:CGI:SimpleLithology:200811:carbonate_wackestone">
		<skos:definition>Carbonate sedimentary rock with discernible mud supported depositional texture and containing greater than 10 percent grains. Source: Dunham 1962</skos:definition>
		<skos:prefLabel xml:lang="en">Carbonate wackestone</skos:prefLabel>
		<skos:prefLabel xml:lang="fr">calcaire wackestone</skos:prefLabel>
		<skos:prefLabel xml:lang="it">wackestone carbonatico</skos:prefLabel>
		<skos:inScheme rdf:resource="urn:cgi:classifierScheme:CGI:SimpleLithology:200811"/>
	</skos:Concept>
	<skos:Concept rdf:about="urn:cgi:classifierScheme:CGI:SimpleLithology:200811:organic_rich_sedimentary_rock">
		<skos:definition>Sedimentary rock with color, composition, texture and apparent density indicating greater than 50 percent organic content by weight on a moisture-free basis. Source: SLTTs 2004</skos:definition>
		<skos:prefLabel xml:lang="en">Organic rich sedimentary rock</skos:prefLabel>
		<skos:prefLabel xml:lang="fr">roche sédimentaire enrichie en matière organique</skos:prefLabel>
		<skos:prefLabel xml:lang="it">roccia sedimentaria ricca di materia organica</skos:prefLabel>
		<skos:inScheme rdf:resource="urn:cgi:classifierScheme:CGI:SimpleLithology:200811"/>
	</skos:Concept>
	<skos:Concept rdf:about="urn:cgi:classifierScheme:CGI:SimpleLithology:200811:coal">
		<skos:definition>Hard, black, organic rich sedimentary rock that yields greater than 8,300 Btu on a moist, mineral-matter-free basis, or contains greater than 69 percent fixed carbon on a dry, mineral-matter-free basis; formed from the compaction or induration of variously altered plant remains similar to those of peaty deposits. Source: ASTM 2002; Schopf 1956</skos:definition>
		<skos:prefLabel xml:lang="en">Coal</skos:prefLabel>
		<skos:prefLabel xml:lang="fr">charbons</skos:prefLabel>
		<skos:prefLabel xml:lang="it">carbone</skos:prefLabel>
		<skos:inScheme rdf:resource="urn:cgi:classifierScheme:CGI:SimpleLithology:200811"/>
	</skos:Concept>
	<skos:Concept rdf:about="urn:cgi:classifierScheme:CGI:SimpleLithology:200811:non_clastic_siliceous_sedimentary_rock">
		<skos:definition>Sedimentary rock that consists of at least 50 percent silicate mineral material, deposited directly by chemical or biological processes at the depositional surface, or in particles formed by chemical or biological processes within the basin of deposition. Source: SLTTs 2004</skos:definition>
		<skos:prefLabel xml:lang="en">Non-clastic siliceous sedimentary rock</skos:prefLabel>
		<skos:prefLabel xml:lang="fr">roche sédimentaire siliceuse non-clastique</skos:prefLabel>
		<skos:prefLabel xml:lang="it">roccia sedimentaria silicea non clastica</skos:prefLabel>
		<skos:inScheme rdf:resource="urn:cgi:classifierScheme:CGI:SimpleLithology:200811"/>
	</skos:Concept>
	<skos:Concept rdf:about="urn:cgi:classifierScheme:CGI:SimpleLithology:200811:biogenic_silica_sedimentary_rock">
		<skos:definition>Sedimentary rock that consists of at least 50 percent silicate mineral material, deposited directly by biological processes at the depositional surface, or in particles formed by biological processes within the basin of deposition. Source: based on NADM SLTT sedimentary; Hallsworth &amp; Knox 1999</skos:definition>
		<skos:prefLabel xml:lang="en">Biogenic silica sedimentary rock</skos:prefLabel>
		<skos:prefLabel xml:lang="fr">roche sédimentaire siliceuse biogénique</skos:prefLabel>
		<skos:prefLabel xml:lang="it">roccia sedimentaria biogenica silicea</skos:prefLabel>
		<skos:inScheme rdf:resource="urn:cgi:classifierScheme:CGI:SimpleLithology:200811"/>
	</skos:Concept>
	<skos:Concept rdf:about="urn:cgi:classifierScheme:CGI:SimpleLithology:200811:iron_rich_sedimentary_rock">
		<skos:definition>Sedimentary rock that consists of at least 50 percent iron-bearing minerals (hematite, magnetite, limonite-group, siderite, iron-sulfides), as determined by hand-lens or petrographic analysis. Corresponds to a rock typically containing 15 percent iron by weight. Source: Hallsworth and Knox 1999; SLTTs 2004</skos:definition>
		<skos:prefLabel xml:lang="en">Iron rich sedimentary rock</skos:prefLabel>
		<skos:prefLabel xml:lang="fr">roche sédimentaire ferrugineux</skos:prefLabel>
		<skos:prefLabel xml:lang="it">roccia sedimentaria ferrifera</skos:prefLabel>
		<skos:inScheme rdf:resource="urn:cgi:classifierScheme:CGI:SimpleLithology:200811"/>
	</skos:Concept>
	<skos:Concept rdf:about="urn:cgi:classifierScheme:CGI:SimpleLithology:200811:phosphorite">
		<skos:definition>Sedimentary rock in which at least 50 percent of the primary or recrystallized constituents are phosphate minerals. Most commonly occurs as a bedded primary or reworked secondary marine rock, composed of microcrystalline carbonate fluorapatite in the form of lamina, pellets, oolites and nodules, and skeletal, shell and bone fragments. Source: Hallsworth&amp;Knox 1999, Jackson 1997</skos:definition>
		<skos:prefLabel xml:lang="en">Phosphorite</skos:prefLabel>
		<skos:prefLabel xml:lang="fr">phosphorite</skos:prefLabel>
		<skos:prefLabel xml:lang="it">fosforite</skos:prefLabel>
		<skos:inScheme rdf:resource="urn:cgi:classifierScheme:CGI:SimpleLithology:200811"/>
	</skos:Concept>
	<skos:Concept rdf:about="urn:cgi:classifierScheme:CGI:SimpleLithology:200811:acidic_igneous_material">
		<skos:definition>Igneous material with more than 63 percent SiO2. Source: after LeMaitre et al. 2002</skos:definition>
		<skos:prefLabel xml:lang="en">Acidic igneous material</skos:prefLabel>
		<skos:prefLabel xml:lang="fr">matériel igné acide</skos:prefLabel>
		<skos:prefLabel xml:lang="it">materiale igneo acido</skos:prefLabel>
		<skos:inScheme rdf:resource="urn:cgi:classifierScheme:CGI:SimpleLithology:200811"/>
		<skos:broader rdf:resource="urn:cgi:classifierScheme:CGI:SimpleLithology:200811:igneous_material"/>
	</skos:Concept>
	<skos:Concept rdf:about="urn:cgi:classifierScheme:CGI:SimpleLithology:200811:igneous_material">
		<skos:definition>Earth material formed as a result of igneous processes, eg. intrusion and cooling of magma in the crust, volcanic eruption. Source: This vocabulary</skos:definition>
		<skos:prefLabel xml:lang="en">Igneous material</skos:prefLabel>
		<skos:prefLabel xml:lang="fr">matériel igné</skos:prefLabel>
		<skos:prefLabel xml:lang="it">materiale igneo</skos:prefLabel>
		<skos:inScheme rdf:resource="urn:cgi:classifierScheme:CGI:SimpleLithology:200811"/>
		<skos:broader rdf:resource="urn:cgi:classifierScheme:CGI:SimpleLithology:200811:compound_material"/>
	</skos:Concept>
	<skos:Concept rdf:about="urn:cgi:classifierScheme:CGI:SimpleLithology:200811:basic_igneous_material">
		<skos:definition>Igneous material with between 45 and 52 percent SiO2. Source: after LeMaitre et al. 2002</skos:definition>
		<skos:prefLabel xml:lang="en">Basic igneous material</skos:prefLabel>
		<skos:prefLabel xml:lang="fr">matériel igné basique</skos:prefLabel>
		<skos:prefLabel xml:lang="it">materiale igneo basico</skos:prefLabel>
		<skos:inScheme rdf:resource="urn:cgi:classifierScheme:CGI:SimpleLithology:200811"/>
	</skos:Concept>
	<skos:Concept rdf:about="urn:cgi:classifierScheme:CGI:SimpleLithology:200811:intermediate_composition_igneous_material">
		<skos:definition>Igneous material with between 52 and 63 percent SiO2. Source: after LeMaitre et al. 2002</skos:definition>
		<skos:prefLabel xml:lang="en">Intermediate composition igneous material</skos:prefLabel>
		<skos:prefLabel xml:lang="fr">matériel igné de composition intermédiaire</skos:prefLabel>
		<skos:prefLabel xml:lang="it">materiale igneo a composizione intermedia</skos:prefLabel>
		<skos:inScheme rdf:resource="urn:cgi:classifierScheme:CGI:SimpleLithology:200811"/>
	</skos:Concept>
	<skos:Concept rdf:about="urn:cgi:classifierScheme:CGI:SimpleLithology:200811:fragmental_igneous_material">
		<skos:definition>Igneous material of unspecified consolidation state in which greater than 75 percent of the rock consists of fragments produced as a result of igneous rock-forming process. Source: CGI concepts task group</skos:definition>
		<skos:prefLabel xml:lang="en">Fragmental igneous material</skos:prefLabel>
		<skos:prefLabel xml:lang="fr">matériel igné fragmenté</skos:prefLabel>
		<skos:prefLabel xml:lang="it">materiale igneo frammentato</skos:prefLabel>
		<skos:inScheme rdf:resource="urn:cgi:classifierScheme:CGI:SimpleLithology:200811"/>
	</skos:Concept>
	<skos:Concept rdf:about="urn:cgi:classifierScheme:CGI:SimpleLithology:200811:pyroclastic_material">
		<skos:definition>Fragmental igneous material that consists of more than 75 percent of particles formed by disruption as a direct result of volcanic action. Source: LeMaitre et al. 2002</skos:definition>
		<skos:prefLabel xml:lang="en">Pyroclastic material</skos:prefLabel>
		<skos:prefLabel xml:lang="fr">matériel pyroclastique</skos:prefLabel>
		<skos:prefLabel xml:lang="it">materiale piroclastico</skos:prefLabel>
		<skos:inScheme rdf:resource="urn:cgi:classifierScheme:CGI:SimpleLithology:200811"/>
	</skos:Concept>
	<skos:Concept rdf:about="urn:cgi:classifierScheme:CGI:SimpleLithology:200811:clastic_sedimentary_material">
		<skos:definition>Sedimentary material of unspecified consolidation state in which at least 50 percent of the constituent particles were derived from erosion, weathering, or mass-wasting of pre-existing earth materials, and transported to the place of deposition by mechanical agents such as water, wind, ice and gravity. Source: SLTTs, 2004; Neuendorf et al., 2005</skos:definition>
		<skos:prefLabel xml:lang="en">Clastic sedimentary material</skos:prefLabel>
		<skos:prefLabel xml:lang="fr">matériel sédimentaire clastique</skos:prefLabel>
		<skos:prefLabel xml:lang="it">materiale sedimentario clastico</skos:prefLabel>
		<skos:inScheme rdf:resource="urn:cgi:classifierScheme:CGI:SimpleLithology:200811"/>
	</skos:Concept>
	<skos:Concept rdf:about="urn:cgi:classifierScheme:CGI:SimpleLithology:200811:sedimentary_material">
		<skos:definition>Material formed by accumulation of solid fragmental material deposited by air, water or ice, or material that accumulated by other natural agents such as chemical precipitation from solution or secretion by organisms. Includes both sediment and sedimentary rock. Includes epiclastic deposits. Source: SLTTs 2004</skos:definition>
		<skos:prefLabel xml:lang="en">Sedimentary material</skos:prefLabel>
		<skos:prefLabel xml:lang="fr">matériel sédimentaire</skos:prefLabel>
		<skos:prefLabel xml:lang="it">materiale sedimentario</skos:prefLabel>
		<skos:inScheme rdf:resource="urn:cgi:classifierScheme:CGI:SimpleLithology:200811"/>
		<skos:broader rdf:resource="urn:cgi:classifierScheme:CGI:SimpleLithology:200811:compound_material"/>
	</skos:Concept>
	<skos:Concept rdf:about="urn:cgi:classifierScheme:CGI:SimpleLithology:200811:organic_rich_sedimentary_material">
		<skos:definition>Sedimentary material in which 50 percent or more of the primary sedimentary material is organic carbon. Source: SLTTs 2004</skos:definition>
		<skos:prefLabel xml:lang="en">Organic rich sedimentary material</skos:prefLabel>
		<skos:prefLabel xml:lang="fr">matériel sédimentaire enrichie en matière organique</skos:prefLabel>
		<skos:prefLabel xml:lang="it">materiale sedimentario arricchito di materia organica </skos:prefLabel>
		<skos:inScheme rdf:resource="urn:cgi:classifierScheme:CGI:SimpleLithology:200811"/>
	</skos:Concept>
	<skos:Concept rdf:about="urn:cgi:classifierScheme:CGI:SimpleLithology:200811:phosphate_rich_sedimentary_material">
		<skos:definition>Sedimentary material in which at least 50 percent of the primary and/or recrystallized constituents are phosphate minerals. Source: SLTTs 2004</skos:definition>
		<skos:prefLabel xml:lang="en">Phosphate rich sedimentary material</skos:prefLabel>
		<skos:prefLabel xml:lang="fr">matériel sédimentaire phosphaté</skos:prefLabel>
		<skos:prefLabel xml:lang="it">materiale sedimentario ricco di fosfati</skos:prefLabel>
		<skos:inScheme rdf:resource="urn:cgi:classifierScheme:CGI:SimpleLithology:200811"/>
	</skos:Concept>
	<skos:Concept rdf:about="urn:cgi:classifierScheme:CGI:SimpleLithology:200811:iron_rich_sedimentary_material">
		<skos:definition>Sedimentary material of unspecified consolidation state that consists of at least 50 percent iron-bearing minerals (hematite, magnetite, limonite-group, siderite, iron-sulfides), as determined by hand-lens or petrographic analysis. Corresponds to a rock typically containing 15 percent iron by weight. Source: SLTTs 2004</skos:definition>
		<skos:prefLabel xml:lang="en">Iron rich sedimentary material</skos:prefLabel>
		<skos:prefLabel xml:lang="fr">matériel sédimentaire ferrugineux</skos:prefLabel>
		<skos:prefLabel xml:lang="it">materiale sedimentario ferrifero</skos:prefLabel>
		<skos:inScheme rdf:resource="urn:cgi:classifierScheme:CGI:SimpleLithology:200811"/>
	</skos:Concept>
	<skos:Concept rdf:about="urn:cgi:classifierScheme:CGI:SimpleLithology:200811:carbonate_sedimentary_material">
		<skos:definition>Sedimentary material in which at least 50 percent of the primary and/or recrystallized constituents are composed of one (or more) of the carbonate minerals calcite, aragonite and dolomite, in particles of intrabasinal origin. Source: SLTTs 2004</skos:definition>
		<skos:prefLabel xml:lang="en">Carbonate sedimentary material</skos:prefLabel>
		<skos:prefLabel xml:lang="fr">matériel sédimentaire carbonaté </skos:prefLabel>
		<skos:prefLabel xml:lang="it">materiale sedimentario carbonatico</skos:prefLabel>
		<skos:inScheme rdf:resource="urn:cgi:classifierScheme:CGI:SimpleLithology:200811"/>
	</skos:Concept>
	<skos:Concept rdf:about="urn:cgi:classifierScheme:CGI:SimpleLithology:200811:calcareous_carbonate_sedimentary_material">
		<skos:definition>Carbonate sedimentary material of unspecified consolidation state with a calcite (plus aragonite) to dolomite ratio greater than 1 to 1. Includes lime-sediments, limestone and dolomitic limestone. Source: after Hallsworth &amp; Knox 1999</skos:definition>
		<skos:prefLabel xml:lang="en">Calcareous carbonate sedimentary material</skos:prefLabel>
		<skos:prefLabel xml:lang="fr">matériel sédimentaire carbonaté calcaire</skos:prefLabel>
		<skos:prefLabel xml:lang="it">materiale sedimentario calcareo carbonatico</skos:prefLabel>
		<skos:inScheme rdf:resource="urn:cgi:classifierScheme:CGI:SimpleLithology:200811"/>
	</skos:Concept>
	<skos:Concept rdf:about="urn:cgi:classifierScheme:CGI:SimpleLithology:200811:dolomitic_or_magnesian_sedimentary_material">
		<skos:definition>Carbonate sedimentary material of unspecified consolidation degree with a ratio of magnesium carbonate to calcite (plus aragonite) greater than 1 to 1. Includes dolomite sediment, dolostone, lime dolostone and magnesite-stone. Source: after SLTTs 2004, Hallsworth and Knox 1999</skos:definition>
		<skos:prefLabel xml:lang="en">Dolomitic or magnesian sedimentary material</skos:prefLabel>
		<skos:prefLabel xml:lang="fr">matériel sédimentaire dolomitique ou magnésien</skos:prefLabel>
		<skos:prefLabel xml:lang="it">materiale sedimentario dolomitico o magnesiaco</skos:prefLabel>
		<skos:inScheme rdf:resource="urn:cgi:classifierScheme:CGI:SimpleLithology:200811"/>
	</skos:Concept>
	<skos:Concept rdf:about="urn:cgi:classifierScheme:CGI:SimpleLithology:200811:non_clastic_siliceous_sedimentary_material">
		<skos:definition>Sedimentary material that consists of at least 50 percent silicate mineral material, deposited directly by chemical or biological processes at the depositional surface, or in particles formed by chemical or biological processes within the basin of deposition. Source: SLTTs 2004</skos:definition>
		<skos:prefLabel xml:lang="en">Non-clastic siliceous sedimentary material</skos:prefLabel>
		<skos:prefLabel xml:lang="fr">matériel sédimentaire siliceux non-clastique</skos:prefLabel>
		<skos:prefLabel xml:lang="it">materiale sedimentario siliceo non-clastico</skos:prefLabel>
		<skos:inScheme rdf:resource="urn:cgi:classifierScheme:CGI:SimpleLithology:200811"/>
	</skos:Concept>
	<skos:Concept rdf:about="urn:cgi:classifierScheme:CGI:SimpleLithology:200811:evaporite">
		<skos:definition>Nonclastic sedimentary rock composed of at least 50 percent non-carbonate salts, including chloride, sulfate or borate minerals; formed through precipitation of mineral salts from a saline solution (non-carbonate salt rock). Source: Jackson 1997; SLTTs 2004</skos:definition>
		<skos:prefLabel xml:lang="en">Evaporite</skos:prefLabel>
		<skos:prefLabel xml:lang="fr">évaporites</skos:prefLabel>
		<skos:prefLabel xml:lang="it">evaporite</skos:prefLabel>
		<skos:inScheme rdf:resource="urn:cgi:classifierScheme:CGI:SimpleLithology:200811"/>
	</skos:Concept>
	<skos:Concept rdf:about="urn:cgi:classifierScheme:CGI:SimpleLithology:200811:anthropogenic_material">
		<skos:definition>Material known to have artificial (human-related) origin; insufficient information to classify in more detail. Source: this vocabulary</skos:definition>
		<skos:prefLabel xml:lang="en">Anthropogenic material</skos:prefLabel>
		<skos:prefLabel xml:lang="fr">matériel anthropique</skos:prefLabel>
		<skos:prefLabel xml:lang="it">materiale antropico</skos:prefLabel>
		<skos:inScheme rdf:resource="urn:cgi:classifierScheme:CGI:SimpleLithology:200811"/>
		<skos:broader rdf:resource="urn:cgi:classifierScheme:CGI:SimpleLithology:200811:compound_material"/>
	</skos:Concept>
</rdf:RDF>