@prefix gsmlgt: <http://my.example.org/ont/gsmlgt#> .
@prefix rdf:   <http://www.w3.org/1999/02/22-rdf-syntax-ns#> .
@prefix owl:   <http://www.w3.org/2002/07/owl#> .
@prefix xsd:   <http://www.w3.org/2001/XMLSchema#> .
@prefix skos:  <http://www.w3.org/2004/02/skos/core#> .
@prefix rdfs:  <http://www.w3.org/2000/01/rdf-schema#> .

gsmlgt:start  a          owl:ObjectProperty ;
        rdfs:range       gsmlgt:TimeOrdinalEraBoundary ;
        skos:definition  "The start property is an association to a TimeOrdinalEraBoundary that defines the start (the oldest) boundary of the era."@en .

gsmlgt:StratigraphicSection
        a                owl:Class ;
        skos:definition  "A type of stratigraphic section used to define a globally agreed standard period of geologic time. This class does not have any properties beyond those inherited from <font color=\"#4f81bd\">StratigraphicSection</font>."@en .

gsmlgt:TimeOrdinalEra
        a                owl:Class ;
        skos:definition  "<font color=\"#4f81bd\">TimeOrdinalEra</font> is a period of time between two time boundaries.  The association of an era with a stratotype is optional.  In the GSSP approach recommended by ICS for the Global Geologic Timescale, Unit Stratotypes are not used.  Rather, the association of an era with geologic units and sections is indirect, via the association of an era with boundaries, which are in turn tied to stratotype points, which occur within host stratotype sections.  <font color=\"#4f81bd\">TimeOrdinalEra</font> can be composed of other eras and organized into an arbitrarily nested tree."@en .

gsmlgt:StandardGlobalNumericalAge
        a                owl:Class ;
        rdfs:subClassOf  gsmlgt:NumericEraBoundary ;
        skos:definition  "A standard numeric age point (a numeric analogue to a 'golden spike') is applicable to the formal subdivision of the Precambrian, and perhaps the Pleistocene/Holocene boundary ( <a href=\"http://www.stratigraphy.org/index.php/ics-chart-timescale\"><font color=\"#0000ff\"><u>http://www.stratigraphy.org/index.php/ics-chart-timescale</u></font></a>). The boundary is not defined from a physical stratotype, although it can be influence by some, but placed at a convenient numerical value."@en .

gsmlgt:accessibility  a  owl:DatatypeProperty ;
        rdfs:range       xsd:string ;
        skos:definition  "The property <font color=\"#4f81bd\">accessibility:Primitive::CharacterString</font> contains a description of the ability to access the stratigraphic section."@en .

gsmlgt:conservation  a   owl:DatatypeProperty ;
        rdfs:range       xsd:string ;
        skos:definition  "The property <font color=\"#4f81bd\">conservation:Primitive::CharacterString</font> contains a description of measures to conserve the stratigraphic section."@en .

gsmlgt:geologicSetting
        a                owl:DatatypeProperty ;
        rdfs:range       xsd:string ;
        skos:definition  "The property <font color=\"#4f81bd\">geologicSetting:Primitive::CharacterString</font> contains a description of the geologic setting of the stratigraphic section."@en .

gsmlgt:geologicDescription
        a                owl:DatatypeProperty ;
        rdfs:range       xsd:string ;
        skos:definition  "The <font color=\"#4f81bd\">geologicDescription:Primitive::CharacterString</font> contains a description of the geology of the stratigraphic section (e.g., lithology, paleontology, paleogeography, etc.)."@en .

gsmlgt:GeochronologicBoundary.stratotype
        a                owl:ObjectProperty ;
        rdfs:domain      gsmlgt:GeochronologicBoundary ;
        rdfs:range       gsmlgt:StratigraphicPoint ;
        skos:definition  "The property stratotype is an association between a GeochronologicBoundary and a StratigraphicPoint that are associated with the boundary. A GeochronologicBoundary can be associated with more than one StratigraphicPoints, but only one may have GSSP ratified status. The others are proposed equivalents."@en .

gsmlgt:GeochronologicEra
        a                owl:Class ;
        rdfs:subClassOf  gsmlgt:TimeOrdinalEra ;
        skos:definition  "A <font color=\"#4f81bd\">GeochronologicEra</font> is a period of time between two <font color=\"#4f81bd\">GeochronologicBoundaries</font>. The association of a <font color=\"#4f81bd\">GeochronologicEra</font> with a stratotype is optional.  In the GSSP approach recommended by ICS for the Global Geologic Timescale, Unit Stratotypes are not used.  Rather, the association of an era with geologic units and sections is indirect, via the association of an era with boundaries, which are in turn tied to stratotype points, which occur within host stratotype sections."@en .

gsmlgt:GeologicTimescale
        a                owl:Class ;
        rdfs:subClassOf  gsmlgt:TimeOrdinalReferenceSystem ;
        skos:definition  "The classic \"Geologic Timescale\" (<a href=\"http://www.stratigraphy.org/index.php/ics-chart-timescale\"><font color=\"#0000ff\"><u>http://www.stratigraphy.org/index.php/ics-chart-timescale</u></font></a>) comprising an ordered, hierarchical set of named \"eras\" is an example of an Ordinal Temporal Reference System. It may be calibrated with reference to a numeric Temporal Coordinate System, but is, in principle, defined independently."@en .

gsmlgt:additionalCorrelationProperty
        a                owl:DatatypeProperty ;
        rdfs:range       xsd:string ;
        skos:definition  "The property <font color=\"#4f81bd\">additionnalCorrelationProperty:Primitive::CharacterString</font> contains any additional criteria used to establish the stratigraphic point."@en .

gsmlgt:end  a            owl:ObjectProperty ;
        rdfs:range       gsmlgt:TimeOrdinalEraBoundary ;
        skos:definition  "The end property is an association to a TimeOrdinalEraBoundary that defines the end (the youngest) boundary of the era."@en .

gsmlgt:rank  a           owl:ObjectProperty ;
        rdfs:range       owl:Class ;
        skos:definition  "The property <font color=\"#4f81bd\">rank:GeochronologicEraRank</font> contains a term from a vocabulary describing the rank of the time period (e.g., eon, era, period, stage)."@en .

gsmlgt:nextEra  a        owl:ObjectProperty ;
        rdfs:range       gsmlgt:TimeOrdinalEra ;
        skos:definition  "The property nextEra is an association between a TimeOrdinalEraBoundary and a TimeOrdinalEra to reference the succeeding era."@en .

gsmlgt:GlobalStratotypeSection
        a                owl:Class ;
        rdfs:subClassOf  gsmlgt:StratigraphicSection ;
        skos:definition  "A type of stratigraphic section used to define a globally agreed standard period of geologic time"@en .

gsmlgt:TimeOrdinalReferenceSystem
        a                owl:Class ;
        skos:definition  "<font color=\"#4f81bd\">TimeOrdinalReferenceSystem</font> is a time reference system comprised of an ordered set of time periods (time ordinal eras)."@en .

gsmlgt:member  a         owl:ObjectProperty ;
        rdfs:range       gsmlgt:TimeOrdinalEra ;
        skos:definition  "The property member is an association between a TimeOrdinalEra and another TimeOrdinalEra which is hierarchically below.  The referred TimeOrdinalEras are subdivision the current TimeOrdinalEra. Note that nesting shall not be cyclic.  A TimeOrdinalEra canâ€™t be a member of itself or any intermediate member (we can consider that member is a transitive property). This is not a model issue but a data coherence issue."@en .

gsmlgt:status  a         owl:DatatypeProperty ;
        rdfs:range       xsd:string ;
        skos:definition  "The property <font color=\"#4f81bd\">status:Primitive::CharacterString</font> contains a description of the status of stratigraphic point (e.g., formally accepted, etc.)."@en .

gsmlgt:primaryGuidingCriterion
        a                owl:DatatypeProperty ;
        rdfs:range       xsd:string ;
        skos:definition  "The property <font color=\"#4f81bd\">primaryGuidingCriterion:Primitive::CharacterString</font> contains a description of the primary criterion used to establish the stratigraphic point."@en .

gsmlgt:NumericEraBoundary
        a                owl:Class ;
        rdfs:subClassOf  gsmlgt:TimeOrdinalEraBoundary ;
        skos:definition  "<font color=\"#4f81bd\">NumericEraBoundary</font> is used for pre-Ediacaran and Pleistocene / Holocene boundaries in the standard timescale where boundaries are not defined by a material reference but as numerical values."@en .

<http://my.example.org/ont/gsmlgt>
        a                owl:Ontology ;
        owl:versionIRI   "http://my.example.org/ont/gsmlgt/4.1.0" ;
        owl:versionInfo  "4.1.0" ;
        skos:definition  "The Geologic Time package, developed by Simon Cox (CSIRO) and Steve Richard (Arizona Geological Survey), contains elements used to describe the classification of geologic time: time periods, time boundaries, and the relationships between them as defined by the IUGS International Commission on Stratigraphy (ICS - http://www.stratigraphy.org/)."@en .

gsmlgt:GeochronologicEra.stratotype
        a                owl:ObjectProperty ;
        rdfs:domain      gsmlgt:GeochronologicEra ;
        rdfs:range       gsmlgt:StratigraphicSection ;
        skos:definition  "The property stratotype is an association between a GeochronologicEra and StratigraphicSection that describes a type section that names the physical location or outcrop of a particular reference exposure of a stratigraphic sequence or stratigraphic boundary. A unit stratotype is the agreed reference point for a particular stratigraphic unit and a boundary stratotype is the reference for a particular boundary between strata (Wikipedia)."@en .

gsmlgt:GeochronologicBoundary
        a                owl:Class ;
        rdfs:subClassOf  gsmlgt:TimeOrdinalEraBoundary ;
        skos:definition  "A <font color=\"#4f81bd\">GeochronologicBoundary</font> is a boundary between two geochronologic time periods."@en .

gsmlgt:positionalUncertainty
        a                owl:ObjectProperty ;
        rdfs:range       owl:Class ;
        skos:definition  "The property <font color=\"#4f81bd\">positionalUncertainty</font> (<font color=\"#4f81bd\">SWE::Quantity</font>) contains a measure of the uncertainty in the estimate of the point in time of the era boundary."@en .

gsmlgt:previousEra  a    owl:ObjectProperty ;
        rdfs:range       gsmlgt:TimeOrdinalEra ;
        skos:definition  "The property previousEra is an association between a TimeOrdinalEraBoundary and a TimeOrdinalEra to reference the preceding (oldest) era."@en .

gsmlgt:GlobalStratotypePoint
        a                owl:Class ;
        rdfs:subClassOf  gsmlgt:StratigraphicPoint ;
        skos:definition  "A type of stratigraphic point used to define a globally agreed point in geologic time.  This class does not have any properties beyond those inherited from <font color=\"#4f81bd\">StratigraphicPoint</font>."@en .

gsmlgt:component  a      owl:ObjectProperty ;
        rdfs:range       gsmlgt:TimeOrdinalEra ;
        skos:definition  "The property component is an association to a TimeOrdinalEra that is part of the TimeOrdinalReferenceSystem.  A TimeOrdinalReferenceSystem is composed of a collection of TimeOrdinalEras."@en .

gsmlgt:position  a       owl:ObjectProperty ;
        rdfs:range       owl:Class ;
        skos:definition  "The <font color=\"#4f81bd\">position:TM_Instant</font> property describes a point in time corresponding to the era boundary."@en .

gsmlgt:observationalBasis
        a                owl:ObjectProperty ;
        rdfs:range       owl:Class ;
        skos:definition  "The property observationalBasis is be an association between a TimeOrdinalEraBoundary and an OM::OM_Observation in support of the existence of the boundary defined by geochronology, paleontology, or other evidence."@en .

gsmlgt:referencePoint
        a                owl:ObjectProperty ;
        rdfs:range       gsmlgt:TimeOrdinalEraBoundary ;
        skos:definition  "The property referencePoint is an association between a TimeOrdinalReferenceSystem and a TimeOrdinalEraBoundary.  A TimeOrdinalReferenceSystem refers to two reference points defining the extent of the system."@en .

gsmlgt:TimeOrdinalEraBoundary
        a                owl:Class ;
        skos:definition  "A <font color=\"#4f81bd\">TimeOrdinalEraBoundary</font> is a point in Earth's history which bounds a <font color=\"#4f81bd\">TimeOrdinalEra</font>."@en .

gsmlgt:StratigraphicPoint
        a                owl:Class ;
        skos:definition  "A point in the stratigraphic record used to define a geochronologic boundary or point in geologic time."@en .
