<?xml version="1.0" encoding="utf-8"?>
<rdf:RDF xmlns:rdf="http://www.w3.org/1999/02/22-rdf-syntax-ns#" xmlns:skos="http://www.w3.org/2004/02/skos/core#" xmlns:dc="http://purl.org/dc/elements/1.1/" xmlns:owl="http://www.w3.org/2002/07/owl#" xmlns:rdfs="http://www.w3.org/2000/01/rdf-schema#" xmlns:xlink="http://www.w3.org/1999/xlink">
  <!--==========================================================================-->
  <!-- Generated by XL2XML Framework (CSIRO).                                   -->
  <!-- -                                                                        -->
  <!-- CDTG XLS to SKOS ruleset, SMR revision -->
  <!-- Ruleset revision date: 2009-06-23   -->
  <!-- Ruleset author: Pavel Golodoniuc, CSIRO Exploration and Mining;
Modified by Stephen M Richard 2009-07-14			-->
  <!-- -                                                                        -->
  <!-- Content owned by originators.                                            -->
  <!--==========================================================================-->
  <skos:ConceptScheme rdf:about="urn:cgi:classifierScheme:CGI:ParticleAspectRatio:200811">
    <skos:prefLabel xml:lang="en">ParticleAspectRatio</skos:prefLabel>
    <skos:changeNote>
      <rdf:Description>
        <rdf:value>Converted from Excel document.</rdf:value>
        <dc:date>2009-07-14</dc:date>
        <dc:creator>Stephen M Richard</dc:creator>
      </rdf:Description>
    </skos:changeNote>
    <skos:editorialNote>This file contains the 200811 version of CGI Particle Aspect Ratio vocabulary. AspectRatio describes the geometry of particles based on the ratios of lengths of long, intermediate and short axes of grains. Equates to sphericity in sedimentary rocks (ie: the degree to which the shape of a particle approximates a sphere). A quantitative specification is based on the ratio of lengths of long, intermediate and short axes of grain shape (Sneed and Folk, 1958; Zingg, 1935). This vocabulary includes terms for specifying average shape of some collection of particles.(eg: prolate, slightly flattened, very bladed, equant, acicular, tabular). Numeric shape values from Sneed and Folk (1958) are best understood by looking at the pictures of particles with the different shapes there and in Pettijohn et al. (1972).</skos:editorialNote>
  </skos:ConceptScheme>
  <skos:Concept rdf:about="urn:cgi:classifier:CGI:ParticleAspectRatio:200811:equant">
    <skos:inScheme rdf:resource="urn:cgi:classifierScheme:CGI:ParticleAspectRatio:200811" />
    <skos:definition>Particles are compact in Sneed &amp; Folk (1958); ratio of S/L is greater than 0.7.</skos:definition>
    <skos:prefLabel xml:lang="en">Equant</skos:prefLabel>
    <skos:notation rdf:datatype="urn:cgi:classifierScheme:CGI:ParticleAspectRatio:200811">equant</skos:notation>
    <skos:notation rdf:datatype="LocalHierarchyKey">1..</skos:notation>
    <skos:historyNote>Sneed and Folk, 1958; Pettijohn et al., 1972; NADM SLTTs, 2004</skos:historyNote>
  </skos:Concept>
  <skos:Concept rdf:about="urn:cgi:classifier:CGI:ParticleAspectRatio:200811:prolate">
    <skos:inScheme rdf:resource="urn:cgi:classifierScheme:CGI:ParticleAspectRatio:200811" />
    <skos:definition>Particles are in 'elongated group' in Sneed &amp; Folk, (1958); S/L is less than 0.7 and (L-I)/(L-S) is greater than 0.66.</skos:definition>
    <skos:prefLabel xml:lang="en">Prolate</skos:prefLabel>
    <skos:notation rdf:datatype="urn:cgi:classifierScheme:CGI:ParticleAspectRatio:200811">prolate</skos:notation>
    <skos:notation rdf:datatype="LocalHierarchyKey">2..</skos:notation>
    <skos:historyNote>Sneed and Folk, 1958; Pettijohn et al., 1972; NADM SLTTs, 2004</skos:historyNote>
  </skos:Concept>
  <skos:Concept rdf:about="urn:cgi:classifier:CGI:ParticleAspectRatio:200811:strongly_prolate">
    <skos:inScheme rdf:resource="urn:cgi:classifierScheme:CGI:ParticleAspectRatio:200811" />
    <skos:definition>Particles are very elongated in Sneed&amp;Folk, (1958); S/L is less than 0.3 and (L-I)/(L-S) is greater than 0.66.</skos:definition>
    <skos:prefLabel xml:lang="en">Strongly prolate</skos:prefLabel>
    <skos:notation rdf:datatype="urn:cgi:classifierScheme:CGI:ParticleAspectRatio:200811">strongly_prolate</skos:notation>
    <skos:broader rdf:resource="urn:cgi:classifier:CGI:ParticleAspectRatio:200811:prolate" />
    <skos:notation rdf:datatype="LocalHierarchyKey">2.1.</skos:notation>
    <skos:historyNote>Sneed and Folk, 1958; Pettijohn et al., 1972; NADM SLTTs, 2004</skos:historyNote>
  </skos:Concept>
  <skos:Concept rdf:about="urn:cgi:classifier:CGI:ParticleAspectRatio:200811:fibrous">
    <skos:inScheme rdf:resource="urn:cgi:classifierScheme:CGI:ParticleAspectRatio:200811" />
    <skos:definition>Particles are so elongate they are fibrous.</skos:definition>
    <skos:prefLabel xml:lang="en">Fibrous</skos:prefLabel>
    <skos:notation rdf:datatype="urn:cgi:classifierScheme:CGI:ParticleAspectRatio:200811">fibrous</skos:notation>
    <skos:broader rdf:resource="urn:cgi:classifier:CGI:ParticleAspectRatio:200811:strongly_prolate" />
    <skos:notation rdf:datatype="LocalHierarchyKey">2.1.1</skos:notation>
    <skos:historyNote>Sneed and Folk, 1958; Pettijohn et al., 1972; NADM SLTTs, 2004</skos:historyNote>
  </skos:Concept>
  <skos:Concept rdf:about="urn:cgi:classifier:CGI:ParticleAspectRatio:200811:prolate_medium">
    <skos:inScheme rdf:resource="urn:cgi:classifierScheme:CGI:ParticleAspectRatio:200811" />
    <skos:definition>Particle are 'just elongated' in Sneed&amp;Folk, (1958); S/L is between 0.3 and 0.5 and (L-I)/(L-S) is greater than 0.66.</skos:definition>
    <skos:prefLabel xml:lang="en">Prolate medium</skos:prefLabel>
    <skos:notation rdf:datatype="urn:cgi:classifierScheme:CGI:ParticleAspectRatio:200811">prolate_medium</skos:notation>
    <skos:broader rdf:resource="urn:cgi:classifier:CGI:ParticleAspectRatio:200811:prolate" />
    <skos:notation rdf:datatype="LocalHierarchyKey">2.2.</skos:notation>
    <skos:historyNote>Sneed and Folk, 1958; Pettijohn et al., 1972; NADM SLTTs, 2004</skos:historyNote>
  </skos:Concept>
  <skos:Concept rdf:about="urn:cgi:classifier:CGI:ParticleAspectRatio:200811:slightly_prolate">
    <skos:inScheme rdf:resource="urn:cgi:classifierScheme:CGI:ParticleAspectRatio:200811" />
    <skos:definition>Particles are compact-elongated in Sneed&amp;Folk, (1958); S/L is between 0.5 and 0.7 and (L-I)/(L-S) is greater than 0.66.</skos:definition>
    <skos:prefLabel xml:lang="en">Slightly prolate</skos:prefLabel>
    <skos:notation rdf:datatype="urn:cgi:classifierScheme:CGI:ParticleAspectRatio:200811">slightly_prolate</skos:notation>
    <skos:broader rdf:resource="urn:cgi:classifier:CGI:ParticleAspectRatio:200811:prolate" />
    <skos:notation rdf:datatype="LocalHierarchyKey">2.3.</skos:notation>
    <skos:historyNote>Sneed and Folk, 1958; Pettijohn et al., 1972; NADM SLTTs, 2004</skos:historyNote>
  </skos:Concept>
  <skos:Concept rdf:about="urn:cgi:classifier:CGI:ParticleAspectRatio:200811:oblate">
    <skos:inScheme rdf:resource="urn:cgi:classifierScheme:CGI:ParticleAspectRatio:200811" />
    <skos:definition>Particles are in 'platy group' in Sneed&amp;Folk, (1958); S/L is less than 0.7 and (L-I)/(L-S) is less than 0.33.</skos:definition>
    <skos:prefLabel xml:lang="en">Oblate</skos:prefLabel>
    <skos:notation rdf:datatype="urn:cgi:classifierScheme:CGI:ParticleAspectRatio:200811">oblate</skos:notation>
    <skos:notation rdf:datatype="LocalHierarchyKey">3..</skos:notation>
    <skos:historyNote>Sneed and Folk, 1958; Pettijohn et al., 1972; NADM SLTTs, 2004</skos:historyNote>
  </skos:Concept>
  <skos:Concept rdf:about="urn:cgi:classifier:CGI:ParticleAspectRatio:200811:slightly_flattened">
    <skos:inScheme rdf:resource="urn:cgi:classifierScheme:CGI:ParticleAspectRatio:200811" />
    <skos:definition>Particles are 'Compact-platy' in Sneed&amp;Folk, (1958); S/L is between 0.5 and 0.7 and (L-I)/(L-S) is less than 0.33.</skos:definition>
    <skos:prefLabel xml:lang="en">Slightly flattened</skos:prefLabel>
    <skos:notation rdf:datatype="urn:cgi:classifierScheme:CGI:ParticleAspectRatio:200811">slightly_flattened</skos:notation>
    <skos:broader rdf:resource="urn:cgi:classifier:CGI:ParticleAspectRatio:200811:oblate" />
    <skos:notation rdf:datatype="LocalHierarchyKey">3.1.</skos:notation>
    <skos:historyNote>Sneed and Folk, 1958; Pettijohn et al., 1972; NADM SLTTs, 2004</skos:historyNote>
  </skos:Concept>
  <skos:Concept rdf:about="urn:cgi:classifier:CGI:ParticleAspectRatio:200811:oblate_medium">
    <skos:inScheme rdf:resource="urn:cgi:classifierScheme:CGI:ParticleAspectRatio:200811" />
    <skos:definition>Particles are 'just platy' in Sneed&amp;Folk, (1958); S/L is between 0.3 and 0.5 and (L-I)/(L-S) is less than 0.33.</skos:definition>
    <skos:prefLabel xml:lang="en">Oblate medium</skos:prefLabel>
    <skos:notation rdf:datatype="urn:cgi:classifierScheme:CGI:ParticleAspectRatio:200811">oblate_medium</skos:notation>
    <skos:broader rdf:resource="urn:cgi:classifier:CGI:ParticleAspectRatio:200811:oblate" />
    <skos:notation rdf:datatype="LocalHierarchyKey">3.2.</skos:notation>
    <skos:historyNote>Sneed and Folk, 1958; Pettijohn et al., 1972; NADM SLTTs, 2004</skos:historyNote>
  </skos:Concept>
  <skos:Concept rdf:about="urn:cgi:classifier:CGI:ParticleAspectRatio:200811:strongly_flattened">
    <skos:inScheme rdf:resource="urn:cgi:classifierScheme:CGI:ParticleAspectRatio:200811" />
    <skos:definition>Particles are 'very platy' in Sneed&amp;Folk, (1958); S/L is less than 0.3 and (L-I)/(L-S) is less than 0.33.</skos:definition>
    <skos:prefLabel xml:lang="en">Strongly flattened</skos:prefLabel>
    <skos:notation rdf:datatype="urn:cgi:classifierScheme:CGI:ParticleAspectRatio:200811">strongly_flattened</skos:notation>
    <skos:broader rdf:resource="urn:cgi:classifier:CGI:ParticleAspectRatio:200811:oblate" />
    <skos:notation rdf:datatype="LocalHierarchyKey">3.3.</skos:notation>
    <skos:historyNote>Sneed and Folk, 1958; Pettijohn et al., 1972; NADM SLTTs, 2004</skos:historyNote>
  </skos:Concept>
  <skos:Concept rdf:about="urn:cgi:classifier:CGI:ParticleAspectRatio:200811:bladed">
    <skos:inScheme rdf:resource="urn:cgi:classifierScheme:CGI:ParticleAspectRatio:200811" />
    <skos:definition>Bladed group in Sneed&amp;Folk, (1958); S/L is less than 0.7 and (L-I)/(L-S) is between 0.33 and 0.66.</skos:definition>
    <skos:prefLabel xml:lang="en">Bladed</skos:prefLabel>
    <skos:notation rdf:datatype="urn:cgi:classifierScheme:CGI:ParticleAspectRatio:200811">bladed</skos:notation>
    <skos:notation rdf:datatype="LocalHierarchyKey">4..</skos:notation>
    <skos:historyNote>Sneed and Folk, 1958; Pettijohn et al., 1972; NADM SLTTs, 2004</skos:historyNote>
  </skos:Concept>
  <skos:Concept rdf:about="urn:cgi:classifier:CGI:ParticleAspectRatio:200811:very_bladed">
    <skos:inScheme rdf:resource="urn:cgi:classifierScheme:CGI:ParticleAspectRatio:200811" />
    <skos:definition>S/L is less than 0.3 and (L-I)/(L-S) is between 0.33 and 0.66 Sneed&amp;Folk, (1958).</skos:definition>
    <skos:prefLabel xml:lang="en">very bladed</skos:prefLabel>
    <skos:notation rdf:datatype="urn:cgi:classifierScheme:CGI:ParticleAspectRatio:200811">very_bladed</skos:notation>
    <skos:broader rdf:resource="urn:cgi:classifier:CGI:ParticleAspectRatio:200811:bladed" />
    <skos:notation rdf:datatype="LocalHierarchyKey">4.1.</skos:notation>
    <skos:historyNote>Sneed and Folk, 1958; Pettijohn et al., 1972; NADM SLTTs, 2004</skos:historyNote>
  </skos:Concept>
  <skos:Concept rdf:about="urn:cgi:classifier:CGI:ParticleAspectRatio:200811:bladed_medium">
    <skos:inScheme rdf:resource="urn:cgi:classifierScheme:CGI:ParticleAspectRatio:200811" />
    <skos:definition>S/L is between 0.3 and 0.5 and (L-I)/(L-S) is between 0.33 and 0.66 Sneed&amp;Folk, (1958).</skos:definition>
    <skos:prefLabel xml:lang="en">bladed medium</skos:prefLabel>
    <skos:notation rdf:datatype="urn:cgi:classifierScheme:CGI:ParticleAspectRatio:200811">bladed_medium</skos:notation>
    <skos:broader rdf:resource="urn:cgi:classifier:CGI:ParticleAspectRatio:200811:bladed" />
    <skos:notation rdf:datatype="LocalHierarchyKey">4.2.</skos:notation>
    <skos:historyNote>Sneed and Folk, 1958; Pettijohn et al., 1972; NADM SLTTs, 2004</skos:historyNote>
  </skos:Concept>
  <skos:Concept rdf:about="urn:cgi:classifier:CGI:ParticleAspectRatio:200811:compact_bladed">
    <skos:inScheme rdf:resource="urn:cgi:classifierScheme:CGI:ParticleAspectRatio:200811" />
    <skos:definition>S/L is between 0.5 and 0.7 and (L-I)/(L-S) is between 0.33 and 0.66 Sneed&amp;Folk, (1958).</skos:definition>
    <skos:prefLabel xml:lang="en">compact bladed</skos:prefLabel>
    <skos:notation rdf:datatype="urn:cgi:classifierScheme:CGI:ParticleAspectRatio:200811">compact_bladed</skos:notation>
    <skos:broader rdf:resource="urn:cgi:classifier:CGI:ParticleAspectRatio:200811:bladed" />
    <skos:notation rdf:datatype="LocalHierarchyKey">4.3.</skos:notation>
    <skos:historyNote>Sneed and Folk, 1958; Pettijohn et al., 1972; NADM SLTTs, 2004</skos:historyNote>
  </skos:Concept>
  <skos:Concept rdf:about="urn:cgi:classifier:CGI:ParticleAspectRatio:200811:particle_geometry_uncertain">
    <skos:inScheme rdf:resource="urn:cgi:classifierScheme:CGI:ParticleAspectRatio:200811" />
    <skos:definition>Particle form is uncertain or not categorizable, generally obscured by overprinting deformation, metamorphism, or alteration, but reason is not specified.</skos:definition>
    <skos:prefLabel xml:lang="en">Particle geometry uncertain</skos:prefLabel>
    <skos:notation rdf:datatype="urn:cgi:classifierScheme:CGI:ParticleAspectRatio:200811">particle_geometry_uncertain</skos:notation>
    <skos:notation rdf:datatype="LocalHierarchyKey">5..</skos:notation>
    <skos:historyNote>this vocabulary</skos:historyNote>
  </skos:Concept>
  <skos:Concept rdf:about="urn:cgi:classifier:CGI:ParticleAspectRatio:200811:form_not_specified">
    <skos:inScheme rdf:resource="urn:cgi:classifierScheme:CGI:ParticleAspectRatio:200811" />
    <skos:definition>Particle form may take any value. For use in normative descriptions.</skos:definition>
    <skos:prefLabel xml:lang="en">Form not specified</skos:prefLabel>
    <skos:notation rdf:datatype="urn:cgi:classifierScheme:CGI:ParticleAspectRatio:200811">form_not_specified</skos:notation>
    <skos:notation rdf:datatype="LocalHierarchyKey">6..</skos:notation>
    <skos:historyNote>this vocabulary</skos:historyNote>
  </skos:Concept>
</rdf:RDF>